@prefix : <http://mismo.org/Subset/> .
@prefix owl: <http://www.w3.org/2002/07/owl#> .
@prefix rdf: <http://www.w3.org/1999/02/22-rdf-syntax-ns#> .
@prefix xml: <http://www.w3.org/XML/1998/namespace> .
@prefix xsd: <http://www.w3.org/2001/XMLSchema#> .
@prefix rdfs: <http://www.w3.org/2000/01/rdf-schema#> .
@base <http://mismo.org/Subset/> .

<http://mismo.org/Subset/> rdf:type owl:Ontology ;
                            owl:imports <http://mismo.org/EnumeratedTypes/> ,
                                        <http://mismo.org/Containers/> ,
                                        <http://mismo.org/DataTypes/> ,
                                        <http://mismo.org/Extensions/> ;
                            rdfs:label "MISMOSubset"^^xsd:string .

#################################################################
#    Object Properties
#################################################################

###  http://mismo.org/Subset/CurrencyURI
:CurrencyURI rdf:type owl:ObjectProperty ;
             rdfs:domain :MISMOAmount ;
             rdfs:range <http://mismo.org/DataTypes/MISMOURI_Base> ;
             rdfs:comment "The currency the value represents. Recommend using the form urn:org:iso:www:4217:xxx where xxx is a three letter code from http://www.iso.org/iso/support/faqs/faqs_widely_used_standards/widely_used_standards_other/currency_codes/currency_codes_list-1.htm"^^xsd:string .


###  http://mismo.org/Subset/DataNotSuppliedReasonTypeAdditionalDescription
:DataNotSuppliedReasonTypeAdditionalDescription rdf:type owl:ObjectProperty ;
                                                rdfs:domain [ rdf:type owl:Class ;
                                                              owl:unionOf ( :MISMOAmount
                                                                            :MISMODate
                                                                            :MISMOIdentifier
                                                                            :MISMOIndicator
                                                                            :MISMORate
                                                                            :MISMOString
                                                                          )
                                                            ] ;
                                                rdfs:range <http://mismo.org/DataTypes/MISMOString_Base> ;
                                                rdfs:comment "A free-form text field used to provide a supplemental comment or remark regarding the Data Not Supplied Reason Type."^^xsd:string .


###  http://mismo.org/Subset/DataNotSuppliedReasonTypeOtherDescription
:DataNotSuppliedReasonTypeOtherDescription rdf:type owl:ObjectProperty ;
                                           rdfs:domain [ rdf:type owl:Class ;
                                                         owl:unionOf ( :MISMOAmount
                                                                       :MISMODate
                                                                       :MISMOIdentifier
                                                                       :MISMOIndicator
                                                                       :MISMORate
                                                                       :MISMOString
                                                                     )
                                                       ] ;
                                           rdfs:range <http://mismo.org/DataTypes/MISMOString_Base> ;
                                           rdfs:comment "A free-form text field used to capture the enumeration when Other is selected for Data Not Supplied Reason Type."^^xsd:string .


###  http://mismo.org/Subset/IdentifierEffectiveDate
:IdentifierEffectiveDate rdf:type owl:ObjectProperty ;
                         rdfs:domain :MISMOIdentifier ;
                         rdfs:range <http://mismo.org/DataTypes/MISMODate_Base> ;
                         rdfs:comment "The date on which the value represented by the MISMOIdentifier is effective as determined by the issuer or owner as specified by the IdentifierOwnerURI."^^xsd:string .


###  http://mismo.org/Subset/IdentifierOwnerURI
:IdentifierOwnerURI rdf:type owl:ObjectProperty ;
                    rdfs:domain :MISMOIdentifier ;
                    rdfs:range <http://mismo.org/DataTypes/MISMOURI_Base> ;
                    rdfs:comment "Identifies the owner or publisher of the identifier associated with a MISMO term with the class word of \"Identifier\" by means or a URI. This is an XML attribute."^^xsd:string .


###  http://mismo.org/Subset/SensitiveIndicator
:SensitiveIndicator rdf:type owl:ObjectProperty ;
                    rdfs:domain [ rdf:type owl:Class ;
                                  owl:unionOf ( :MISMOAmount
                                                :MISMODate
                                                :MISMOIdentifier
                                                :MISMOIndicator
                                                :MISMORate
                                                :MISMOString
                                              )
                                ] ;
                    rdfs:range <http://mismo.org/DataTypes/MISMOIndicator_Base> ;
                    rdfs:comment "Allows producers and consumers of XML instance documents that are valid MISMO V3 documents to mark any data point to be treated as sensitive. MISMO recommends that any use of a data point labeled as \"Sensitive Information\" in the LDD ALWAYS have this attribute set to \"true\"."^^xsd:string .


###  http://mismo.org/Subset/aboutVersions
:aboutVersions rdf:type owl:ObjectProperty ;
               rdfs:domain :DealSequence ;
               rdfs:range <http://mismo.org/Containers/AboutVersion> ;
               rdfs:comment "Information about one or more ABOUT_VERSION. Holds all occurrences of ABOUT_VERSION."^^xsd:string ;
               rdfs:label "about versions"^^xsd:string .


###  http://mismo.org/Subset/acceleratedPaymentProgramIndicator
:acceleratedPaymentProgramIndicator rdf:type owl:ObjectProperty ;
                                    rdfs:domain :Loan ;
                                    rdfs:range :MISMOIndicator ;
                                    rdfs:comment "Indicates that mortgagor participates in some sort of accelerated principal re-payment program which may be administered by a third party."^^xsd:string ;
                                    rdfs:label "Accelerated Payment Program Indicator"^^xsd:string .


###  http://mismo.org/Subset/accessoryDwellingUnitTotalCount
:accessoryDwellingUnitTotalCount rdf:type owl:ObjectProperty ;
                                 rdfs:domain :Property ;
                                 rdfs:range <http://mismo.org/DataTypes/MISMOCount> ;
                                 rdfs:comment "The total number of accessory dwelling units in the subject property. Possible examples may include in-law quarters, apartment over a garage, etc."^^xsd:string ;
                                 rdfs:label "Accessory Dwelling Unit Total Count"^^xsd:string .


###  http://mismo.org/Subset/ach
:ach rdf:type owl:ObjectProperty ;
     rdfs:domain [ rdf:type owl:Class ;
                   owl:unionOf ( :DealSet
                                 :Loan
                               )
                 ] ;
     rdfs:range <http://mismo.org/Containers/ACH> ;
     rdfs:comment "Information specific to drafting of automatic/regular payment."^^xsd:string .


###  http://mismo.org/Subset/ach-Indicator
:ach-Indicator rdf:type owl:ObjectProperty ;
               rdfs:domain :Loan ;
               rdfs:range :MISMOIndicator ;
               rdfs:comment "When true, indicates that a loan is enrolled in Automatic Clearing House (ACH) payment drafting."^^xsd:string ;
               rdfs:label "ACH Indicator"^^xsd:string .


###  http://mismo.org/Subset/activeLitigationIndicator
:activeLitigationIndicator rdf:type owl:ObjectProperty ;
                           rdfs:domain :Loan ;
                           rdfs:range :MISMOIndicator ;
                           rdfs:comment "When true, indicates that the loan is subject to active litigation."^^xsd:string ;
                           rdfs:label "Active Litigation Indicator"^^xsd:string .


###  http://mismo.org/Subset/additionalAddresses
:additionalAddresses rdf:type owl:ObjectProperty ;
                     rdfs:domain :Property ;
                     rdfs:range :Address ;
                     rdfs:comment "Information about one or more additional addresses associated with the property. Holds all occurrences of ADDITIONAL_ADDRESS."^^xsd:string ;
                     rdfs:label "additional addresses"^^xsd:string .


###  http://mismo.org/Subset/address
:address rdf:type owl:ObjectProperty ;
         rdfs:domain :Property ;
         rdfs:range :Address ;
         rdfs:comment "Address is based upon USPS publication 28. Publication 28 has two sections, format of an address on a piece of mail and data points that MAY compose an address. The data point children of ADDRESS are the union components of an address on a piece of mail or a package."^^xsd:string .


###  http://mismo.org/Subset/addressAdditionalLineText
:addressAdditionalLineText rdf:type owl:ObjectProperty ;
                           rdfs:domain :Address ;
                           rdfs:range :MISMOString ;
                           rdfs:comment "Address information that cannot be contained in the Address Line Text."^^xsd:string ;
                           rdfs:label "Address Additional Line Text"^^xsd:string .


###  http://mismo.org/Subset/addressAdditionalLineTwoText
:addressAdditionalLineTwoText rdf:type owl:ObjectProperty ;
                              rdfs:domain :Address ;
                              rdfs:range :MISMOString ;
                              rdfs:comment "A free-form alphanumeric string which contains a second additional line of Address information."^^xsd:string ;
                              rdfs:label "Address Additional Line Two Text"^^xsd:string .


###  http://mismo.org/Subset/addressCondominiumApartmentText
:addressCondominiumApartmentText rdf:type owl:ObjectProperty ;
                                 rdfs:domain :Address ;
                                 rdfs:range :MISMOString ;
                                 rdfs:comment "A free-form alphanumeric string that describes the apartment or condominium component of a specific address."^^xsd:string ;
                                 rdfs:label "Address Condominium Apartment Text"^^xsd:string .


###  http://mismo.org/Subset/addressFormatType
:addressFormatType rdf:type owl:ObjectProperty ;
                   rdfs:domain :Address ;
                   rdfs:range <http://mismo.org/EnumeratedTypes/AddressFormatEnum> ;
                   rdfs:comment "A collection of values that specify an address format as defined by the USPS Publication 28 Appendix A2 Address Types."^^xsd:string ;
                   rdfs:label "Address Format Type"^^xsd:string .


###  http://mismo.org/Subset/addressFormatTypeOtherDescription
:addressFormatTypeOtherDescription rdf:type owl:ObjectProperty ;
                                   rdfs:domain :Address ;
                                   rdfs:range :MISMOString ;
                                   rdfs:comment "A free-form text field that specifies the enumeration when the value of Other is used for the Address Format Type."^^xsd:string ;
                                   rdfs:label "Address Format Type Other Description"^^xsd:string .


###  http://mismo.org/Subset/addressIsNotUSPS-CodableIndicator
:addressIsNotUSPS-CodableIndicator rdf:type owl:ObjectProperty ;
                                   rdfs:domain :Address ;
                                   rdfs:range :MISMOIndicator ;
                                   rdfs:comment "When true, indicates the given Address is not formatted according to USPS standards or on the USPS master file."^^xsd:string ;
                                   rdfs:label "Address Is Not USPS Codable Indicator"^^xsd:string .


###  http://mismo.org/Subset/addressLineText
:addressLineText rdf:type owl:ObjectProperty ;
                 rdfs:domain :Address ;
                 rdfs:range :MISMOString ;
                 rdfs:comment "The address with the address number, pre-directional, street name, post-directional, address unit designators and address unit value."^^xsd:string ;
                 rdfs:label "Address Line Text"^^xsd:string .


###  http://mismo.org/Subset/addressPR-UrbanizationText
:addressPR-UrbanizationText rdf:type owl:ObjectProperty ;
                            rdfs:domain :Address ;
                            rdfs:range :MISMOString ;
                            rdfs:comment "A free-form alphanumeric string that describes the urbanization component of a specific address. Urbanization denotes an area, sector, or development within a geographic area. Often precededby \"URB\" in the address,it is commonly used in urban areas of Puerto Rico, and is an important part of the addressing format, as it describes the location of a given street."^^xsd:string ;
                            rdfs:label "Address PR Urbanization Text"^^xsd:string .


###  http://mismo.org/Subset/addressType
:addressType rdf:type owl:ObjectProperty ;
             rdfs:domain :Address ;
             rdfs:range <http://mismo.org/EnumeratedTypes/AddressEnum> ;
             rdfs:comment "A value from a MISMO prescribed list that specifies the type of address."^^xsd:string ;
             rdfs:label "Address Type"^^xsd:string .


###  http://mismo.org/Subset/addressTypeOtherDescription
:addressTypeOtherDescription rdf:type owl:ObjectProperty ;
                             rdfs:domain :Address ;
                             rdfs:range :MISMOString ;
                             rdfs:comment "A free-form text field used to collect additional information when Other is selected for Address Type."^^xsd:string ;
                             rdfs:label "Address Type Other Description"^^xsd:string .


###  http://mismo.org/Subset/addressUnitDesignatorType
:addressUnitDesignatorType rdf:type owl:ObjectProperty ;
                           rdfs:domain :Address ;
                           rdfs:range <http://mismo.org/EnumeratedTypes/AddressUnitDesignatorEnum> ;
                           rdfs:comment "A value from a MISMO prescribed list that specifies a further level of detail for a street address, for example, Suite or Unit. This list is based on the USPS Publication 28 on Postal Addressing Standards."^^xsd:string ;
                           rdfs:label "Address Unit Designator Type"^^xsd:string .


###  http://mismo.org/Subset/addressUnitDesignatorTypeOtherDescription
:addressUnitDesignatorTypeOtherDescription rdf:type owl:ObjectProperty ;
                                           rdfs:domain :Address ;
                                           rdfs:range :MISMOString ;
                                           rdfs:comment "The description of the Address Unit Designator Type when Other is selected as the option from the enumerated list."^^xsd:string ;
                                           rdfs:label "Address Unit Designator Type Other Description"^^xsd:string .


###  http://mismo.org/Subset/addressUnitIdentifier
:addressUnitIdentifier rdf:type owl:ObjectProperty ;
                       rdfs:domain :Address ;
                       rdfs:range :MISMOIdentifier ;
                       rdfs:comment "The identifier value associated with the Secondary Address Unit Designator. Example: 123, C, B1C, etc."^^xsd:string ;
                       rdfs:label "Address Unit Identifier"^^xsd:string .


###  http://mismo.org/Subset/adjustment
:adjustment rdf:type owl:ObjectProperty ;
            rdfs:domain :Loan ;
            rdfs:range <http://mismo.org/Containers/Adjustment> ;
            rdfs:comment "Data specific to the rules for adjustments and conversions to the interest rate and principal and interest payment for the life of the loan as specified in the Note. Includes provisions to capture the modifications to interest rate and principal and interest payment for each adjustment occurrence period. Also specifies the Rules for selecting the appropriate Index upon which the adjustments may be based."^^xsd:string .


###  http://mismo.org/Subset/affordableLending
:affordableLending rdf:type owl:ObjectProperty ;
                   rdfs:domain :Loan ;
                   rdfs:range <http://mismo.org/Containers/AffordableLending> ;
                   rdfs:comment "Contains information related to mortgage loan products that are affordable by low- to moderate-income homebuyers or buyers in high-cost or underserved communities."^^xsd:string ;
                   rdfs:label "affordable lending"^^xsd:string .


###  http://mismo.org/Subset/affordableLoanTotalSubordinateFinancingAmount
:affordableLoanTotalSubordinateFinancingAmount rdf:type owl:ObjectProperty ;
                                               rdfs:domain :Loan ;
                                               rdfs:range :MISMOAmount ;
                                               rdfs:comment "The total amount of subordinate financing associated with an affordable loan program."^^xsd:string ;
                                               rdfs:label "Affordable Loan Total Subordinate Financing Amount"^^xsd:string .


###  http://mismo.org/Subset/affordableUnitsCount
:affordableUnitsCount rdf:type owl:ObjectProperty ;
                      rdfs:domain :Property ;
                      rdfs:range <http://mismo.org/DataTypes/MISMOCount> ;
                      rdfs:comment "The number of individual dwelling units related to the property securing the loan or, in the case of an application, proposed to secure the loan that are income-restricted pursuant to Federal, State, or local affordable housing programs."^^xsd:string ;
                      rdfs:label "Affordable Units Count"^^xsd:string .


###  http://mismo.org/Subset/amortization
:amortization rdf:type owl:ObjectProperty ;
              rdfs:domain :Loan ;
              rdfs:range <http://mismo.org/Containers/Amortization> ;
              rdfs:comment "Information about the payments of principal and interest on a loan that reduce the current balance of the loan."^^xsd:string .


###  http://mismo.org/Subset/amortizationType
:amortizationType rdf:type owl:ObjectProperty ;
                  rdfs:domain :Pool ;
                  rdfs:range <http://mismo.org/EnumeratedTypes/AmortizationEnum> ;
                  rdfs:comment "A classification or description of a loan or a group of loans generally based on the changeability of the rate or payment over time."^^xsd:string ;
                  rdfs:label "Amortization Type"^^xsd:string .


###  http://mismo.org/Subset/amortizationTypeOtherDescription
:amortizationTypeOtherDescription rdf:type owl:ObjectProperty ;
                                  rdfs:domain :Pool ;
                                  rdfs:range :MISMOString ;
                                  rdfs:comment "A free-form text field used to collect additional information or a description of the amortization type when Other is selected."^^xsd:string ;
                                  rdfs:label "Amortization Type Other Description"^^xsd:string .


###  http://mismo.org/Subset/applicationReceivedDate
:applicationReceivedDate rdf:type owl:ObjectProperty ;
                         rdfs:domain :Loan ;
                         rdfs:range :MISMODate ;
                         rdfs:comment "The date the creditor or originator received the application from the borrower for the subject mortgage loan."^^xsd:string ;
                         rdfs:label "Application Received Date"^^xsd:string .


###  http://mismo.org/Subset/armsLengthIndicator
:armsLengthIndicator rdf:type owl:ObjectProperty ;
                     rdfs:domain :Loan ;
                     rdfs:range :MISMOIndicator ;
                     rdfs:comment "Indicates that this is an arm's length transaction. An arm's length transaction is between a willing buyer and a willing seller with no undue influence on either party and there is no relationship between the parties except that of the specific transaction."^^xsd:string ;
                     rdfs:label "Arms Length Indicator"^^xsd:string .


###  http://mismo.org/Subset/assetSummary
:assetSummary rdf:type owl:ObjectProperty ;
              rdfs:domain :DealSequence ;
              rdfs:range <http://mismo.org/Containers/AssetSummary> ;
              rdfs:comment "Information regarding the type and totals of a defined group of assets."^^xsd:string ;
              rdfs:label "asset summary"^^xsd:string .


###  http://mismo.org/Subset/assets
:assets rdf:type owl:ObjectProperty ;
        rdfs:domain :DealSequence ;
        rdfs:range <http://mismo.org/Containers/Asset> ;
        rdfs:comment "A collection of assets that are used to determine credit worthiness of the parties."^^xsd:string .


###  http://mismo.org/Subset/assignmentOfRentsIndicator
:assignmentOfRentsIndicator rdf:type owl:ObjectProperty ;
                            rdfs:domain :Property ;
                            rdfs:range :MISMOIndicator ;
                            rdfs:comment "When true, indicates that a signed Assignment of Rents associated with the property is in effect."^^xsd:string ;
                            rdfs:label "Assignment Of Rents Indicator"^^xsd:string .


###  http://mismo.org/Subset/assumability
:assumability rdf:type owl:ObjectProperty ;
              rdfs:domain :Loan ;
              rdfs:range <http://mismo.org/Containers/Assumability> ;
              rdfs:comment "Information about the terms for transferring mortgage obligations from the current owner to a buyer."^^xsd:string .


###  http://mismo.org/Subset/assumabilityIndicator
:assumabilityIndicator rdf:type owl:ObjectProperty ;
                       rdfs:domain :Loan ;
                       rdfs:range :MISMOIndicator ;
                       rdfs:comment "Indicates whether the loan is assumable by another borrower."^^xsd:string ;
                       rdfs:label "Assumability Indicator"^^xsd:string .


###  http://mismo.org/Subset/assumedIndicator
:assumedIndicator rdf:type owl:ObjectProperty ;
                  rdfs:domain :Loan ;
                  rdfs:range :MISMOIndicator ;
                  rdfs:comment "When true, indicates that the loan has been assumed."^^xsd:string ;
                  rdfs:label "Assumed Indicator"^^xsd:string .


###  http://mismo.org/Subset/attachmentType
:attachmentType rdf:type owl:ObjectProperty ;
                rdfs:domain :Property ;
                rdfs:range <http://mismo.org/EnumeratedTypes/AttachmentEnum> ;
                rdfs:comment "A value from a MISMO prescribed list that specifies the type of physical attachment, if any, between the dwelling and adjacent dwellings."^^xsd:string ;
                rdfs:label "Attachment Type"^^xsd:string .


###  http://mismo.org/Subset/attentionToName
:attentionToName rdf:type owl:ObjectProperty ;
                 rdfs:domain :Address ;
                 rdfs:range :MISMOString ;
                 rdfs:comment "A label that identifies the person or department to whose attention the mailing is sent."^^xsd:string ;
                 rdfs:label "Attention To Name"^^xsd:string .


###  http://mismo.org/Subset/balloonGuaranteedRefinancingIndicator
:balloonGuaranteedRefinancingIndicator rdf:type owl:ObjectProperty ;
                                       rdfs:domain :Loan ;
                                       rdfs:range :MISMOIndicator ;
                                       rdfs:comment "When true, indicates refinancing of the balloon mortgage loan is guaranteed by the lender."^^xsd:string ;
                                       rdfs:label "Balloon Guaranteed Refinancing Indicator"^^xsd:string .


###  http://mismo.org/Subset/balloonIndicator
:balloonIndicator rdf:type owl:ObjectProperty ;
                  rdfs:domain :Loan ;
                  rdfs:range :MISMOIndicator ;
                  rdfs:comment "When true, indicates that a final balloon payment is required to fully pay off the loan."^^xsd:string ;
                  rdfs:label "Balloon Indicator"^^xsd:string .


###  http://mismo.org/Subset/balloonPaymentAmount
:balloonPaymentAmount rdf:type owl:ObjectProperty ;
                      rdfs:domain :Loan ;
                      rdfs:range :MISMOAmount ;
                      rdfs:comment "The dollar amount of the final, or lump sum, balloon payment."^^xsd:string ;
                      rdfs:label "Balloon Payment Amount"^^xsd:string .


###  http://mismo.org/Subset/balloonPaymentMaximumAmount
:balloonPaymentMaximumAmount rdf:type owl:ObjectProperty ;
                             rdfs:domain :Loan ;
                             rdfs:range :MISMOAmount ;
                             rdfs:comment "The largest scheduled lump sum payment over the life of loan. This applies when there are scheduled lump sum payments that are more than twice as large as the average of earlier scheduled payments."^^xsd:string ;
                             rdfs:label "Balloon Payment Maximum Amount"^^xsd:string .


###  http://mismo.org/Subset/balloonPaymentMinimumAmount
:balloonPaymentMinimumAmount rdf:type owl:ObjectProperty ;
                             rdfs:domain :Loan ;
                             rdfs:range :MISMOAmount ;
                             rdfs:comment "The smallest scheduled lump sum payment over the life of loan. This applies when there are scheduled lump sum payments that are more than twice as large as the average of earlier scheduled payments."^^xsd:string ;
                             rdfs:label "Balloon Payment Minimum Amount"^^xsd:string .


###  http://mismo.org/Subset/balloonResetIndicator
:balloonResetIndicator rdf:type owl:ObjectProperty ;
                       rdfs:domain :Loan ;
                       rdfs:range :MISMOIndicator ;
                       rdfs:comment "When true, indicates that the balloon loan has been reset to the current market rate."^^xsd:string ;
                       rdfs:label "Balloon Reset Indicator"^^xsd:string .


###  http://mismo.org/Subset/balloonResetOptionIndicator
:balloonResetOptionIndicator rdf:type owl:ObjectProperty ;
                             rdfs:domain :Loan ;
                             rdfs:range :MISMOIndicator ;
                             rdfs:comment "When true, indicates the balloon loan has an option to reset."^^xsd:string ;
                             rdfs:label "Balloon Reset Option Indicator"^^xsd:string .


###  http://mismo.org/Subset/baseFloodElevationLinearMeasure
:baseFloodElevationLinearMeasure rdf:type owl:ObjectProperty ;
                                 rdfs:domain :FloodRiskFactor ;
                                 rdfs:range <http://mismo.org/DataTypes/MISMOLinearMeasure> ;
                                 rdfs:comment "A measurement that specifies the elevation of flood water in relation to sea level at its highest point for a property. The applicable unit of measurement is specified by the Linear Unit Of Measure Type."^^xsd:string ;
                                 rdfs:label "Base Flood Elevation Linear Measure"^^xsd:string .


###  http://mismo.org/Subset/belowMarketSubordinateFinancingIndicator
:belowMarketSubordinateFinancingIndicator rdf:type owl:ObjectProperty ;
                                          rdfs:domain :Loan ;
                                          rdfs:range :MISMOIndicator ;
                                          rdfs:comment "Indicates whether the seller provided below-market subordinate financing."^^xsd:string ;
                                          rdfs:label "Below Market Subordinate Financing Indicator"^^xsd:string .


###  http://mismo.org/Subset/billingAddress
:billingAddress rdf:type owl:ObjectProperty ;
                rdfs:domain :Loan ;
                rdfs:range <http://mismo.org/Containers/BillingAddress> ;
                rdfs:comment "The address data to be used for sending invoices to a legal entity."^^xsd:string ;
                rdfs:label "billing address"^^xsd:string .


###  http://mismo.org/Subset/biweeklyToMonthlyOnDefaultIndicator
:biweeklyToMonthlyOnDefaultIndicator rdf:type owl:ObjectProperty ;
                                     rdfs:domain :Loan ;
                                     rdfs:range :MISMOIndicator ;
                                     rdfs:comment "Indicates if the lender allows conversion from Bi-weekly payments to monthly upon a default by the borrower."^^xsd:string ;
                                     rdfs:label "Biweekly To Monthly On Default Indicator"^^xsd:string .


###  http://mismo.org/Subset/borrowerContinuesToOwnPropertyIndicator
:borrowerContinuesToOwnPropertyIndicator rdf:type owl:ObjectProperty ;
                                         rdfs:domain :Property ;
                                         rdfs:range :MISMOIndicator ;
                                         rdfs:comment "When true, indicates that the property associated with the loan is still owned by the borrower(s)."^^xsd:string ;
                                         rdfs:label "Borrower Continues To Own Property Indicator"^^xsd:string .


###  http://mismo.org/Subset/borrowerCount
:borrowerCount rdf:type owl:ObjectProperty ;
               rdfs:domain :Loan ;
               rdfs:range <http://mismo.org/DataTypes/MISMOCount> ;
               rdfs:comment "The number of borrowers obligated on the note."^^xsd:string ;
               rdfs:label "Borrower Count"^^xsd:string .


###  http://mismo.org/Subset/buildingCount
:buildingCount rdf:type owl:ObjectProperty ;
               rdfs:domain :Property ;
               rdfs:range <http://mismo.org/DataTypes/MISMOCount> ;
               rdfs:comment "The total number of detached buildings on the site."^^xsd:string ;
               rdfs:label "Building Count"^^xsd:string .


###  http://mismo.org/Subset/buildingPermits
:buildingPermits rdf:type owl:ObjectProperty ;
                 rdfs:domain :Property ;
                 rdfs:range <http://mismo.org/Containers/BuildingPermit> ;
                 rdfs:comment "Information regarding one or more types of permits. Holds all occurrences of BUILDING_PERMIT."^^xsd:string ;
                 rdfs:label "building permits"^^xsd:string .


###  http://mismo.org/Subset/buydown
:buydown rdf:type owl:ObjectProperty ;
         rdfs:domain :Loan ;
         rdfs:range <http://mismo.org/Containers/Buydown> ;
         rdfs:comment "Describes the provision, schedule, and structure of funds used to reduce the interest rate and/or payment on a mortgage note a temporary basis. A permanent buydown is covered by points paid at origination, see Borrower Paid Discount Points Total Amount."^^xsd:string .


###  http://mismo.org/Subset/buydownTemporarySubsidyFundingIndicator
:buydownTemporarySubsidyFundingIndicator rdf:type owl:ObjectProperty ;
                                         rdfs:domain :Loan ;
                                         rdfs:range :MISMOIndicator ;
                                         rdfs:comment "When true, indicates that there is buydown funding on this loan that reduces the interest rate and/or the payments for a specified period."^^xsd:string ;
                                         rdfs:label "Buydown Temporary Subsidy Funding Indicator"^^xsd:string .


###  http://mismo.org/Subset/capitalizationSummary
:capitalizationSummary rdf:type owl:ObjectProperty ;
                       rdfs:domain :Loan ;
                       rdfs:range <http://mismo.org/Containers/CapitalizationSummary> ;
                       rdfs:comment "Summarization of the capitalization items."^^xsd:string ;
                       rdfs:label "capitalization summary"^^xsd:string .


###  http://mismo.org/Subset/capitalizations
:capitalizations rdf:type owl:ObjectProperty ;
                 rdfs:domain :Loan ;
                 rdfs:range <http://mismo.org/Containers/Capitalization> ;
                 rdfs:comment "Information about one or more types of capitalization for a loan. Holds all occurrences of CAPITALIZATION."^^xsd:string .


###  http://mismo.org/Subset/capitalizedFeesIndicator
:capitalizedFeesIndicator rdf:type owl:ObjectProperty ;
                          rdfs:domain :Loan ;
                          rdfs:range :MISMOIndicator ;
                          rdfs:comment "Indicates that the mortgage balance includes capitalized origination fees."^^xsd:string ;
                          rdfs:label "Capitalized Fees Indicator"^^xsd:string .


###  http://mismo.org/Subset/capitalizedLoanIndicator
:capitalizedLoanIndicator rdf:type owl:ObjectProperty ;
                          rdfs:domain :Loan ;
                          rdfs:range :MISMOIndicator ;
                          rdfs:comment "Indicates that interest accrued, escrow disbursements made and/or fees charged are included in the unpaid principal balance."^^xsd:string ;
                          rdfs:label "Capitalized Loan Indicator"^^xsd:string .


###  http://mismo.org/Subset/carStorages
:carStorages rdf:type owl:ObjectProperty ;
             rdfs:domain :Property ;
             rdfs:range <http://mismo.org/Containers/CarStorage> ;
             rdfs:comment "Information about one or more types of car storage. Holds all occurrences of CAR_STORAGE."^^xsd:string ;
             rdfs:label "car storages"^^xsd:string .


###  http://mismo.org/Subset/carrierRouteCode
:carrierRouteCode rdf:type owl:ObjectProperty ;
                  rdfs:domain :Address ;
                  rdfs:range <http://mismo.org/DataTypes/MISMOCode> ;
                  rdfs:comment "A postal carrier route code is a part of the complete carrier route. The carrier route code is 4 characters consisting of 1 letter for the type of carrier route and 3 digits for the carrier route. The complete carrier route identifies a group of addresses to which the USPS assigns the same code to aid in mail delivery. The complete Carrier Route consists of 9 digits â 5 numbers for the ZIP Code and the 4 characters for the carrier route code."^^xsd:string ;
                  rdfs:label "Carrier Route Code"^^xsd:string .


###  http://mismo.org/Subset/cashRemittanceSummaryNotification
:cashRemittanceSummaryNotification rdf:type owl:ObjectProperty ;
                                   rdfs:domain :DealSet ;
                                   rdfs:range <http://mismo.org/Containers/CashRemittanceSummaryNotification> ;
                                   rdfs:comment "Container for summary cash remittances due to the Investor."^^xsd:string ;
                                   rdfs:label "cash remittance summary notification"^^xsd:string .


###  http://mismo.org/Subset/certificates
:certificates rdf:type owl:ObjectProperty ;
              rdfs:domain :Property ;
              rdfs:range <http://mismo.org/Containers/Certificate> ;
              rdfs:comment "Information regarding one or more types of certificate. Holds all occurrences of CERTIFICATE."^^xsd:string .


###  http://mismo.org/Subset/chargeOff
:chargeOff rdf:type owl:ObjectProperty ;
           rdfs:domain :Loan ;
           rdfs:range <http://mismo.org/Containers/ChargeOff> ;
           rdfs:comment "Information regarding identification, reason and total amounts charged off on the loan."^^xsd:string ;
           rdfs:label "charge off"^^xsd:string .


###  http://mismo.org/Subset/cityName
:cityName rdf:type owl:ObjectProperty ;
          rdfs:domain :Address ;
          rdfs:range :MISMOString ;
          rdfs:comment "The name of the city or Military APO FPO designation."^^xsd:string ;
          rdfs:label "City Name"^^xsd:string .


###  http://mismo.org/Subset/closingCostFinancedIndicator
:closingCostFinancedIndicator rdf:type owl:ObjectProperty ;
                              rdfs:domain :Loan ;
                              rdfs:range :MISMOIndicator ;
                              rdfs:comment "Indicates that some or all of the closing cost were financed into the loan amount."^^xsd:string ;
                              rdfs:label "Closing Cost Financed Indicator"^^xsd:string .


###  http://mismo.org/Subset/closingDisclosureWaitingPeriodWaivedIndicator
:closingDisclosureWaitingPeriodWaivedIndicator rdf:type owl:ObjectProperty ;
                                               rdfs:domain :Loan ;
                                               rdfs:range :MISMOIndicator ;
                                               rdfs:comment "When true, indicates that upon receipt of the Closing Disclosure, and due to a bona fide personal financial emergency, the consumer modified or waived the three-business-day waiting period that must be met prior to consummation of the mortgage loan transaction."^^xsd:string ;
                                               rdfs:label "Closing Disclosure Waiting Period Waived Indicator"^^xsd:string .


###  http://mismo.org/Subset/closingInformation
:closingInformation rdf:type owl:ObjectProperty ;
                    rdfs:domain :Loan ;
                    rdfs:range <http://mismo.org/Containers/ClosingInformation> ;
                    rdfs:comment "Information about the process to transfer of the legal title from the seller to the buyer."^^xsd:string ;
                    rdfs:label "closing information"^^xsd:string .


###  http://mismo.org/Subset/collateralPledgedToName
:collateralPledgedToName rdf:type owl:ObjectProperty ;
                         rdfs:domain :Loan ;
                         rdfs:range :MISMOString ;
                         rdfs:comment "Specifies to whom the loan has been pledged as collateral."^^xsd:string ;
                         rdfs:label "Collateral Pledged To Name"^^xsd:string .


###  http://mismo.org/Subset/collaterals
:collaterals rdf:type owl:ObjectProperty ;
             rdfs:domain :DealSequence ;
             rdfs:range <http://mismo.org/Containers/Collateral> ;
             rdfs:comment "A collection of assets that will be used as collateral for the loans of this deal or the collateral that has been used for collateral in this deal."^^xsd:string .


###  http://mismo.org/Subset/collections
:collections rdf:type owl:ObjectProperty ;
             rdfs:domain :Loan ;
             rdfs:range <http://mismo.org/Containers/Collection> ;
             rdfs:comment "Information about one or more types of collection efforts for a loan. Holds all occurrences of  COLLECTION."^^xsd:string .


###  http://mismo.org/Subset/combinedLtvs
:combinedLtvs rdf:type owl:ObjectProperty ;
              rdfs:domain [ rdf:type owl:Class ;
                            owl:unionOf ( :DealSequence
                                          :FloodResponse
                                        )
                          ] ;
              rdfs:range <http://mismo.org/Containers/CombinedLTV> ;
              rdfs:comment "Information about one or more COMBINED_LTV. Holds all occurrences of COMBINED_LTV."^^xsd:string ;
              rdfs:label "combined ltvs"^^xsd:string .


###  http://mismo.org/Subset/communicationEvents
:communicationEvents rdf:type owl:ObjectProperty ;
                     rdfs:domain :DealSequence ;
                     rdfs:range <http://mismo.org/Containers/CommunicationEvent> ;
                     rdfs:comment "Information regarding one or more events. Holds all occurrences of COMMUNICATION EVENT."^^xsd:string ;
                     rdfs:label "communication events"^^xsd:string .


###  http://mismo.org/Subset/communityLandTrustIndicator
:communityLandTrustIndicator rdf:type owl:ObjectProperty ;
                             rdfs:domain :Property ;
                             rdfs:range :MISMOIndicator ;
                             rdfs:comment "Indicates that the property is located in a community land trust."^^xsd:string ;
                             rdfs:label "Community Land Trust Indicator"^^xsd:string .


###  http://mismo.org/Subset/communityPropertyStateIndicator
:communityPropertyStateIndicator rdf:type owl:ObjectProperty ;
                                 rdfs:domain :Property ;
                                 rdfs:range :MISMOIndicator ;
                                 rdfs:comment "When true, indicates the property is located in a community property state."^^xsd:string ;
                                 rdfs:label "Community Property State Indicator"^^xsd:string .


###  http://mismo.org/Subset/communityReinvestmentActDelineatedCommunityIndicator
:communityReinvestmentActDelineatedCommunityIndicator rdf:type owl:ObjectProperty ;
                                                      rdfs:domain :Property ;
                                                      rdfs:range :MISMOIndicator ;
                                                      rdfs:comment "Indicates that the property is in an area defined by the Community Reinvestment Act."^^xsd:string ;
                                                      rdfs:label "Community Reinvestment Act Delineated Community Indicator"^^xsd:string .


###  http://mismo.org/Subset/comparable
:comparable rdf:type owl:ObjectProperty ;
            rdfs:domain :Property ;
            rdfs:range <http://mismo.org/Containers/Comparable> ;
            rdfs:comment "Information regarding the research, adjustments, summary conclusions and other facts about selections used in the sales comparison approach to value and in the context of grid style reporting."^^xsd:string .


###  http://mismo.org/Subset/concurrentOriginationIndicator
:concurrentOriginationIndicator rdf:type owl:ObjectProperty ;
                                rdfs:domain :Loan ;
                                rdfs:range :MISMOIndicator ;
                                rdfs:comment "Indicates that a new first mortgage will be closed concurrently with a second or a HELOC loan."^^xsd:string ;
                                rdfs:label "Concurrent Origination Indicator"^^xsd:string .


###  http://mismo.org/Subset/concurrentOriginationLenderIndicator
:concurrentOriginationLenderIndicator rdf:type owl:ObjectProperty ;
                                      rdfs:domain :Loan ;
                                      rdfs:range :MISMOIndicator ;
                                      rdfs:comment "Indicates that a concurrent loan is from the same lender. This is in conjunction with Concurrent Origination Indicator."^^xsd:string ;
                                      rdfs:label "Concurrent Origination Lender Indicator"^^xsd:string .


###  http://mismo.org/Subset/conformingIndicator
:conformingIndicator rdf:type owl:ObjectProperty ;
                     rdfs:domain :Loan ;
                     rdfs:range :MISMOIndicator ;
                     rdfs:comment "When true, indicates that the loan amount is a conforming loan amount by Fannie Mae and Freddie Mac standards."^^xsd:string ;
                     rdfs:label "Conforming Indicator"^^xsd:string .


###  http://mismo.org/Subset/construction
:construction rdf:type owl:ObjectProperty ;
              rdfs:domain :Loan ;
              rdfs:range <http://mismo.org/Containers/Construction> ;
              rdfs:comment "Information related to funds used for building of a structure or structures on a property."^^xsd:string .


###  http://mismo.org/Subset/constructionLoanIndicator
:constructionLoanIndicator rdf:type owl:ObjectProperty ;
                           rdfs:domain :Loan ;
                           rdfs:range :MISMOIndicator ;
                           rdfs:comment "When true, indicates that the loan is a construction loan."^^xsd:string ;
                           rdfs:label "Construction Loan Indicator"^^xsd:string .


###  http://mismo.org/Subset/constructionStatusType
:constructionStatusType rdf:type owl:ObjectProperty ;
                        rdfs:domain :Property ;
                        rdfs:range <http://mismo.org/EnumeratedTypes/ConstructionStatusEnum> ;
                        rdfs:comment "A value from a MISMO prescribed list that represents stage of construction at the time of the inspection."^^xsd:string ;
                        rdfs:label "Construction Status Type"^^xsd:string .


###  http://mismo.org/Subset/constructionStatusTypeOtherDescription
:constructionStatusTypeOtherDescription rdf:type owl:ObjectProperty ;
                                        rdfs:domain :Property ;
                                        rdfs:range :MISMOString ;
                                        rdfs:comment "A free-form text field used to collect additional information when Other is selected for Construction Status Type."^^xsd:string ;
                                        rdfs:label "Construction Status Type Other Description"^^xsd:string .


###  http://mismo.org/Subset/contractVariances
:contractVariances rdf:type owl:ObjectProperty ;
                   rdfs:domain :Loan ;
                   rdfs:range <http://mismo.org/Containers/ContractVariance> ;
                   rdfs:comment "Information about one or more types of contract variances associated with a LOAN. Contains all instances of CONTRACT_VARIANCE."^^xsd:string ;
                   rdfs:label "contract variances"^^xsd:string .


###  http://mismo.org/Subset/conversionOfContractForDeedIndicator
:conversionOfContractForDeedIndicator rdf:type owl:ObjectProperty ;
                                      rdfs:domain :Loan ;
                                      rdfs:range :MISMOIndicator ;
                                      rdfs:comment "When true, indicates that the subject transaction proceeds are used to pay off the remaining balance of the land contract (also known as a contract for deed)."^^xsd:string ;
                                      rdfs:label "Conversion Of Contract For Deed Indicator"^^xsd:string .


###  http://mismo.org/Subset/convertibleIndicator
:convertibleIndicator rdf:type owl:ObjectProperty ;
                      rdfs:domain :Loan ;
                      rdfs:range :MISMOIndicator ;
                      rdfs:comment "Indicates that the loan has a convertible characteristic."^^xsd:string ;
                      rdfs:label "Convertible Indicator"^^xsd:string .


###  http://mismo.org/Subset/cooperativeProprietaryLeaseExpirationDate
:cooperativeProprietaryLeaseExpirationDate rdf:type owl:ObjectProperty ;
                                           rdfs:domain :Property ;
                                           rdfs:range :MISMODate ;
                                           rdfs:comment "The expiration date of the lease agreement that gives a shareholder the right to occupy a particular dwelling unit."^^xsd:string ;
                                           rdfs:label "Cooperative Proprietary Lease Expiration Date"^^xsd:string .


###  http://mismo.org/Subset/correspondentAcquisitionType
:correspondentAcquisitionType rdf:type owl:ObjectProperty ;
                              rdfs:domain :Loan ;
                              rdfs:range <http://mismo.org/EnumeratedTypes/CorrespondentAcquisitionEnum> ;
                              rdfs:comment "A value from a MISMO prescribed list that specifies the method under which a loan was obtained from a correspondent lender by a security issuer."^^xsd:string ;
                              rdfs:label "Correspondent Acquisition Type"^^xsd:string .


###  http://mismo.org/Subset/correspondentAcquisitionTypeOtherDescription
:correspondentAcquisitionTypeOtherDescription rdf:type owl:ObjectProperty ;
                                              rdfs:domain :Loan ;
                                              rdfs:range :MISMOString ;
                                              rdfs:comment "A free-form text field that specifies the enumeration when the value of Other is used for Correspondent Acquisition Type."^^xsd:string ;
                                              rdfs:label "Correspondent Acquisition Type Other Description"^^xsd:string .


###  http://mismo.org/Subset/countryCode
:countryCode rdf:type owl:ObjectProperty ;
             rdfs:domain :Address ;
             rdfs:range <http://mismo.org/DataTypes/MISMOCode> ;
             rdfs:comment "The two-character representation of the country."^^xsd:string ;
             rdfs:label "Country Code"^^xsd:string .


###  http://mismo.org/Subset/countryName
:countryName rdf:type owl:ObjectProperty ;
             rdfs:domain :Address ;
             rdfs:range :MISMOString ;
             rdfs:comment "The name of the country."^^xsd:string ;
             rdfs:label "Country Name"^^xsd:string .


###  http://mismo.org/Subset/countyCode
:countyCode rdf:type owl:ObjectProperty ;
            rdfs:domain :Address ;
            rdfs:range <http://mismo.org/DataTypes/MISMOCode> ;
            rdfs:comment "Code identifying the county within a state. (Designator Code based on FIPS Publication 6-4)"^^xsd:string ;
            rdfs:label "County Code"^^xsd:string .


###  http://mismo.org/Subset/countyName
:countyName rdf:type owl:ObjectProperty ;
            rdfs:domain :Address ;
            rdfs:range :MISMOString ;
            rdfs:comment "An unstructured name that identifies the county within a state. (Designator Name based on FIPS Publication 6-4)."^^xsd:string ;
            rdfs:label "County Name"^^xsd:string .


###  http://mismo.org/Subset/creditEnhancementIndicator
:creditEnhancementIndicator rdf:type owl:ObjectProperty ;
                            rdfs:domain :Loan ;
                            rdfs:range :MISMOIndicator ;
                            rdfs:comment "When true, indicates that the loan has a credit enhancement."^^xsd:string ;
                            rdfs:label "Credit Enhancement Indicator"^^xsd:string .


###  http://mismo.org/Subset/creditEnhancements
:creditEnhancements rdf:type owl:ObjectProperty ;
                    rdfs:domain :Loan ;
                    rdfs:range <http://mismo.org/Containers/CreditEnhancement> ;
                    rdfs:comment "Information about one or more CREDIT_ENHANCEMENT. Holds all occurrences of CREDIT_ENHANCEMENT."^^xsd:string ;
                    rdfs:label "credit enhancements"^^xsd:string .


###  http://mismo.org/Subset/creditorServicingOfLoanStatementType
:creditorServicingOfLoanStatementType rdf:type owl:ObjectProperty ;
                                      rdfs:domain :Loan ;
                                      rdfs:range <http://mismo.org/EnumeratedTypes/CreditorServicingOfLoanStatementEnum> ;
                                      rdfs:comment "Specifies the certainty of the originating lender's or creditor's intention to service the mortgage loan."^^xsd:string ;
                                      rdfs:label "Creditor Servicing Of Loan Statement Type"^^xsd:string .


###  http://mismo.org/Subset/creditorServicingOfLoanStatementTypeOtherDescription
:creditorServicingOfLoanStatementTypeOtherDescription rdf:type owl:ObjectProperty ;
                                                      rdfs:domain :Loan ;
                                                      rdfs:range :MISMOString ;
                                                      rdfs:comment "A free-form text field used to capture additional information when Other is selected for Creditor Servicing Of Loan Statement Type."^^xsd:string ;
                                                      rdfs:label "Creditor Servicing Of Loan Statement Type Other Description"^^xsd:string .


###  http://mismo.org/Subset/currentInterestRatePercent
:currentInterestRatePercent rdf:type owl:ObjectProperty ;
                            rdfs:domain :Loan ;
                            rdfs:range <http://mismo.org/DataTypes/MISMOPercent> ;
                            rdfs:comment "The current interest rate, expressed as a percent, for this loan."^^xsd:string ;
                            rdfs:label "Current Interest Rate Percent"^^xsd:string .


###  http://mismo.org/Subset/cusip-Identifier
:cusip-Identifier rdf:type owl:ObjectProperty ;
                  rdfs:domain :Pool ;
                  rdfs:range :MISMOIdentifier ;
                  rdfs:comment "Unique identifier according to the standards set by Committee on Uniform Security Identification Practices. The CUSIP is registered with the SEC and the Federal Reserve."^^xsd:string ;
                  rdfs:label "CUSIP Identifier"^^xsd:string .


###  http://mismo.org/Subset/dataSources
:dataSources rdf:type owl:ObjectProperty ;
             rdfs:domain :Property ;
             rdfs:range <http://mismo.org/Containers/DataSource> ;
             rdfs:comment "Details about one or more information sources used for facts or references. Holds all occurrences of DATA_SOURCE."^^xsd:string ;
             rdfs:label "data sources"^^xsd:string .


###  http://mismo.org/Subset/dealChoice1
:dealChoice1 rdf:type owl:ObjectProperty ;
             rdfs:domain :Deal ;
             rdfs:range :DealChoice ;
             rdfs:label "deal choice 1"^^xsd:string .


###  http://mismo.org/Subset/dealComments
:dealComments rdf:type owl:ObjectProperty ;
              rdfs:domain :DealSequence ;
              rdfs:range <http://mismo.org/Containers/DealComment> ;
              rdfs:comment "Information about one or more DEAL_COMMENT. Holds all occurrences of DEAL_COMMENT."^^xsd:string ;
              rdfs:label "deal comments"^^xsd:string .


###  http://mismo.org/Subset/dealSequence1
:dealSequence1 rdf:type owl:ObjectProperty ;
               rdfs:domain :DealChoice ;
               rdfs:range :DealSequence ;
               rdfs:label "deal sequence 1"^^xsd:string .


###  http://mismo.org/Subset/dealSetExpenses
:dealSetExpenses rdf:type owl:ObjectProperty ;
                 rdfs:domain :DealSet ;
                 rdfs:range <http://mismo.org/Containers/DealSetExpense> ;
                 rdfs:comment "Information about one or more types of expense associated with a DEAL_SET. Holds all occurrences of DEAL_SET_EXPENSE."^^xsd:string ;
                 rdfs:label "deal set expenses"^^xsd:string .


###  http://mismo.org/Subset/dealSetIncomes
:dealSetIncomes rdf:type owl:ObjectProperty ;
                rdfs:domain :DealSet ;
                rdfs:range <http://mismo.org/Containers/DealSetIncome> ;
                rdfs:comment "Information about one or more types of income associated with a DEAL_SET. Holds all occurrences of DEAL_SET_INCOMES."^^xsd:string ;
                rdfs:label "deal set incomes"^^xsd:string .


###  http://mismo.org/Subset/deals
:deals rdf:type owl:ObjectProperty ;
       rdfs:domain :DealSet ;
       rdfs:range :Deal ;
       rdfs:comment "The root element for all use cases where a collection of loans need to be delivered."^^xsd:string .


###  http://mismo.org/Subset/deedRestrictionIndicator
:deedRestrictionIndicator rdf:type owl:ObjectProperty ;
                          rdfs:domain :Property ;
                          rdfs:range :MISMOIndicator ;
                          rdfs:comment "If true, indicates that the deed has associated restrictions."^^xsd:string ;
                          rdfs:label "Deed Restriction Indicator"^^xsd:string .


###  http://mismo.org/Subset/deferredInterestBalanceAmount
:deferredInterestBalanceAmount rdf:type owl:ObjectProperty ;
                               rdfs:domain :Loan ;
                               rdfs:range :MISMOAmount ;
                               rdfs:comment "Accrued Uncollected Interest."^^xsd:string ;
                               rdfs:label "Deferred Interest Balance Amount"^^xsd:string .


###  http://mismo.org/Subset/delegatedUnderwritingIndicator
:delegatedUnderwritingIndicator rdf:type owl:ObjectProperty ;
                                rdfs:domain :Loan ;
                                rdfs:range :MISMOIndicator ;
                                rdfs:comment "When true, indicates that the underwriting authority on a loan is delegated to the loan originator based on disclosed guidelines."^^xsd:string ;
                                rdfs:label "Delegated Underwriting Indicator"^^xsd:string .


###  http://mismo.org/Subset/deliveryPointBarCodeCheckValue
:deliveryPointBarCodeCheckValue rdf:type owl:ObjectProperty ;
                                rdfs:domain :Address ;
                                rdfs:range <http://mismo.org/DataTypes/MISMOValue> ;
                                rdfs:comment "A check digit calculated using the MOD 10 method on the total of all 10 digits that make up the bar code for use in the Delivery Point Bar Code (DPBC). The DPBC is an 11 digit (plus check digit) barcode, containing the ZIP Code, ZIP+4 Code, and the delivery point code. This is the predominant barcode in use currently (as of 2008), and it enables the Postal Service to sort mail into delivery point (address) sequence."^^xsd:string ;
                                rdfs:label "Delivery Point Bar Code Check Value"^^xsd:string .


###  http://mismo.org/Subset/deliveryPointBarCodeValue
:deliveryPointBarCodeValue rdf:type owl:ObjectProperty ;
                           rdfs:domain :Address ;
                           rdfs:range <http://mismo.org/DataTypes/MISMOValue> ;
                           rdfs:comment "A code maintained by the USPS representing a delivery point (DP) which is a single mailbox or other place at which mail is delivered. This may be appended to the combination of zip code and zip+4 code for the purposes of creating a barcode."^^xsd:string ;
                           rdfs:label "Delivery Point Bar Code Value"^^xsd:string .


###  http://mismo.org/Subset/demandFeatureIndicator
:demandFeatureIndicator rdf:type owl:ObjectProperty ;
                        rdfs:domain :Loan ;
                        rdfs:range :MISMOIndicator ;
                        rdfs:comment "When true, indicates that the loan has a demand feature."^^xsd:string ;
                        rdfs:label "Demand Feature Indicator"^^xsd:string .


###  http://mismo.org/Subset/disasterForbearances
:disasterForbearances rdf:type owl:ObjectProperty ;
                      rdfs:domain :Loan ;
                      rdfs:range <http://mismo.org/Containers/DisasterForbearance> ;
                      rdfs:comment "Information about one or more disaster forbearance events or payment suspensions. Holds all occurrences of DISASTER_FORBEARANCE."^^xsd:string ;
                      rdfs:label "disaster forbearances"^^xsd:string .


###  http://mismo.org/Subset/disasterIndicator
:disasterIndicator rdf:type owl:ObjectProperty ;
                   rdfs:domain :Property ;
                   rdfs:range :MISMOIndicator ;
                   rdfs:comment "Indicates that the property is damaged as a result of a natural disaster, such as a hurricane, tornado, or earthquake."^^xsd:string ;
                   rdfs:label "Disaster Indicator"^^xsd:string .


###  http://mismo.org/Subset/disasterMitigationFeatures
:disasterMitigationFeatures rdf:type owl:ObjectProperty ;
                            rdfs:domain :Property ;
                            rdfs:range <http://mismo.org/Containers/DisasterMitigationFeature> ;
                            rdfs:comment "Information about one or more DISASTER_MITIGATION_FEATURE. Contains all instances of DISASTER_MITIGATION_FEATURE."^^xsd:string ;
                            rdfs:label "disaster mitigation features"^^xsd:string .


###  http://mismo.org/Subset/disasters
:disasters rdf:type owl:ObjectProperty ;
           rdfs:domain :Property ;
           rdfs:range <http://mismo.org/Containers/Disaster> ;
           rdfs:comment "Information about one or more disasters that have affected the property. Holds all occurrences of DISASTER."^^xsd:string .


###  http://mismo.org/Subset/disclosures
:disclosures rdf:type owl:ObjectProperty ;
             rdfs:domain :Loan ;
             rdfs:range <http://mismo.org/Containers/Disclosure> ;
             rdfs:comment "Information about one or more types of disclosure. Holds all occurrences of DISCLOSURE."^^xsd:string .


###  http://mismo.org/Subset/disputeResolutionIndicator
:disputeResolutionIndicator rdf:type owl:ObjectProperty ;
                            rdfs:domain :FloodResponse ;
                            rdfs:range :MISMOIndicator ;
                            rdfs:comment "Indicates that the response is a result of a dispute."^^xsd:string ;
                            rdfs:label "Dispute Resolution Indicator"^^xsd:string .


###  http://mismo.org/Subset/documentSpecificDataSets
:documentSpecificDataSets rdf:type owl:ObjectProperty ;
                          rdfs:domain :Loan ;
                          rdfs:range <http://mismo.org/Containers/DocumentSpecificDataSet> ;
                          rdfs:comment "Data that is not used for anything else except for document preparation AND does not fit well anywhere else under DEAL."^^xsd:string ;
                          rdfs:label "document specific data sets"^^xsd:string .


###  http://mismo.org/Subset/documentations
:documentations rdf:type owl:ObjectProperty ;
                rdfs:domain :Loan ;
                rdfs:range <http://mismo.org/Containers/Documentation> ;
                rdfs:comment "Information about one or more DOCUMENTATION. Holds all occurrences of DOCUMENTATION."^^xsd:string .


###  http://mismo.org/Subset/downPayments
:downPayments rdf:type owl:ObjectProperty ;
              rdfs:domain :Loan ;
              rdfs:range <http://mismo.org/Containers/DownPayment> ;
              rdfs:comment "Information about one or more DOWN_PAYMENT. Holds all occurrences of DOWN_PAYMENT."^^xsd:string ;
              rdfs:label "down payments"^^xsd:string .


###  http://mismo.org/Subset/draw
:draw rdf:type owl:ObjectProperty ;
      rdfs:domain :Loan ;
      rdfs:range <http://mismo.org/Containers/Draw> ;
      rdfs:comment "Information on the disbursement of a portion of the loan proceeds to the borrower. This container would be used for a loan with a line of credit or a construction loan."^^xsd:string .


###  http://mismo.org/Subset/dwellingCount
:dwellingCount rdf:type owl:ObjectProperty ;
               rdfs:domain :Property ;
               rdfs:range <http://mismo.org/DataTypes/MISMOCount> ;
               rdfs:comment "The total number of structures on the property, excluding outbuildings, that contains a living unit."^^xsd:string ;
               rdfs:label "Dwelling Count"^^xsd:string .


###  http://mismo.org/Subset/eligibleForLenderPaidMI-Indicator
:eligibleForLenderPaidMI-Indicator rdf:type owl:ObjectProperty ;
                                   rdfs:domain :Loan ;
                                   rdfs:range :MISMOIndicator ;
                                   rdfs:comment "Indicates that the mortgage loan is eligible for lender-paid MI."^^xsd:string ;
                                   rdfs:label "Eligible For Lender Paid MI Indicator"^^xsd:string .


###  http://mismo.org/Subset/employeeLoanProgramIndicator
:employeeLoanProgramIndicator rdf:type owl:ObjectProperty ;
                              rdfs:domain :Loan ;
                              rdfs:range :MISMOIndicator ;
                              rdfs:comment "Indicates if the loan is part of an employee loan program."^^xsd:string ;
                              rdfs:label "Employee Loan Program Indicator"^^xsd:string .


###  http://mismo.org/Subset/encumbrances
:encumbrances rdf:type owl:ObjectProperty ;
              rdfs:domain :Property ;
              rdfs:range <http://mismo.org/Containers/Encumbrance> ;
              rdfs:comment "Information about one or more types of encumbrance. Holds all occurrences of ENCUMBRANCE."^^xsd:string .


###  http://mismo.org/Subset/energyEfficiencyAndGreen
:energyEfficiencyAndGreen rdf:type owl:ObjectProperty ;
                          rdfs:domain :Property ;
                          rdfs:range <http://mismo.org/Containers/EnergyEfficiencyAndGreen> ;
                          rdfs:comment "Contains information about the property's energy efficiency and green features, certifications, ratings and/or equipment."^^xsd:string ;
                          rdfs:label "energy efficiency and green"^^xsd:string .


###  http://mismo.org/Subset/energyRelatedImprovementsIndicator
:energyRelatedImprovementsIndicator rdf:type owl:ObjectProperty ;
                                    rdfs:domain :Loan ;
                                    rdfs:range :MISMOIndicator ;
                                    rdfs:comment "When true, indicates that the loan will include an amount for energy-related improvements."^^xsd:string ;
                                    rdfs:label "Energy Related Improvements Indicator"^^xsd:string .


###  http://mismo.org/Subset/enoteCertifiedIndicator
:enoteCertifiedIndicator rdf:type owl:ObjectProperty ;
                         rdfs:domain :Loan ;
                         rdfs:range :MISMOIndicator ;
                         rdfs:comment "Indicates whether the loan delivery data has been automatically certified against eNote data."^^xsd:string ;
                         rdfs:label "ENote Certified Indicator"^^xsd:string .


###  http://mismo.org/Subset/enoteIndicator
:enoteIndicator rdf:type owl:ObjectProperty ;
                rdfs:domain :Loan ;
                rdfs:range :MISMOIndicator ;
                rdfs:comment "Indicates that an eNote is used as part of this loan."^^xsd:string ;
                rdfs:label "ENote Indicator"^^xsd:string .


###  http://mismo.org/Subset/environmentalConditions
:environmentalConditions rdf:type owl:ObjectProperty ;
                         rdfs:domain :Property ;
                         rdfs:range <http://mismo.org/Containers/EnvironmentalCondition> ;
                         rdfs:comment "Information regarding one or more types of property environmental considerations. Holds all occurrences of ENVIRONMENTAL CONSIDERATION."^^xsd:string ;
                         rdfs:label "environmental conditions"^^xsd:string .


###  http://mismo.org/Subset/escrow
:escrow rdf:type owl:ObjectProperty ;
        rdfs:domain :Loan ;
        rdfs:range <http://mismo.org/Containers/Escrow> ;
        rdfs:comment "Information specific to funds collected through the loan payment and held to pay expenses such as taxes and insurance or funds held back after closing that are to be used for property improvements or repairs."^^xsd:string .


###  http://mismo.org/Subset/escrowAbsenceReasonType
:escrowAbsenceReasonType rdf:type owl:ObjectProperty ;
                         rdfs:domain :Loan ;
                         rdfs:range <http://mismo.org/EnumeratedTypes/EscrowAbsenceReasonEnum> ;
                         rdfs:comment "Specifies the reason the loan does not have an escrow account."^^xsd:string ;
                         rdfs:label "Escrow Absence Reason Type"^^xsd:string .


###  http://mismo.org/Subset/escrowAbsenceReasonTypeOtherDescription
:escrowAbsenceReasonTypeOtherDescription rdf:type owl:ObjectProperty ;
                                         rdfs:domain :Loan ;
                                         rdfs:range :MISMOString ;
                                         rdfs:comment "A free-form text field used to collect additional information when Other is selected for Escrow Absence Reason Type."^^xsd:string ;
                                         rdfs:label "Escrow Absence Reason Type Other Description"^^xsd:string .


###  http://mismo.org/Subset/escrowAccountLenderRequirementType
:escrowAccountLenderRequirementType rdf:type owl:ObjectProperty ;
                                    rdfs:domain :Loan ;
                                    rdfs:range <http://mismo.org/EnumeratedTypes/EscrowAccountLenderRequirementEnum> ;
                                    rdfs:comment "Identifies the escrow account status in terms of the requirements of the lender in the mortgage loan transaction."^^xsd:string ;
                                    rdfs:label "Escrow Account Lender Requirement Type"^^xsd:string .


###  http://mismo.org/Subset/escrowAccountRequestedIndicator
:escrowAccountRequestedIndicator rdf:type owl:ObjectProperty ;
                                 rdfs:domain :Loan ;
                                 rdfs:range :MISMOIndicator ;
                                 rdfs:comment "When true, indicates that the establishment of an escrow account has been requested by the borrower(s) for the loan."^^xsd:string ;
                                 rdfs:label "Escrow Account Requested Indicator"^^xsd:string .


###  http://mismo.org/Subset/escrowIndicator
:escrowIndicator rdf:type owl:ObjectProperty ;
                 rdfs:domain :Loan ;
                 rdfs:range :MISMOIndicator ;
                 rdfs:comment "Indicates whether or not escrows are associated with this loan."^^xsd:string ;
                 rdfs:label "Escrow Indicator"^^xsd:string .


###  http://mismo.org/Subset/escrowNotAllowedIndicator
:escrowNotAllowedIndicator rdf:type owl:ObjectProperty ;
                           rdfs:domain :Loan ;
                           rdfs:range :MISMOIndicator ;
                           rdfs:comment "When true, indicates that, under applicable law, a servicer may not establish an escrow account for the mortgage loan being modified."^^xsd:string ;
                           rdfs:label "Escrow Not Allowed Indicator"^^xsd:string .


###  http://mismo.org/Subset/escrowsElectedByBorrowerIndicator
:escrowsElectedByBorrowerIndicator rdf:type owl:ObjectProperty ;
                                   rdfs:domain :Loan ;
                                   rdfs:range :MISMOIndicator ;
                                   rdfs:comment "When true, indicates the borrower has elected to establish an escrow account."^^xsd:string ;
                                   rdfs:label "Escrows Elected By Borrower Indicator"^^xsd:string .


###  http://mismo.org/Subset/expenses
:expenses rdf:type owl:ObjectProperty ;
          rdfs:domain :DealSequence ;
          rdfs:range <http://mismo.org/Containers/Expense> ;
          rdfs:comment "Information about one or more EXPENSE. Holds all occurrences of EXPENSE."^^xsd:string .


###  http://mismo.org/Subset/extension
:extension rdf:type owl:ObjectProperty ;
           rdfs:domain [ rdf:type owl:Class ;
                         owl:unionOf ( :Address
                                       :DealSequence
                                       :DealSet
                                       :FloodDetermination
                                       :FloodResponse
                                       :FloodRiskFactor
                                       :HazardInsurance
                                       :Loan
                                       :Pool
                                       :Property
                                     )
                       ] ;
           rdfs:range [ rdf:type owl:Class ;
                        owl:unionOf ( <http://mismo.org/Extensions/AddressExtension>
                                      <http://mismo.org/Extensions/DealExtension>
                                      <http://mismo.org/Extensions/DealSetExtension>
                                      <http://mismo.org/Extensions/FloodDeterminationExtension>
                                      <http://mismo.org/Extensions/FloodResponseExtension>
                                      <http://mismo.org/Extensions/FloodRiskFactorExtension>
                                      <http://mismo.org/Extensions/HazardInsuranceExtension>
                                      <http://mismo.org/Extensions/LoanExtension>
                                      <http://mismo.org/Extensions/PoolExtension>
                                      <http://mismo.org/Extensions/PropertyExtension>
                                    )
                      ] ;
           rdfs:comment "Information added in a specific implementation that is not part of the used reference model, but is a proprietary extension, or belongs to a forward MISMO reference model."^^xsd:string .


###  http://mismo.org/Subset/facilitateServicingREO-PurchaseIndicator
:facilitateServicingREO-PurchaseIndicator rdf:type owl:ObjectProperty ;
                                          rdfs:domain :DealSequence ;
                                          rdfs:range :MISMOIndicator ;
                                          rdfs:comment "When true, indicates that this loan or mortgage was made to facilitate the sale of a Servicing REO property."^^xsd:string ;
                                          rdfs:label "Facilitate Servicing REO Purchase Indicator"^^xsd:string .


###  http://mismo.org/Subset/feeInformation
:feeInformation rdf:type owl:ObjectProperty ;
                rdfs:domain :Loan ;
                rdfs:range <http://mismo.org/Containers/FeeInformation> ;
                rdfs:comment "Information concerning fees or costs paid or assessed during the origination, closing, or ongoing servicing of a loan."^^xsd:string ;
                rdfs:label "fee information"^^xsd:string .


###  http://mismo.org/Subset/fema-AdditionalLenderDescription
:fema-AdditionalLenderDescription rdf:type owl:ObjectProperty ;
                                  rdfs:domain :FloodResponse ;
                                  rdfs:range :MISMOString ;
                                  rdfs:comment "Additional information for the lender in Box 1 of the FEMA document."^^xsd:string ;
                                  rdfs:label "FEMA Additional Lender Description"^^xsd:string .


###  http://mismo.org/Subset/fha-SecondaryResidenceIndicator
:fha-SecondaryResidenceIndicator rdf:type owl:ObjectProperty ;
                                 rdfs:domain :Property ;
                                 rdfs:range :MISMOIndicator ;
                                 rdfs:comment "When true, indicates that the property usage falls under the FHA Secondary Residence policy and guidelines."^^xsd:string ;
                                 rdfs:label "FHA Secondary Residence Indicator"^^xsd:string .


###  http://mismo.org/Subset/financedUnitCount
:financedUnitCount rdf:type owl:ObjectProperty ;
                   rdfs:domain :Property ;
                   rdfs:range <http://mismo.org/DataTypes/MISMOCount> ;
                   rdfs:comment "The number of individual family dwelling units being financed in the subject property."^^xsd:string ;
                   rdfs:label "Financed Unit Count"^^xsd:string .


###  http://mismo.org/Subset/floodCertificationIdentifier
:floodCertificationIdentifier rdf:type owl:ObjectProperty ;
                              rdfs:domain :FloodDetermination ;
                              rdfs:range :MISMOIdentifier ;
                              rdfs:comment "The certification number assigned by the compliance company when an order is received from the submitting / requesting party."^^xsd:string ;
                              rdfs:label "Flood Certification Identifier"^^xsd:string .


###  http://mismo.org/Subset/floodContractFeeAmount
:floodContractFeeAmount rdf:type owl:ObjectProperty ;
                        rdfs:domain :HazardInsurance ;
                        rdfs:range <http://mismo.org/DataTypes/MISMOAmount> ;
                        rdfs:comment "The amount charged by the provider to obtain the Flood Contract associated with the subject property."^^xsd:string ;
                        rdfs:label "Flood Contract Fee Amount"^^xsd:string .


###  http://mismo.org/Subset/floodDepthLinearMeasure
:floodDepthLinearMeasure rdf:type owl:ObjectProperty ;
                         rdfs:domain :FloodRiskFactor ;
                         rdfs:range <http://mismo.org/DataTypes/MISMOLinearMeasure> ;
                         rdfs:comment "A measurement that specifies the depth of the flood water in relation to the ground for a particular property.The applicable unit of measurement is specified by the Linear Unit Of Measure Type."^^xsd:string ;
                         rdfs:label "Flood Depth Linear Measure"^^xsd:string .


###  http://mismo.org/Subset/floodDetermination
:floodDetermination rdf:type owl:ObjectProperty ;
                    rdfs:domain [ rdf:type owl:Class ;
                                  owl:unionOf ( :FloodResponse
                                                :Property
                                              )
                                ] ;
                    rdfs:range :FloodDetermination ;
                    rdfs:comment "Information specific to the Flood Zone Determination pursuant to the National Flood Insurance Program."^^xsd:string ;
                    rdfs:label "flood determination"^^xsd:string .


###  http://mismo.org/Subset/floodDeterminationLifeOfLoanIndicator
:floodDeterminationLifeOfLoanIndicator rdf:type owl:ObjectProperty ;
                                       rdfs:domain :FloodDetermination ;
                                       rdfs:range :MISMOIndicator ;
                                       rdfs:comment "Indicates if the flood contract with the compliance company is for the Life of the Loan."^^xsd:string ;
                                       rdfs:label "Flood Determination Life Of Loan Indicator"^^xsd:string .


###  http://mismo.org/Subset/floodDiscrepancyGrandfatheredIndicator
:floodDiscrepancyGrandfatheredIndicator rdf:type owl:ObjectProperty ;
                                        rdfs:domain :FloodDetermination ;
                                        rdfs:range :MISMOIndicator ;
                                        rdfs:comment "When true, indicates that a discrepancy between the property location flood zone and the policy flood zone is acceptable because the property location in which the flood zone code is grandfathered."^^xsd:string ;
                                        rdfs:label "Flood Discrepancy Grandfathered Indicator"^^xsd:string .


###  http://mismo.org/Subset/floodDiscrepancyIndicator
:floodDiscrepancyIndicator rdf:type owl:ObjectProperty ;
                           rdfs:domain :FloodDetermination ;
                           rdfs:range :MISMOIndicator ;
                           rdfs:comment "When true, indicates there is a discrepancy between the property location flood zone code and the flood zone specified in the loan's flood insurance policy."^^xsd:string ;
                           rdfs:label "Flood Discrepancy Indicator"^^xsd:string .


###  http://mismo.org/Subset/floodDiscrepancyResolvedIndicator
:floodDiscrepancyResolvedIndicator rdf:type owl:ObjectProperty ;
                                   rdfs:domain :FloodDetermination ;
                                   rdfs:range :MISMOIndicator ;
                                   rdfs:comment "When true, indicates there was a discrepancy between the property location flood zone code and the flood zone specified in the loan's flood insurance policy but the discrepancy has been resolved."^^xsd:string ;
                                   rdfs:label "Flood Discrepancy Resolved Indicator"^^xsd:string .


###  http://mismo.org/Subset/floodPartialIndicator
:floodPartialIndicator rdf:type owl:ObjectProperty ;
                       rdfs:domain :FloodDetermination ;
                       rdfs:range :MISMOIndicator ;
                       rdfs:comment "Indicates that a portion of the subject property is in an identified Special Flood Hazard Area (SFHA)."^^xsd:string ;
                       rdfs:label "Flood Partial Indicator"^^xsd:string .


###  http://mismo.org/Subset/floodProductCertifyDate
:floodProductCertifyDate rdf:type owl:ObjectProperty ;
                         rdfs:domain :FloodDetermination ;
                         rdfs:range :MISMODate ;
                         rdfs:comment "The date on which the flood determination was assessed by the certification provider."^^xsd:string ;
                         rdfs:label "Flood Product Certify Date"^^xsd:string .


###  http://mismo.org/Subset/floodRiskFactor
:floodRiskFactor rdf:type owl:ObjectProperty ;
                 rdfs:domain :FloodDetermination ;
                 rdfs:range :FloodRiskFactor ;
                 rdfs:comment "Information about Risk Factors used in Flood Determination."^^xsd:string ;
                 rdfs:label "flood risk factor"^^xsd:string .


###  http://mismo.org/Subset/floodTransactionIdentifier
:floodTransactionIdentifier rdf:type owl:ObjectProperty ;
                            rdfs:domain :FloodResponse ;
                            rdfs:range :MISMOIdentifier ;
                            rdfs:comment "A unique alphanumeric string identifying the flood transaction as assigned by the sender. This is typically returned by the sender in a resulting response."^^xsd:string ;
                            rdfs:label "Flood Transaction Identifier"^^xsd:string .


###  http://mismo.org/Subset/foreclosures
:foreclosures rdf:type owl:ObjectProperty ;
              rdfs:domain :Loan ;
              rdfs:range <http://mismo.org/Containers/Foreclosure> ;
              rdfs:comment "Information regarding foreclosure on a loan. Holds all occurrences of FORECLOSURE."^^xsd:string .


###  http://mismo.org/Subset/foreignObjects
:foreignObjects rdf:type owl:ObjectProperty ;
                rdfs:domain :DealSequence ;
                rdfs:range <http://mismo.org/Containers/ForeignObject> ;
                rdfs:comment "Information about one or more FOREIGN_OBJECT. Holds all occurrences of FOREIGN_OBJECT."^^xsd:string ;
                rdfs:label "foreign objects"^^xsd:string .


###  http://mismo.org/Subset/functionalIssueDescription
:functionalIssueDescription rdf:type owl:ObjectProperty ;
                            rdfs:domain :Property ;
                            rdfs:range :MISMOString ;
                            rdfs:comment "A free-form text field describing all apparent functional issues associated with the property."^^xsd:string ;
                            rdfs:label "Functional Issue Description"^^xsd:string .


###  http://mismo.org/Subset/functionalIssues
:functionalIssues rdf:type owl:ObjectProperty ;
                  rdfs:domain :Property ;
                  rdfs:range <http://mismo.org/Containers/FunctionalIssue> ;
                  rdfs:comment "Information about one or more FUNCTIONAL_ISSUE. Holds all occurrences of FUNCTIONAL_ISSUE."^^xsd:string ;
                  rdfs:label "functional issues"^^xsd:string .


###  http://mismo.org/Subset/governmentBondFinanceIndicator
:governmentBondFinanceIndicator rdf:type owl:ObjectProperty ;
                                rdfs:domain :Pool ;
                                rdfs:range :MISMOIndicator ;
                                rdfs:comment "Indicates that the pool is to back securities for use as collateral for a state or local housing bond financing program (BFP)."^^xsd:string ;
                                rdfs:label "Government Bond Finance Indicator"^^xsd:string .


###  http://mismo.org/Subset/governmentBondFinancingProgramType
:governmentBondFinancingProgramType rdf:type owl:ObjectProperty ;
                                    rdfs:domain :Pool ;
                                    rdfs:range <http://mismo.org/EnumeratedTypes/GovernmentBondFinancingProgramEnum> ;
                                    rdfs:comment "Type of state or local housing bond financing program (BFP)."^^xsd:string ;
                                    rdfs:label "Government Bond Financing Program Type"^^xsd:string .


###  http://mismo.org/Subset/governmentBondFinancingProgramTypeOtherDescription
:governmentBondFinancingProgramTypeOtherDescription rdf:type owl:ObjectProperty ;
                                                    rdfs:domain :Pool ;
                                                    rdfs:range :MISMOString ;
                                                    rdfs:comment "A free-form text field used to collect additional information or a description of the mortgage type when Other is selected for Government Bond Financing Program Type."^^xsd:string ;
                                                    rdfs:label "Government Bond Financing Program Type Other Description"^^xsd:string .


###  http://mismo.org/Subset/governmentLoan
:governmentLoan rdf:type owl:ObjectProperty ;
                rdfs:domain :Loan ;
                rdfs:range <http://mismo.org/Containers/GovernmentLoan> ;
                rdfs:comment "Information about government loan details specific to programs for HUD such as FHA and VA."^^xsd:string ;
                rdfs:label "government loan"^^xsd:string .


###  http://mismo.org/Subset/grossLivingAreaTotalAreaMeasure
:grossLivingAreaTotalAreaMeasure rdf:type owl:ObjectProperty ;
                                 rdfs:domain :Property ;
                                 rdfs:range <http://mismo.org/DataTypes/MISMOAreaMeasure> ;
                                 rdfs:comment "A measurement that specifies the total area of all habitable rooms above grade measured contiguously.The applicable unit of measurement is specified by the Area Unit Of Measure Type."^^xsd:string ;
                                 rdfs:label "Gross Living Area Total Area Measure"^^xsd:string .


###  http://mismo.org/Subset/groundRentIndicator
:groundRentIndicator rdf:type owl:ObjectProperty ;
                     rdfs:domain :Property ;
                     rdfs:range :MISMOIndicator ;
                     rdfs:comment "When true indicates the property's title is held in a leasehold estate for which ground rent is paid."^^xsd:string ;
                     rdfs:label "Ground Rent Indicator"^^xsd:string .


###  http://mismo.org/Subset/groupHomeIndicator
:groupHomeIndicator rdf:type owl:ObjectProperty ;
                    rdfs:domain :Property ;
                    rdfs:range :MISMOIndicator ;
                    rdfs:comment "When true, indicates the property will be used as a group home. A group home is used for individuals with special needs, including the frail elderly, developmentally and/or physically disabled."^^xsd:string ;
                    rdfs:label "Group Home Indicator"^^xsd:string .


###  http://mismo.org/Subset/hasBorrower
:hasBorrower rdf:type owl:ObjectProperty ;
             rdfs:domain :Loan ;
             rdfs:range <http://mismo.org/Containers/Borrower> ;
             rdfs:label "has borrower"^^xsd:string .


###  http://mismo.org/Subset/hasHazardInsurance
:hasHazardInsurance rdf:type owl:ObjectProperty ;
                    rdfs:domain :Property ;
                    rdfs:range :HazardInsurance ;
                    rdfs:label "has hazard insurance"^^xsd:string .


###  http://mismo.org/Subset/hazardInsuranceCoverageAmount
:hazardInsuranceCoverageAmount rdf:type owl:ObjectProperty ;
                               rdfs:domain :HazardInsurance ;
                               rdfs:range <http://mismo.org/DataTypes/MISMOAmount> ;
                               rdfs:comment "The coverage amount of the property casualty policy on the property securing the loan."^^xsd:string ;
                               rdfs:label "Hazard Insurance Coverage Amount"^^xsd:string .


###  http://mismo.org/Subset/hazardInsuranceCoverageType
:hazardInsuranceCoverageType rdf:type owl:ObjectProperty ;
                             rdfs:domain :HazardInsurance ;
                             rdfs:range <http://mismo.org/EnumeratedTypes/HazardInsuranceCoverageEnum> ;
                             rdfs:comment "The type of loss the insurance policy covers."^^xsd:string ;
                             rdfs:label "Hazard Insurance Coverage Type"^^xsd:string .


###  http://mismo.org/Subset/hazardInsuranceCoverageTypeOtherDescription
:hazardInsuranceCoverageTypeOtherDescription rdf:type owl:ObjectProperty ;
                                             rdfs:domain :HazardInsurance ;
                                             rdfs:range <http://mismo.org/DataTypes/MISMOString> ;
                                             rdfs:comment "A free-form text field used to capture the hazard insurance coverage type if Other is selected as the hazard insurance coverage type."^^xsd:string ;
                                             rdfs:label "Hazard Insurance Coverage Type Other Description"^^xsd:string .


###  http://mismo.org/Subset/hazardInsuranceEffectiveDate
:hazardInsuranceEffectiveDate rdf:type owl:ObjectProperty ;
                              rdfs:domain :HazardInsurance ;
                              rdfs:range <http://mismo.org/DataTypes/MISMODate> ;
                              rdfs:comment "The date the hazard insurance went into effect."^^xsd:string ;
                              rdfs:label "Hazard Insurance Effective Date"^^xsd:string .


###  http://mismo.org/Subset/hazardInsuranceEscrowedIndicator
:hazardInsuranceEscrowedIndicator rdf:type owl:ObjectProperty ;
                                  rdfs:domain :HazardInsurance ;
                                  rdfs:range <http://mismo.org/DataTypes/MISMOIndicator> ;
                                  rdfs:comment "Indicates whether hazard is paid by the borrower or the lender."^^xsd:string ;
                                  rdfs:label "Hazard Insurance Escrowed Indicator"^^xsd:string .


###  http://mismo.org/Subset/hazardInsuranceExpirationDate
:hazardInsuranceExpirationDate rdf:type owl:ObjectProperty ;
                               rdfs:domain :HazardInsurance ;
                               rdfs:range <http://mismo.org/DataTypes/MISMODate> ;
                               rdfs:comment "The date the property casualty policy expires."^^xsd:string ;
                               rdfs:label "Hazard Insurance Expiration Date"^^xsd:string .


###  http://mismo.org/Subset/hazardInsuranceNextPremiumDueDate
:hazardInsuranceNextPremiumDueDate rdf:type owl:ObjectProperty ;
                                   rdfs:domain :HazardInsurance ;
                                   rdfs:range <http://mismo.org/DataTypes/MISMODate> ;
                                   rdfs:comment "The month and year the next property casualty premium is due."^^xsd:string ;
                                   rdfs:label "Hazard Insurance Next Premium Due Date"^^xsd:string .


###  http://mismo.org/Subset/hazardInsuranceNonStandardPolicyType
:hazardInsuranceNonStandardPolicyType rdf:type owl:ObjectProperty ;
                                      rdfs:domain :HazardInsurance ;
                                      rdfs:range <http://mismo.org/EnumeratedTypes/HazardInsuranceNonStandardPolicyEnum> ;
                                      rdfs:comment "Additional Description of the Hazard Insurance coverage document."^^xsd:string ;
                                      rdfs:label "Hazard Insurance Non Standard Policy Type"^^xsd:string .


###  http://mismo.org/Subset/hazardInsuranceNonStandardPolicyTypeOtherDescription
:hazardInsuranceNonStandardPolicyTypeOtherDescription rdf:type owl:ObjectProperty ;
                                                      rdfs:domain :HazardInsurance ;
                                                      rdfs:range <http://mismo.org/DataTypes/MISMOString> ;
                                                      rdfs:comment "A free-form text field used to capture the Hazard Insurance Non-standard Policy Type if Other is selected as the Hazard Insurance Non Standard Policy Type."^^xsd:string ;
                                                      rdfs:label "Hazard Insurance Non Standard Policy Type Other Description"^^xsd:string .


###  http://mismo.org/Subset/hazardInsurancePolicyCancellationDate
:hazardInsurancePolicyCancellationDate rdf:type owl:ObjectProperty ;
                                       rdfs:domain :HazardInsurance ;
                                       rdfs:range <http://mismo.org/DataTypes/MISMODate> ;
                                       rdfs:comment "The date the insurance company terminates the policy."^^xsd:string ;
                                       rdfs:label "Hazard Insurance Policy Cancellation Date"^^xsd:string .


###  http://mismo.org/Subset/hazardInsurancePolicyIdentifier
:hazardInsurancePolicyIdentifier rdf:type owl:ObjectProperty ;
                                 rdfs:domain :HazardInsurance ;
                                 rdfs:range <http://mismo.org/DataTypes/MISMOIdentifier> ;
                                 rdfs:comment "The number assigned to the policy by the insurance company."^^xsd:string ;
                                 rdfs:label "Hazard Insurance Policy Identifier"^^xsd:string .


###  http://mismo.org/Subset/hazardInsurancePremiumAmount
:hazardInsurancePremiumAmount rdf:type owl:ObjectProperty ;
                              rdfs:domain :HazardInsurance ;
                              rdfs:range <http://mismo.org/DataTypes/MISMOAmount> ;
                              rdfs:comment "The projected property casualty premium to be paid."^^xsd:string ;
                              rdfs:label "Hazard Insurance Premium Amount"^^xsd:string .


###  http://mismo.org/Subset/hazardInsurancePremiumMonthsCount
:hazardInsurancePremiumMonthsCount rdf:type owl:ObjectProperty ;
                                   rdfs:domain :HazardInsurance ;
                                   rdfs:range <http://mismo.org/DataTypes/MISMOCount> ;
                                   rdfs:comment "The term expressed in months between each property casualty insurance premium."^^xsd:string ;
                                   rdfs:label "Hazard Insurance Premium Months Count"^^xsd:string .


###  http://mismo.org/Subset/hazardInsuranceReplacementValueIndicator
:hazardInsuranceReplacementValueIndicator rdf:type owl:ObjectProperty ;
                                          rdfs:domain :HazardInsurance ;
                                          rdfs:range <http://mismo.org/DataTypes/MISMOIndicator> ;
                                          rdfs:comment "When true, indicates that the coverage provides full replacement value of the property."^^xsd:string ;
                                          rdfs:label "Hazard Insurance Replacement Value Indicator"^^xsd:string .


###  http://mismo.org/Subset/hazardInsurances
:hazardInsurances rdf:type owl:ObjectProperty ;
                  rdfs:domain :Property ;
                  rdfs:range <http://mismo.org/Containers/HazardInsurance> ;
                  rdfs:comment "Information about one or more HAZARD_INSURANCE. Holds all occurrences of HAZARD_INSURANCE."^^xsd:string ;
                  rdfs:label "hazard insurances"^^xsd:string .


###  http://mismo.org/Subset/heloc
:heloc rdf:type owl:ObjectProperty ;
       rdfs:domain :Loan ;
       rdfs:range <http://mismo.org/Containers/HELOC> ;
       rdfs:comment "Information about Home Equity Lines Of Credit (HELOCs)."^^xsd:string .


###  http://mismo.org/Subset/heloc-Indicator
:heloc-Indicator rdf:type owl:ObjectProperty ;
                 rdfs:domain :Loan ;
                 rdfs:range :MISMOIndicator ;
                 rdfs:comment "When true, indicates that the loan is a Home Equity Line of Credit (HELOC)."^^xsd:string ;
                 rdfs:label "HELOC Indicator"^^xsd:string .


###  http://mismo.org/Subset/highCostMortgages
:highCostMortgages rdf:type owl:ObjectProperty ;
                   rdfs:domain :Loan ;
                   rdfs:range <http://mismo.org/Containers/HighCostMortgage> ;
                   rdfs:comment "Information related to one or more determinations of the transaction as a high cost or higher priced mortgage. Holds all occurrences of HIGH_COST_MORTGAGE."^^xsd:string ;
                   rdfs:label "high cost mortgages"^^xsd:string .


###  http://mismo.org/Subset/higherPricedMortgageLoanIndicator
:higherPricedMortgageLoanIndicator rdf:type owl:ObjectProperty ;
                                   rdfs:domain :Loan ;
                                   rdfs:range :MISMOIndicator ;
                                   rdfs:comment "When true, indicates the transaction is considered to be a higher priced mortgage loan under Regulation Z requirements."^^xsd:string ;
                                   rdfs:label "Higher Priced Mortgage Loan Indicator"^^xsd:string .


###  http://mismo.org/Subset/highwayContractBoxIdentifier
:highwayContractBoxIdentifier rdf:type owl:ObjectProperty ;
                              rdfs:domain :Address ;
                              rdfs:range :MISMOIdentifier ;
                              rdfs:comment "A unique alphanumeric string identifying the highway contract route box for the delivery of mail, as assigned by the USPS."^^xsd:string ;
                              rdfs:label "Highway Contract Box Identifier"^^xsd:string .


###  http://mismo.org/Subset/highwayContractRouteIdentifier
:highwayContractRouteIdentifier rdf:type owl:ObjectProperty ;
                                rdfs:domain :Address ;
                                rdfs:range :MISMOIdentifier ;
                                rdfs:comment "A unique alphanumeric string identifying the highway contract route for the delivery of mail, as assigned by the USPS."^^xsd:string ;
                                rdfs:label "Highway Contract Route Identifier"^^xsd:string .


###  http://mismo.org/Subset/hmdaLoan
:hmdaLoan rdf:type owl:ObjectProperty ;
          rdfs:domain :Loan ;
          rdfs:range <http://mismo.org/Containers/HMDA-Loan> ;
          rdfs:comment "Information used for reporting on a HMDA specific loan."^^xsd:string ;
          rdfs:label "hmda loan"^^xsd:string .


###  http://mismo.org/Subset/homeBuyersHomeownershipEducationCertificateIndicator
:homeBuyersHomeownershipEducationCertificateIndicator rdf:type owl:ObjectProperty ;
                                                      rdfs:domain :Loan ;
                                                      rdfs:range :MISMOIndicator ;
                                                      rdfs:comment "Indicates whether the Home Buyers/Home Ownership Education certificate is included in the loan file."^^xsd:string ;
                                                      rdfs:label "Home Buyers Homeownership Education Certificate Indicator"^^xsd:string .


###  http://mismo.org/Subset/homeownerResponsibleForExteriorMaintenanceIndicator
:homeownerResponsibleForExteriorMaintenanceIndicator rdf:type owl:ObjectProperty ;
                                                     rdfs:domain :Property ;
                                                     rdfs:range :MISMOIndicator ;
                                                     rdfs:comment "When true, indicates that the homeowner is responsible for maintaining the exterior of the subject property."^^xsd:string ;
                                                     rdfs:label "Homeowner Responsible For Exterior Maintenance Indicator"^^xsd:string .


###  http://mismo.org/Subset/homeownersAssociationIndicator
:homeownersAssociationIndicator rdf:type owl:ObjectProperty ;
                                rdfs:domain :Property ;
                                rdfs:range :MISMOIndicator ;
                                rdfs:comment "When true, indicates there is a homeowners association tied to the property."^^xsd:string ;
                                rdfs:label "Homeowners Association Indicator"^^xsd:string .


###  http://mismo.org/Subset/homeownersAssociations
:homeownersAssociations rdf:type owl:ObjectProperty ;
                        rdfs:domain :Property ;
                        rdfs:range <http://mismo.org/Containers/HomeownersAssociation> ;
                        rdfs:comment "Information about one or more homeowners associations. Holds all occurrences of HOMEOWNERS ASSOCIATION."^^xsd:string ;
                        rdfs:label "homeowners associations"^^xsd:string .


###  http://mismo.org/Subset/housingExpenseSummary
:housingExpenseSummary rdf:type owl:ObjectProperty ;
                       rdfs:domain :Loan ;
                       rdfs:range <http://mismo.org/Containers/HousingExpenseSummary> ;
                       rdfs:comment "Summary information about housing expenses."^^xsd:string ;
                       rdfs:label "housing expense summary"^^xsd:string .


###  http://mismo.org/Subset/housingExpenses
:housingExpenses rdf:type owl:ObjectProperty ;
                 rdfs:domain :Loan ;
                 rdfs:range <http://mismo.org/Containers/HousingExpense> ;
                 rdfs:comment "Information regarding one or more types of housing expense. Holds all occurrences of HOUSING_EXPENSE."^^xsd:string ;
                 rdfs:label "housing expenses"^^xsd:string .


###  http://mismo.org/Subset/improvements
:improvements rdf:type owl:ObjectProperty ;
              rdfs:domain :Property ;
              rdfs:range <http://mismo.org/Containers/Improvement> ;
              rdfs:comment "Information about one or more improvements on the property. Contains all occurrences of IMPROVEMENT."^^xsd:string .


###  http://mismo.org/Subset/ineligibleLoanProductIndicator
:ineligibleLoanProductIndicator rdf:type owl:ObjectProperty ;
                                rdfs:domain :Loan ;
                                rdfs:range <http://mismo.org/DataTypes/MISMOIndicator_Base> ;
                                rdfs:comment "When true, indicates this Loan Product is ineligible based on Deal characteristics."^^xsd:string ;
                                rdfs:label "Ineligible Loan Product Indicator"^^xsd:string .


###  http://mismo.org/Subset/initialFixedPeriodEffectiveMonthsCount
:initialFixedPeriodEffectiveMonthsCount rdf:type owl:ObjectProperty ;
                                        rdfs:domain :Loan ;
                                        rdfs:range <http://mismo.org/DataTypes/MISMOCount> ;
                                        rdfs:comment "The number of months in the initial fixed period of a loan with an adjustable rate or payment."^^xsd:string ;
                                        rdfs:label "Initial Fixed Period Effective Months Count"^^xsd:string .


###  http://mismo.org/Subset/inspections
:inspections rdf:type owl:ObjectProperty ;
             rdfs:domain :Property ;
             rdfs:range <http://mismo.org/Containers/Inspection> ;
             rdfs:comment "Information about one or more types of inspection of the property. Holds all occurrences of INSPECTION."^^xsd:string .


###  http://mismo.org/Subset/insuranceClaims
:insuranceClaims rdf:type owl:ObjectProperty ;
                 rdfs:domain :Loan ;
                 rdfs:range <http://mismo.org/Containers/InsuranceClaim> ;
                 rdfs:comment "Information about one or more insurance claims proceeds associated with the loan or subject property. Holds all occurrences of INSURANCE_CLAIM."^^xsd:string ;
                 rdfs:label "insurance claims"^^xsd:string .


###  http://mismo.org/Subset/insuranceRequiredIndicator
:insuranceRequiredIndicator rdf:type owl:ObjectProperty ;
                            rdfs:domain :HazardInsurance ;
                            rdfs:range <http://mismo.org/DataTypes/MISMOIndicator> ;
                            rdfs:comment "When true, indicates that a specific Hazard Insurance Coverage Type on the property is required for the loan transaction."^^xsd:string ;
                            rdfs:label "Insurance Required Indicator"^^xsd:string .


###  http://mismo.org/Subset/interestCalculation
:interestCalculation rdf:type owl:ObjectProperty ;
                     rdfs:domain :Loan ;
                     rdfs:range <http://mismo.org/Containers/InterestCalculation> ;
                     rdfs:comment "Information regarding the RULES and OCCURRENCES for Interest Accrual calculation, as established by contract at loan origination."^^xsd:string ;
                     rdfs:label "interest calculation"^^xsd:string .


###  http://mismo.org/Subset/interestCreditedToBorrowerIndicator
:interestCreditedToBorrowerIndicator rdf:type owl:ObjectProperty ;
                                     rdfs:domain :Loan ;
                                     rdfs:range :MISMOIndicator ;
                                     rdfs:comment "Identifies whether interest was credited to the borrower at time of closing for a closed-end mortgage."^^xsd:string ;
                                     rdfs:label "Interest Credited To Borrower Indicator"^^xsd:string .


###  http://mismo.org/Subset/interestOnly
:interestOnly rdf:type owl:ObjectProperty ;
              rdfs:domain :Loan ;
              rdfs:range <http://mismo.org/Containers/InterestOnly> ;
              rdfs:comment "Information about Interest Only loan features, where a Borrower pays only interest for a specific period of time on the loan before payments switch to full interest and principal amortizing payments."^^xsd:string ;
              rdfs:label "interest only"^^xsd:string .


###  http://mismo.org/Subset/interestOnlyIndicator
:interestOnlyIndicator rdf:type owl:ObjectProperty ;
                       rdfs:domain :Loan ;
                       rdfs:range :MISMOIndicator ;
                       rdfs:comment "When true, indicates that the loan terms allow interest-only payments to be made for a specified time period."^^xsd:string ;
                       rdfs:label "Interest Only Indicator"^^xsd:string .


###  http://mismo.org/Subset/interestRateIncreaseIndicator
:interestRateIncreaseIndicator rdf:type owl:ObjectProperty ;
                               rdfs:domain :Loan ;
                               rdfs:range :MISMOIndicator ;
                               rdfs:comment "When true, indicates that the interest rate on the loan can increase after the closing."^^xsd:string ;
                               rdfs:label "Interest Rate Increase Indicator"^^xsd:string .


###  http://mismo.org/Subset/investmentRentalIncomePresentIndicator
:investmentRentalIncomePresentIndicator rdf:type owl:ObjectProperty ;
                                        rdfs:domain :Property ;
                                        rdfs:range :MISMOIndicator ;
                                        rdfs:comment "When true, indicates that an investment property is currently generating rental income on behalf of the owner."^^xsd:string ;
                                        rdfs:label "Investment Rental Income Present Indicator"^^xsd:string .


###  http://mismo.org/Subset/investorFeatures
:investorFeatures rdf:type owl:ObjectProperty ;
                  rdfs:domain [ rdf:type owl:Class ;
                                owl:unionOf ( :DealSet
                                              :Loan
                                            )
                              ] ;
                  rdfs:range <http://mismo.org/Containers/InvestorFeature> ;
                  rdfs:comment "Information about one or more INVESTOR_FEATURE. Holds all occurrences of INVESTOR_FEATURE."^^xsd:string ;
                  rdfs:label "investor features"^^xsd:string .


###  http://mismo.org/Subset/investorLoanInformation
:investorLoanInformation rdf:type owl:ObjectProperty ;
                         rdfs:domain :Loan ;
                         rdfs:range <http://mismo.org/Containers/InvestorLoanInformation> ;
                         rdfs:comment "Data specific to the relationship between the seller and the investor, including the reporting and financial obligations between the seller, the servicer, and the investor. The structure also holds data on the investor's interest in the Delivery Loan."^^xsd:string ;
                         rdfs:label "investor loan information"^^xsd:string .


###  http://mismo.org/Subset/investorREO-PropertyIdentifier
:investorREO-PropertyIdentifier rdf:type owl:ObjectProperty ;
                                rdfs:domain :Property ;
                                rdfs:range :MISMOIdentifier ;
                                rdfs:comment "A unique identifier assigned by an investor to a property acquired as the result of delinquency."^^xsd:string ;
                                rdfs:label "Investor REO Property Identifier"^^xsd:string .


###  http://mismo.org/Subset/jurisdictionHighCostLoanIndicator
:jurisdictionHighCostLoanIndicator rdf:type owl:ObjectProperty ;
                                   rdfs:domain :Loan ;
                                   rdfs:range :MISMOIndicator ;
                                   rdfs:comment "When true, indicates the loan is determined to be high cost under the jurisdictions high cost rules or requirements."^^xsd:string ;
                                   rdfs:label "Jurisdiction High Cost Loan Indicator"^^xsd:string .


###  http://mismo.org/Subset/landTrustType
:landTrustType rdf:type owl:ObjectProperty ;
               rdfs:domain :Property ;
               rdfs:range <http://mismo.org/EnumeratedTypes/LandTrustEnum> ;
               rdfs:comment "A value from a MISMO prescribed list that specifies the type of land trust associated with the title."^^xsd:string ;
               rdfs:label "Land Trust Type"^^xsd:string .


###  http://mismo.org/Subset/landTrustTypeOtherDescription
:landTrustTypeOtherDescription rdf:type owl:ObjectProperty ;
                               rdfs:domain :Property ;
                               rdfs:range :MISMOString ;
                               rdfs:comment "A free-form text field used to collect additional information when Other is selected for Land Trust Type."^^xsd:string ;
                               rdfs:label "Land Trust Type Other Description"^^xsd:string .


###  http://mismo.org/Subset/landUseDescription
:landUseDescription rdf:type owl:ObjectProperty ;
                    rdfs:domain :Property ;
                    rdfs:range :MISMOString ;
                    rdfs:comment "A free-form text field used to further describe the land use of the property as defined by Land Use Type."^^xsd:string ;
                    rdfs:label "Land Use Description"^^xsd:string .


###  http://mismo.org/Subset/landUseType
:landUseType rdf:type owl:ObjectProperty ;
             rdfs:domain :Property ;
             rdfs:range <http://mismo.org/EnumeratedTypes/LandUseEnum> ;
             rdfs:comment "Identifies the designation of land use by a governmental authority described by Land Used Description."^^xsd:string ;
             rdfs:label "Land Use Type"^^xsd:string .


###  http://mismo.org/Subset/landUseTypeOtherDescription
:landUseTypeOtherDescription rdf:type owl:ObjectProperty ;
                             rdfs:domain :Property ;
                             rdfs:range :MISMOString ;
                             rdfs:comment "A free-form text field used to describe the land use designation if Other is selected as the Property Land Use Type."^^xsd:string ;
                             rdfs:label "Land Use Type Other Description"^^xsd:string .


###  http://mismo.org/Subset/lang
:lang rdf:type owl:ObjectProperty ;
      rdfs:domain :MISMOString ;
      rdfs:range <http://mismo.org/DataTypes/MISMOCode_Base> .


###  http://mismo.org/Subset/lateCharge
:lateCharge rdf:type owl:ObjectProperty ;
            rdfs:domain :Loan ;
            rdfs:range <http://mismo.org/Containers/LateCharge> ;
            rdfs:comment "Defines the calculation of late charges that apply when a borrower does not make timely payments."^^xsd:string ;
            rdfs:label "late charge"^^xsd:string .


###  http://mismo.org/Subset/legalDescriptions
:legalDescriptions rdf:type owl:ObjectProperty ;
                   rdfs:domain :Property ;
                   rdfs:range <http://mismo.org/Containers/LegalDescription> ;
                   rdfs:comment "TERM NOT FOUND"^^xsd:string ;
                   rdfs:label "legal descriptions"^^xsd:string .


###  http://mismo.org/Subset/lenderDesignatedDecliningMarketIdentifier
:lenderDesignatedDecliningMarketIdentifier rdf:type owl:ObjectProperty ;
                                           rdfs:domain :Property ;
                                           rdfs:range :MISMOIdentifier ;
                                           rdfs:comment "Identifies the type of declining market based on lender analysis."^^xsd:string ;
                                           rdfs:label "Lender Designated Declining Market Identifier"^^xsd:string .


###  http://mismo.org/Subset/lenderPlacedHazardInsuranceIndicator
:lenderPlacedHazardInsuranceIndicator rdf:type owl:ObjectProperty ;
                                      rdfs:domain :Loan ;
                                      rdfs:range :MISMOIndicator ;
                                      rdfs:comment "When true, indicates that there is lender placed hazard insurance of any kind associated with this loan."^^xsd:string ;
                                      rdfs:label "Lender Placed Hazard Insurance Indicator"^^xsd:string .


###  http://mismo.org/Subset/lenderSelfInsuredIndicator
:lenderSelfInsuredIndicator rdf:type owl:ObjectProperty ;
                            rdfs:domain :Loan ;
                            rdfs:range :MISMOIndicator ;
                            rdfs:comment "Indicates that the Lender will provide self-insurance."^^xsd:string ;
                            rdfs:label "Lender Self Insured Indicator"^^xsd:string .


###  http://mismo.org/Subset/lendingLimitAmount
:lendingLimitAmount rdf:type owl:ObjectProperty ;
                    rdfs:domain :Loan ;
                    rdfs:range :MISMOAmount ;
                    rdfs:comment "The maximum dollar amount limit for the mortgage loan."^^xsd:string ;
                    rdfs:label "Lending Limit Amount"^^xsd:string .


###  http://mismo.org/Subset/lendingLimitType
:lendingLimitType rdf:type owl:ObjectProperty ;
                  rdfs:domain :Loan ;
                  rdfs:range <http://mismo.org/EnumeratedTypes/LendingLimitEnum> ;
                  rdfs:comment "Specifies the criteria, guidelines or calculation used to establish the Lending Limit Amount."^^xsd:string ;
                  rdfs:label "Lending Limit Type"^^xsd:string .


###  http://mismo.org/Subset/lendingLimitTypeOtherDescription
:lendingLimitTypeOtherDescription rdf:type owl:ObjectProperty ;
                                  rdfs:domain :Loan ;
                                  rdfs:range :MISMOString ;
                                  rdfs:comment "A free-form text field used to collect additional information when Other is selected for Other is selected for the Lending Limit Type."^^xsd:string ;
                                  rdfs:label "Lending Limit Type Other Description"^^xsd:string .


###  http://mismo.org/Subset/liabilities
:liabilities rdf:type owl:ObjectProperty ;
             rdfs:domain :DealSequence ;
             rdfs:range <http://mismo.org/Containers/Liability> ;
             rdfs:comment "collection of objects that describe the liabilities of borrower parties that were examined to determine credit worthiness."^^xsd:string .


###  http://mismo.org/Subset/liabilitySummary
:liabilitySummary rdf:type owl:ObjectProperty ;
                  rdfs:domain :DealSequence ;
                  rdfs:range <http://mismo.org/Containers/LiabilitySummary> ;
                  rdfs:comment "Information regarding the type and totals of a defined group of liabilities."^^xsd:string ;
                  rdfs:label "liability summary"^^xsd:string .


###  http://mismo.org/Subset/licenses
:licenses rdf:type owl:ObjectProperty ;
          rdfs:domain :Property ;
          rdfs:range <http://mismo.org/Containers/License> ;
          rdfs:comment "Information about one or more types of license. Holds all occurrences of LICENSE."^^xsd:string .


###  http://mismo.org/Subset/lienHolderSameAsSubjectLoanIndicator
:lienHolderSameAsSubjectLoanIndicator rdf:type owl:ObjectProperty ;
                                      rdfs:domain :Loan ;
                                      rdfs:range :MISMOIndicator ;
                                      rdfs:comment "Indicates that the lien holder of the related loan is the same as the lien holder of the subject loan."^^xsd:string ;
                                      rdfs:label "Lien Holder Same As Subject Loan Indicator"^^xsd:string .


###  http://mismo.org/Subset/listingInformationSummary
:listingInformationSummary rdf:type owl:ObjectProperty ;
                           rdfs:domain :Property ;
                           rdfs:range <http://mismo.org/Containers/ListingInformationSummary> ;
                           rdfs:comment "Contains aggregate listing information for a specific real property instance."^^xsd:string ;
                           rdfs:label "listing information summary"^^xsd:string .


###  http://mismo.org/Subset/listingInformations
:listingInformations rdf:type owl:ObjectProperty ;
                     rdfs:domain :Property ;
                     rdfs:range <http://mismo.org/Containers/ListingInformation> ;
                     rdfs:comment "Information about one or more types of listing information. Holds all occurrences of LISTING_INFORMATION."^^xsd:string ;
                     rdfs:label "listing informations"^^xsd:string .


###  http://mismo.org/Subset/litigations
:litigations rdf:type owl:ObjectProperty ;
             rdfs:domain :DealSequence ;
             rdfs:range <http://mismo.org/Containers/Litigation> ;
             rdfs:comment "Information about one or more litigations. Holds all occurrences of LITIGATION."^^xsd:string .


###  http://mismo.org/Subset/livingUnitExcludingADU-Count
:livingUnitExcludingADU-Count rdf:type owl:ObjectProperty ;
                              rdfs:domain :Property ;
                              rdfs:range <http://mismo.org/DataTypes/MISMOCount> ;
                              rdfs:comment "The number of separate living units in the subject property, excluding any accessory dwelling units."^^xsd:string ;
                              rdfs:label "Living Unit Excluding ADU Count"^^xsd:string .


###  http://mismo.org/Subset/loanAffordableIndicator
:loanAffordableIndicator rdf:type owl:ObjectProperty ;
                         rdfs:domain :Loan ;
                         rdfs:range :MISMOIndicator ;
                         rdfs:comment "When true, indicates that the loan is classified as an affordable loan by the lender or the investor."^^xsd:string ;
                         rdfs:label "Loan Affordable Indicator"^^xsd:string .


###  http://mismo.org/Subset/loanAgeMonthsCount
:loanAgeMonthsCount rdf:type owl:ObjectProperty ;
                    rdfs:domain :Loan ;
                    rdfs:range <http://mismo.org/DataTypes/MISMOCount> ;
                    rdfs:comment "The age of the loan expressed in months calculated as defined by trading partner agreement."^^xsd:string ;
                    rdfs:label "Loan Age Months Count"^^xsd:string .


###  http://mismo.org/Subset/loanAmountIncreaseIndicator
:loanAmountIncreaseIndicator rdf:type owl:ObjectProperty ;
                             rdfs:domain :Loan ;
                             rdfs:range :MISMOIndicator ;
                             rdfs:comment "When true, indicates that the loan amount can increase after closing."^^xsd:string ;
                             rdfs:label "Loan Amount Increase Indicator"^^xsd:string .


###  http://mismo.org/Subset/loanApprovalDate
:loanApprovalDate rdf:type owl:ObjectProperty ;
                  rdfs:domain :Loan ;
                  rdfs:range :MISMODate ;
                  rdfs:comment "The date the mortgage loan approval was made by the lender to the borrower. A loan approval involves verifying credit, down payment, employment history, etc. of the borrower(s) and will generally state that the borrower is approved for a loan upon satisfaction of certain conditions."^^xsd:string ;
                  rdfs:label "Loan Approval Date"^^xsd:string .


###  http://mismo.org/Subset/loanApprovalExpirationDate
:loanApprovalExpirationDate rdf:type owl:ObjectProperty ;
                            rdfs:domain :Loan ;
                            rdfs:range :MISMODate ;
                            rdfs:comment "The date the mortgage loan approval expires."^^xsd:string ;
                            rdfs:label "Loan Approval Expiration Date"^^xsd:string .


###  http://mismo.org/Subset/loanApprovalPeriodDaysCount
:loanApprovalPeriodDaysCount rdf:type owl:ObjectProperty ;
                             rdfs:domain :Loan ;
                             rdfs:range <http://mismo.org/DataTypes/MISMOCount> ;
                             rdfs:comment "The number of days the mortgage loan approval is in effect."^^xsd:string ;
                             rdfs:label "Loan Approval Period Days Count"^^xsd:string .


###  http://mismo.org/Subset/loanAssetAddedIndicator
:loanAssetAddedIndicator rdf:type owl:ObjectProperty ;
                         rdfs:domain :Loan ;
                         rdfs:range :MISMOIndicator ;
                         rdfs:comment "When true, indicates that this loan asset was added to the security in the current investor reporting period."^^xsd:string ;
                         rdfs:label "Loan Asset Added Indicator"^^xsd:string .


###  http://mismo.org/Subset/loanClosingStatusType
:loanClosingStatusType rdf:type owl:ObjectProperty ;
                       rdfs:domain :Loan ;
                       rdfs:range <http://mismo.org/EnumeratedTypes/LoanClosingStatusEnum> ;
                       rdfs:comment "Defines whether the loan is a closed loan purchase or a table funded loan."^^xsd:string ;
                       rdfs:label "Loan Closing Status Type"^^xsd:string .


###  http://mismo.org/Subset/loanComments
:loanComments rdf:type owl:ObjectProperty ;
              rdfs:domain :Loan ;
              rdfs:range <http://mismo.org/Containers/LoanComment> ;
              rdfs:comment "Information about one or more LOAN_COMMENT. Holds all occurrences of LOAN_COMMENT."^^xsd:string ;
              rdfs:label "loan comments"^^xsd:string .


###  http://mismo.org/Subset/loanCommitmentDate
:loanCommitmentDate rdf:type owl:ObjectProperty ;
                    rdfs:domain :Loan ;
                    rdfs:range :MISMODate ;
                    rdfs:comment "The date the mortgage loan commitment to the borrower was made. The loan commitment is a formal, binding offer from a lender that a specified amount of loan or line of credit will be made available to the named borrower at a certain interest rate, during a certain period and, usually, for a certain purpose. The commitment also specifies the terms and requirements under which the loan will be advanced."^^xsd:string ;
                    rdfs:label "Loan Commitment Date"^^xsd:string .


###  http://mismo.org/Subset/loanCommitmentExpirationDate
:loanCommitmentExpirationDate rdf:type owl:ObjectProperty ;
                              rdfs:domain :Loan ;
                              rdfs:range :MISMODate ;
                              rdfs:comment "The date the mortgage loan commitment expires."^^xsd:string ;
                              rdfs:label "Loan Commitment Expiration Date"^^xsd:string .


###  http://mismo.org/Subset/loanCommitmentPeriodDaysCount
:loanCommitmentPeriodDaysCount rdf:type owl:ObjectProperty ;
                               rdfs:domain :Loan ;
                               rdfs:range <http://mismo.org/DataTypes/MISMOCount> ;
                               rdfs:comment "The number of days the mortgage loan commitment is in effect."^^xsd:string ;
                               rdfs:label "Loan Commitment Period Days Count"^^xsd:string .


###  http://mismo.org/Subset/loanEstimateWaitingPeriodWaivedIndicator
:loanEstimateWaitingPeriodWaivedIndicator rdf:type owl:ObjectProperty ;
                                          rdfs:domain :Loan ;
                                          rdfs:range :MISMOIndicator ;
                                          rdfs:comment "When true, indicates that upon receipt of the Loan Estimate, and due to a bona fide personal financial emergency, the consumer modified or waived the seven-business-day waiting period that must be met prior to consummation of the mortgage loan transaction."^^xsd:string ;
                                          rdfs:label "Loan Estimate Waiting Period Waived Indicator"^^xsd:string .


###  http://mismo.org/Subset/loanFundingDate
:loanFundingDate rdf:type owl:ObjectProperty ;
                 rdfs:domain :Loan ;
                 rdfs:range :MISMODate ;
                 rdfs:comment "The date the loan funds were released from the original lender to the closing agent for disbursement to the borrower."^^xsd:string ;
                 rdfs:label "Loan Funding Date"^^xsd:string .


###  http://mismo.org/Subset/loanIdentifiers
:loanIdentifiers rdf:type owl:ObjectProperty ;
                 rdfs:domain :Loan ;
                 rdfs:range <http://mismo.org/Containers/LoanIdentifier> ;
                 rdfs:comment "Collection of current and previous identifiers for this loan."^^xsd:string ;
                 rdfs:label "loan identifiers"^^xsd:string .


###  http://mismo.org/Subset/loanLevelCredit
:loanLevelCredit rdf:type owl:ObjectProperty ;
                 rdfs:domain :Loan ;
                 rdfs:range <http://mismo.org/Containers/LoanLevelCredit> ;
                 rdfs:comment "Information about the credit score used for a loan when a loan level credit score methodology is used."^^xsd:string ;
                 rdfs:label "loan level credit"^^xsd:string .


###  http://mismo.org/Subset/loanLevelCreditScoreIndicator
:loanLevelCreditScoreIndicator rdf:type owl:ObjectProperty ;
                               rdfs:domain :Loan ;
                               rdfs:range :MISMOIndicator ;
                               rdfs:comment "When true, indicates that the loan level credit score was used for decisioning of the loan."^^xsd:string ;
                               rdfs:label "Loan Level Credit Score Indicator"^^xsd:string .


###  http://mismo.org/Subset/loanProduct
:loanProduct rdf:type owl:ObjectProperty ;
             rdfs:domain :Loan ;
             rdfs:range <http://mismo.org/Containers/LoanProduct> ;
             rdfs:comment "A collection of facts used as descriptors of the characteristics of a financial instrument for sale in the marketplace that an investor is willing to buy."^^xsd:string ;
             rdfs:label "loan product"^^xsd:string .


###  http://mismo.org/Subset/loanPrograms
:loanPrograms rdf:type owl:ObjectProperty ;
              rdfs:domain :Loan ;
              rdfs:range <http://mismo.org/Containers/LoanProgram> ;
              rdfs:comment "Information about one or more LOAN_PROGRAM. Holds all occurrences of LOAN_PROGRAM."^^xsd:string ;
              rdfs:label "loan programs"^^xsd:string .


###  http://mismo.org/Subset/loanRepaymentType
:loanRepaymentType rdf:type owl:ObjectProperty ;
                   rdfs:domain :Loan ;
                   rdfs:range <http://mismo.org/EnumeratedTypes/LoanRepaymentEnum> ;
                   rdfs:comment "Specifies whether the loan payment schedule has been calculated to fully repay the loan over the mortgage term."^^xsd:string ;
                   rdfs:label "Loan Repayment Type"^^xsd:string .


###  http://mismo.org/Subset/loanRepaymentTypeOtherDescription
:loanRepaymentTypeOtherDescription rdf:type owl:ObjectProperty ;
                                   rdfs:domain :Loan ;
                                   rdfs:range :MISMOString ;
                                   rdfs:comment "A free-form text field used to collect additional information when Other is selected for Loan Repayment Type."^^xsd:string ;
                                   rdfs:label "Loan Repayment Type Other Description"^^xsd:string .


###  http://mismo.org/Subset/loanSaleFundingDate
:loanSaleFundingDate rdf:type owl:ObjectProperty ;
                     rdfs:domain :Loan ;
                     rdfs:range :MISMODate ;
                     rdfs:comment "The date the investor releases funds to the seller of the loan."^^xsd:string ;
                     rdfs:label "Loan Sale Funding Date"^^xsd:string .


###  http://mismo.org/Subset/loanSecuredByType
:loanSecuredByType rdf:type owl:ObjectProperty ;
                   rdfs:domain :Loan ;
                   rdfs:range <http://mismo.org/EnumeratedTypes/LoanSecuredByEnum> ;
                   rdfs:comment "Specifies the type of collateral securing the loan."^^xsd:string ;
                   rdfs:label "Loan Secured By Type"^^xsd:string .


###  http://mismo.org/Subset/loanSecuredByTypeOtherDescription
:loanSecuredByTypeOtherDescription rdf:type owl:ObjectProperty ;
                                   rdfs:domain :Loan ;
                                   rdfs:range :MISMOString ;
                                   rdfs:comment "A free-form text field used to collect additional information when Other is selected for Loan Secured By Type."^^xsd:string ;
                                   rdfs:label "Loan Secured By Type Other Description"^^xsd:string .


###  http://mismo.org/Subset/loanSecuredIndicator
:loanSecuredIndicator rdf:type owl:ObjectProperty ;
                      rdfs:domain :Loan ;
                      rdfs:range :MISMOIndicator ;
                      rdfs:comment "When true, indicates that the loan is secured by some type of collateral."^^xsd:string ;
                      rdfs:label "Loan Secured Indicator"^^xsd:string .


###  http://mismo.org/Subset/loanSellerProvidedInvestmentRatingDescription
:loanSellerProvidedInvestmentRatingDescription rdf:type owl:ObjectProperty ;
                                               rdfs:domain :Loan ;
                                               rdfs:range :MISMOString ;
                                               rdfs:comment "The widely-recognized alpha code (e.g., AA, A, B, etc.) provided by the seller which specifies the credit risk class of a financial asset (e.g. a loan or mortgage backed security)."^^xsd:string ;
                                               rdfs:label "Loan Seller Provided Investment Rating Description"^^xsd:string .


###  http://mismo.org/Subset/loanState
:loanState rdf:type owl:ObjectProperty ;
           rdfs:domain :Loan ;
           rdfs:range <http://mismo.org/Containers/LoanState> ;
           rdfs:comment "Information regarding key milestones in the mortgage lifecycle and their associated dates."^^xsd:string ;
           rdfs:label "loan state"^^xsd:string .


###  http://mismo.org/Subset/loanStatuses
:loanStatuses rdf:type owl:ObjectProperty ;
              rdfs:domain :Loan ;
              rdfs:range <http://mismo.org/Containers/LoanStatus> ;
              rdfs:comment "Information about one or more LOAN_STATUS. Holds all occurrences of LOAN_STATUS."^^xsd:string ;
              rdfs:label "loan statuses"^^xsd:string .


###  http://mismo.org/Subset/loans
:loans rdf:type owl:ObjectProperty ;
       rdfs:domain [ rdf:type owl:Class ;
                     owl:unionOf ( :DealSequence
                                   :FloodResponse
                                 )
                   ] ;
       rdfs:range :Loan ;
       rdfs:comment "A collection of loans that are part of a single deal."^^xsd:string .


###  http://mismo.org/Subset/locationIdentifier
:locationIdentifier rdf:type owl:ObjectProperty ;
                    rdfs:domain :Property ;
                    rdfs:range <http://mismo.org/Containers/LocationIdentifier> ;
                    rdfs:comment "Information regarding location identifiers, which provide unique identification of specific locations."^^xsd:string ;
                    rdfs:label "location identifier"^^xsd:string .


###  http://mismo.org/Subset/lostNoteAffidavitIndicator
:lostNoteAffidavitIndicator rdf:type owl:ObjectProperty ;
                            rdfs:domain :Loan ;
                            rdfs:range :MISMOIndicator ;
                            rdfs:comment "Indicates whether or not a lost note affidavit (LNA) is associated with the loan."^^xsd:string ;
                            rdfs:label "Lost Note Affidavit Indicator"^^xsd:string .


###  http://mismo.org/Subset/ltv
:ltv rdf:type owl:ObjectProperty ;
     rdfs:domain :Loan ;
     rdfs:range <http://mismo.org/Containers/LTV> ;
     rdfs:comment "Information about the Loan-to-Value (LTV) ratio, its value and the date it was calculated."^^xsd:string .


###  http://mismo.org/Subset/mailStopCode
:mailStopCode rdf:type owl:ObjectProperty ;
              rdfs:domain :Address ;
              rdfs:range <http://mismo.org/DataTypes/MISMOCode> ;
              rdfs:comment "Uniquely identifies an individual or office within a private company for the purposes of internal mail distribution. USPS calls this a MailStop Code (MSC)."^^xsd:string ;
              rdfs:label "Mail Stop Code"^^xsd:string .


###  http://mismo.org/Subset/market
:market rdf:type owl:ObjectProperty ;
        rdfs:domain :Property ;
        rdfs:range <http://mismo.org/Containers/Market> ;
        rdfs:comment "Information about the inventories, trends and other facts about the market area of the property. A market is described in terms of its supply and demand characteristics for property in a given geographic location and economic condition."^^xsd:string .


###  http://mismo.org/Subset/maturity
:maturity rdf:type owl:ObjectProperty ;
          rdfs:domain :Loan ;
          rdfs:range <http://mismo.org/Containers/Maturity> ;
          rdfs:comment "Information regarding how the LOAN is paid in full over the life of loan as determined in the Note."^^xsd:string .


###  http://mismo.org/Subset/mersRegistrations
:mersRegistrations rdf:type owl:ObjectProperty ;
                   rdfs:domain :Loan ;
                   rdfs:range <http://mismo.org/Containers/MERS-Registration> ;
                   rdfs:comment "Information about one or more MERS_REGISTRATION. Holds all occurrences of MERS_REGISTRATION."^^xsd:string ;
                   rdfs:label "mers registrations"^^xsd:string .


###  http://mismo.org/Subset/metropolitanDivisionIndicator
:metropolitanDivisionIndicator rdf:type owl:ObjectProperty ;
                               rdfs:domain :Property ;
                               rdfs:range :MISMOIndicator ;
                               rdfs:comment "When true, indicates that the property is located in a Metropolitan Division."^^xsd:string ;
                               rdfs:label "Metropolitan Division Indicator"^^xsd:string .


###  http://mismo.org/Subset/mi-CoverageExistsIndicator
:mi-CoverageExistsIndicator rdf:type owl:ObjectProperty ;
                            rdfs:domain :Loan ;
                            rdfs:range :MISMOIndicator ;
                            rdfs:comment "When true, indicates that the loan is covered by mortgage insurance."^^xsd:string ;
                            rdfs:label "MI Coverage Exists Indicator"^^xsd:string .


###  http://mismo.org/Subset/mi-RequiredIndicator
:mi-RequiredIndicator rdf:type owl:ObjectProperty ;
                      rdfs:domain :Loan ;
                      rdfs:range :MISMOIndicator ;
                      rdfs:comment "Indicates that Mortgage Insurance is or was required as a condition for originating the loan."^^xsd:string ;
                      rdfs:label "MI Required Indicator"^^xsd:string .


###  http://mismo.org/Subset/miData
:miData rdf:type owl:ObjectProperty ;
        rdfs:domain :Loan ;
        rdfs:range <http://mismo.org/Containers/MI-Data> ;
        rdfs:comment "Information specific to the mortgage insurance carried by the lender on the loan."^^xsd:string ;
        rdfs:label "mi data"^^xsd:string .


###  http://mismo.org/Subset/mineralRightsLeasedIndicator
:mineralRightsLeasedIndicator rdf:type owl:ObjectProperty ;
                              rdfs:domain :Property ;
                              rdfs:range :MISMOIndicator ;
                              rdfs:comment "When true, indicates that mineral rights for the subject property is subject to a lease agreement."^^xsd:string ;
                              rdfs:label "Mineral Rights Leased Indicator"^^xsd:string .


###  http://mismo.org/Subset/mismo-LogicalDataDictionaryIdentifier
:mismo-LogicalDataDictionaryIdentifier rdf:type owl:ObjectProperty ;
                                       rdfs:domain :Deal ;
                                       rdfs:range <http://mismo.org/DataTypes/MISMOLogicalDataDictionaryIdentifier> ;
                                       rdfs:comment "The MISMO Logical Data Dictionary Identifier is a unique value that represents the version of the MISMO LDD section of the reference model to which the containing XML instance document complies. For detailed information, please see MISMO Engineering Guide 006 â âVersioning and Release Scheduleâ, at https://www.mismo.org/standards-resources/mismo-product/mismo-engineering-guideline-(meg)-6."^^xsd:string ;
                                       rdfs:label "MISMO Logical Data Dictionary Identifier"^^xsd:string .


###  http://mismo.org/Subset/mismo-ReferenceModelIdentifier
:mismo-ReferenceModelIdentifier rdf:type owl:ObjectProperty ;
                                rdfs:domain :Deal ;
                                rdfs:range <http://mismo.org/DataTypes/MISMOReferenceModelIdentifier> ;
                                rdfs:comment "The MISMO Reference Model Identifier is a unique value that represents the version of the MISMO reference model to which the containing XML instance document complies. For detailed information, please see MISMO Engineering Guide 006 â âVersioning and Release Scheduleâ, at https://www.mismo.org/standards-resources/mismo-product/mismo-engineering-guideline-(meg)-6."^^xsd:string ;
                                rdfs:label "MISMO Reference Model Identifier"^^xsd:string .


###  http://mismo.org/Subset/modificationSummary
:modificationSummary rdf:type owl:ObjectProperty ;
                     rdfs:domain :Loan ;
                     rdfs:range <http://mismo.org/Containers/ModificationSummary> ;
                     rdfs:comment "A summary of amounts forgiven over the course of the life of the modified loan."^^xsd:string ;
                     rdfs:label "modification summary"^^xsd:string .


###  http://mismo.org/Subset/modifications
:modifications rdf:type owl:ObjectProperty ;
               rdfs:domain :Loan ;
               rdfs:range <http://mismo.org/Containers/Modification> ;
               rdfs:comment "Information about one or more MODIFICATION. Holds all occurrences of MODIFICATION."^^xsd:string .


###  http://mismo.org/Subset/mortgageModificationIndicator
:mortgageModificationIndicator rdf:type owl:ObjectProperty ;
                               rdfs:domain :Loan ;
                               rdfs:range :MISMOIndicator ;
                               rdfs:comment "Indicates that a loan modification exists."^^xsd:string ;
                               rdfs:label "Mortgage Modification Indicator"^^xsd:string .


###  http://mismo.org/Subset/mortgageOriginatorFirstTimeHomeBuyerEligibilityIndicator
:mortgageOriginatorFirstTimeHomeBuyerEligibilityIndicator rdf:type owl:ObjectProperty ;
                                                          rdfs:domain :DealSequence ;
                                                          rdfs:range :MISMOIndicator ;
                                                          rdfs:comment "When true, indicates that the mortgage originator has determined that this deal is eligible to be considered a \"First Time Home Buyer.\""^^xsd:string ;
                                                          rdfs:label "Mortgage Originator First Time Home Buyer Eligibility Indicator"^^xsd:string .


###  http://mismo.org/Subset/mortgageScores
:mortgageScores rdf:type owl:ObjectProperty ;
                rdfs:domain :Loan ;
                rdfs:range <http://mismo.org/Containers/MortgageScore> ;
                rdfs:comment "Information about one or more MORTGAGE_SCORE. Holds all occurrences of MORTGAGE_SCORE."^^xsd:string ;
                rdfs:label "mortgage scores"^^xsd:string .


###  http://mismo.org/Subset/msa-Indicator
:msa-Indicator rdf:type owl:ObjectProperty ;
               rdfs:domain :Property ;
               rdfs:range :MISMOIndicator ;
               rdfs:comment "When true, indicates that the property is located in a Metropolitan Statistical Area."^^xsd:string ;
               rdfs:label "MSA Indicator"^^xsd:string .


###  http://mismo.org/Subset/nativeAmericanLandsIndicator
:nativeAmericanLandsIndicator rdf:type owl:ObjectProperty ;
                              rdfs:domain :Property ;
                              rdfs:range :MISMOIndicator ;
                              rdfs:comment "When true, indicates that the property is located on Native American lands."^^xsd:string ;
                              rdfs:label "Native American Lands Indicator"^^xsd:string .


###  http://mismo.org/Subset/nativeAmericanLandsType
:nativeAmericanLandsType rdf:type owl:ObjectProperty ;
                         rdfs:domain :Property ;
                         rdfs:range <http://mismo.org/EnumeratedTypes/NativeAmericanLandsEnum> ;
                         rdfs:comment "A value from a MISMO prescribed list that categorizes the legal means by which Native American land may be owned."^^xsd:string ;
                         rdfs:label "Native American Lands Type"^^xsd:string .


###  http://mismo.org/Subset/nativeAmericanLandsTypeOtherDescription
:nativeAmericanLandsTypeOtherDescription rdf:type owl:ObjectProperty ;
                                         rdfs:domain :Property ;
                                         rdfs:range :MISMOString ;
                                         rdfs:comment "A free-form text field used to collect additional information when Other is selected for Native American Lands Type."^^xsd:string ;
                                         rdfs:label "Native American Lands Type Other Description"^^xsd:string .


###  http://mismo.org/Subset/negativeAmortization
:negativeAmortization rdf:type owl:ObjectProperty ;
                      rdfs:domain :Loan ;
                      rdfs:range <http://mismo.org/Containers/NegativeAmortization> ;
                      rdfs:comment "Information regarding loans with negative amortization. Negative amortization is unpaid interest added to the mortgage principal. This applies to loans where the principal balance increases because the payments do not cover the interest."^^xsd:string ;
                      rdfs:label "negative amortization"^^xsd:string .


###  http://mismo.org/Subset/negativeAmortizationIndicator
:negativeAmortizationIndicator rdf:type owl:ObjectProperty ;
                               rdfs:domain :Loan ;
                               rdfs:range :MISMOIndicator ;
                               rdfs:comment "When true, indicates that the loan terms allow unpaid interest to be added to the principal of the loan that can or will result in negative amortization."^^xsd:string ;
                               rdfs:label "Negative Amortization Indicator"^^xsd:string .


###  http://mismo.org/Subset/neighborhood
:neighborhood rdf:type owl:ObjectProperty ;
              rdfs:domain :Property ;
              rdfs:range <http://mismo.org/Containers/Neighborhood> ;
              rdfs:comment "Information regarding the housing, schools, influences, land use and other facts about a neighborhood. A neighborhood is a geographically localized community within a larger city, town or suburb."^^xsd:string .


###  http://mismo.org/Subset/newConstructionIndicator
:newConstructionIndicator rdf:type owl:ObjectProperty ;
                          rdfs:domain :Property ;
                          rdfs:range :MISMOIndicator ;
                          rdfs:comment "When true, indicates that all dwellings on the property have been completed in the last 12 months, have a 100% new foundation, and have never been occupied."^^xsd:string ;
                          rdfs:label "New Construction Indicator"^^xsd:string .


###  http://mismo.org/Subset/nfip-CommunityFIRM-Date
:nfip-CommunityFIRM-Date rdf:type owl:ObjectProperty ;
                         rdfs:domain :FloodDetermination ;
                         rdfs:range :MISMODate ;
                         rdfs:comment "The date on which a community received its first Flood Insurance Rate Map. Used by Insurance companies to determine flood rates as to whether the structure is pre or post FIRM."^^xsd:string ;
                         rdfs:label "NFIP Community FIRM Date"^^xsd:string .


###  http://mismo.org/Subset/nfip-CommunityIdentifier
:nfip-CommunityIdentifier rdf:type owl:ObjectProperty ;
                          rdfs:domain :FloodDetermination ;
                          rdfs:range :MISMOIdentifier ;
                          rdfs:comment "The 6 digit NFIP community number."^^xsd:string ;
                          rdfs:label "NFIP Community Identifier"^^xsd:string .


###  http://mismo.org/Subset/nfip-CommunityName
:nfip-CommunityName rdf:type owl:ObjectProperty ;
                    rdfs:domain :FloodDetermination ;
                    rdfs:range :MISMOString ;
                    rdfs:comment "The complete name of the community in which the building or mobile home is located."^^xsd:string ;
                    rdfs:label "NFIP Community Name"^^xsd:string .


###  http://mismo.org/Subset/nfip-CommunityParticipationStartDate
:nfip-CommunityParticipationStartDate rdf:type owl:ObjectProperty ;
                                      rdfs:domain :FloodDetermination ;
                                      rdfs:range :MISMODate ;
                                      rdfs:comment "The date on which the community entered the Regular Program of the NFIP."^^xsd:string ;
                                      rdfs:label "NFIP Community Participation Start Date"^^xsd:string .


###  http://mismo.org/Subset/nfip-CommunityParticipationStatusType
:nfip-CommunityParticipationStatusType rdf:type owl:ObjectProperty ;
                                       rdfs:domain :FloodDetermination ;
                                       rdfs:range <http://mismo.org/EnumeratedTypes/NFIPCommunityParticipationStatusEnum> ;
                                       rdfs:comment "A code indicating the type of flood program."^^xsd:string ;
                                       rdfs:label "NFIP Community Participation Status Type"^^xsd:string .


###  http://mismo.org/Subset/nfip-CommunityParticipationStatusTypeOtherDescription
:nfip-CommunityParticipationStatusTypeOtherDescription rdf:type owl:ObjectProperty ;
                                                       rdfs:domain :FloodDetermination ;
                                                       rdfs:range :MISMOString ;
                                                       rdfs:comment "A free-form text field used to capture the NFIP Community Participation Status Type Other Description if Other is selected."^^xsd:string ;
                                                       rdfs:label "NFIP Community Participation Status Type Other Description"^^xsd:string .


###  http://mismo.org/Subset/nfip-CountyName
:nfip-CountyName rdf:type owl:ObjectProperty ;
                 rdfs:domain :FloodDetermination ;
                 rdfs:range :MISMOString ;
                 rdfs:comment "The name of the county or counties in which the community is located. In unincorporated areas of a county, this would be classified as: unincorporated areas. For independent cities, this would be classified as: independent city."^^xsd:string ;
                 rdfs:label "NFIP County Name"^^xsd:string .


###  http://mismo.org/Subset/nfip-FloodDataRevisionType
:nfip-FloodDataRevisionType rdf:type owl:ObjectProperty ;
                            rdfs:domain :FloodDetermination ;
                            rdfs:range <http://mismo.org/EnumeratedTypes/NFIPFloodDataRevisionEnum> ;
                            rdfs:comment "Letter of Map Amendment or Revision has been issued by FEMA."^^xsd:string ;
                            rdfs:label "NFIP Flood Data Revision Type"^^xsd:string .


###  http://mismo.org/Subset/nfip-FloodZoneIdentifier
:nfip-FloodZoneIdentifier rdf:type owl:ObjectProperty ;
                          rdfs:domain :FloodDetermination ;
                          rdfs:range :MISMOIdentifier ;
                          rdfs:comment "The flood zone covering the building or mobile home."^^xsd:string ;
                          rdfs:label "NFIP Flood Zone Identifier"^^xsd:string .


###  http://mismo.org/Subset/nfip-LetterOfMapDate
:nfip-LetterOfMapDate rdf:type owl:ObjectProperty ;
                      rdfs:domain :FloodDetermination ;
                      rdfs:range :MISMODate ;
                      rdfs:comment "The date the letter (LOMA /LOMR) was issued."^^xsd:string ;
                      rdfs:label "NFIP Letter Of Map Date"^^xsd:string .


###  http://mismo.org/Subset/nfip-MapIdentifier
:nfip-MapIdentifier rdf:type owl:ObjectProperty ;
                    rdfs:domain :FloodDetermination ;
                    rdfs:range :MISMOIdentifier ;
                    rdfs:comment "The 11-digit number shown on the NFIP map that covers the building or mobile home (Full concatenated version of the National Flood Community Identifier, NFIP Map Panel Identifier, NFIP Map Panel Suffix Identifier)."^^xsd:string ;
                    rdfs:label "NFIP Map Identifier"^^xsd:string .


###  http://mismo.org/Subset/nfip-MapIndicator
:nfip-MapIndicator rdf:type owl:ObjectProperty ;
                   rdfs:domain :FloodDetermination ;
                   rdfs:range :MISMOIndicator ;
                   rdfs:comment "Indicates if the NFIP map covers the area where the building or mobile home is located."^^xsd:string ;
                   rdfs:label "NFIP Map Indicator"^^xsd:string .


###  http://mismo.org/Subset/nfip-MapPanelDate
:nfip-MapPanelDate rdf:type owl:ObjectProperty ;
                   rdfs:domain :FloodDetermination ;
                   rdfs:range :MISMODate ;
                   rdfs:comment "The map effective date or the map revised date shown on the NFIP map."^^xsd:string ;
                   rdfs:label "NFIP Map Panel Date"^^xsd:string .


###  http://mismo.org/Subset/nfip-MapPanelIdentifier
:nfip-MapPanelIdentifier rdf:type owl:ObjectProperty ;
                         rdfs:domain :FloodDetermination ;
                         rdfs:range :MISMOIdentifier ;
                         rdfs:comment "The 4-digit number that describes the panel in which the property is located."^^xsd:string ;
                         rdfs:label "NFIP Map Panel Identifier"^^xsd:string .


###  http://mismo.org/Subset/nfip-MapPanelSuffixIdentifier
:nfip-MapPanelSuffixIdentifier rdf:type owl:ObjectProperty ;
                               rdfs:domain :FloodDetermination ;
                               rdfs:range :MISMOIdentifier ;
                               rdfs:comment "The letter that indicates the current map revision."^^xsd:string ;
                               rdfs:label "NFIP Map Panel Suffix Identifier"^^xsd:string .


###  http://mismo.org/Subset/nfip-StateCode
:nfip-StateCode rdf:type owl:ObjectProperty ;
                rdfs:domain :FloodDetermination ;
                rdfs:range <http://mismo.org/DataTypes/MISMOCode> ;
                rdfs:comment "The state in which the community is located, the two-digit state abbreviation."^^xsd:string ;
                rdfs:label "NFIP State Code"^^xsd:string .


###  http://mismo.org/Subset/openEndCreditIndicator
:openEndCreditIndicator rdf:type owl:ObjectProperty ;
                        rdfs:domain :Loan ;
                        rdfs:range :MISMOIndicator ;
                        rdfs:comment "When true, indicates that the loan or the application is for an open end loan, also known as a line of credit."^^xsd:string ;
                        rdfs:label "Open End Credit Indicator"^^xsd:string .


###  http://mismo.org/Subset/optionalProductSummary
:optionalProductSummary rdf:type owl:ObjectProperty ;
                        rdfs:domain :Loan ;
                        rdfs:range <http://mismo.org/Containers/OptionalProductSummary> ;
                        rdfs:comment "A collection of data points used to provide summary total(s) related to a single optional product or multiple optional products."^^xsd:string ;
                        rdfs:label "optional product summary"^^xsd:string .


###  http://mismo.org/Subset/optionalProducts
:optionalProducts rdf:type owl:ObjectProperty ;
                  rdfs:domain :Loan ;
                  rdfs:range <http://mismo.org/Containers/OptionalProduct> ;
                  rdfs:comment "Information about one or more OPTIONAL_PRODUCT. Holds all occurrences of OPTIONAL_PRODUCT."^^xsd:string ;
                  rdfs:label "optional products"^^xsd:string .


###  http://mismo.org/Subset/originalLoanStandardEscrowProvisionsIndicator
:originalLoanStandardEscrowProvisionsIndicator rdf:type owl:ObjectProperty ;
                                               rdfs:domain :Loan ;
                                               rdfs:range :MISMOIndicator ;
                                               rdfs:comment "When true indicates the original loan documents included standard Fannie Mae/Freddie Mac Uniform Instrument provisions for escrow items."^^xsd:string ;
                                               rdfs:label "Original Loan Standard Escrow Provisions Indicator"^^xsd:string .


###  http://mismo.org/Subset/originationFunds
:originationFunds rdf:type owl:ObjectProperty ;
                  rdfs:domain :Loan ;
                  rdfs:range <http://mismo.org/Containers/OriginationFund> ;
                  rdfs:comment "Information about one or more ORIGINATION_FUND. Holds all occurrences of ORIGINATION_FUND."^^xsd:string ;
                  rdfs:label "origination funds"^^xsd:string .


###  http://mismo.org/Subset/originationSystems
:originationSystems rdf:type owl:ObjectProperty ;
                    rdfs:domain :Loan ;
                    rdfs:range <http://mismo.org/Containers/OriginationSystem> ;
                    rdfs:comment "Information about one or more ORIGINATION_SYSTEM. Holds all occurrences of ORIGINATION_SYSTEM."^^xsd:string ;
                    rdfs:label "origination systems"^^xsd:string .


###  http://mismo.org/Subset/outbuildingCount
:outbuildingCount rdf:type owl:ObjectProperty ;
                  rdfs:domain :Property ;
                  rdfs:range <http://mismo.org/DataTypes/MISMOCount> ;
                  rdfs:comment "The total number of outbuildings (e.g., barn, shed, bunkhouse) that are considered real property."^^xsd:string ;
                  rdfs:label "Outbuilding Count"^^xsd:string .


###  http://mismo.org/Subset/overallConditionRatingCode
:overallConditionRatingCode rdf:type owl:ObjectProperty ;
                            rdfs:domain :Property ;
                            rdfs:range <http://mismo.org/DataTypes/MISMOCode> ;
                            rdfs:comment "An enumerated or coded value that represents the condition rating of all dwellings on the property utilized in the development of the opinion of value."^^xsd:string ;
                            rdfs:label "Overall Condition Rating Code"^^xsd:string .


###  http://mismo.org/Subset/overallQualityRatingCode
:overallQualityRatingCode rdf:type owl:ObjectProperty ;
                          rdfs:domain :Property ;
                          rdfs:range <http://mismo.org/DataTypes/MISMOCode> ;
                          rdfs:comment "An enumerated or coded value that represents the quality rating of all dwellings on the property utilized in the development of the opinion of value."^^xsd:string ;
                          rdfs:label "Overall Quality Rating Code"^^xsd:string .


###  http://mismo.org/Subset/overdueInterestAmount
:overdueInterestAmount rdf:type owl:ObjectProperty ;
                       rdfs:domain :Loan ;
                       rdfs:range :MISMOAmount ;
                       rdfs:comment "The dollar amount of interest accrued but not yet paid for Daily Simple Interest loans. This interest is considered overdue interest and is paid first when a payment is applied."^^xsd:string ;
                       rdfs:label "Overdue Interest Amount"^^xsd:string .


###  http://mismo.org/Subset/pace-LoanPayoffAmount
:pace-LoanPayoffAmount rdf:type owl:ObjectProperty ;
                       rdfs:domain :Loan ;
                       rdfs:range :MISMOAmount ;
                       rdfs:comment "The payoff amount of any existing Property Assessed Clean Energy (PACE) loans. These loans are made by localities to finance residential energy-related improvements and are generally repaid through the homeownerâs real estate tax bill."^^xsd:string ;
                       rdfs:label "PACE Loan Payoff Amount"^^xsd:string .


###  http://mismo.org/Subset/parcelSummary
:parcelSummary rdf:type owl:ObjectProperty ;
               rdfs:domain :Property ;
               rdfs:range <http://mismo.org/Containers/ParcelSummary> ;
               rdfs:comment "Contains summary level information about all parcels of land."^^xsd:string ;
               rdfs:label "parcel summary"^^xsd:string .


###  http://mismo.org/Subset/parcels
:parcels rdf:type owl:ObjectProperty ;
         rdfs:domain :Property ;
         rdfs:range <http://mismo.org/Containers/Parcel> ;
         rdfs:comment "Information about one or more parcel of land. Holds all occurrences of PARCEL."^^xsd:string .


###  http://mismo.org/Subset/parties
:parties rdf:type owl:ObjectProperty ;
         rdfs:domain [ rdf:type owl:Class ;
                       owl:unionOf ( :DealSequence
                                     :DealSet
                                     :FloodResponse
                                   )
                     ] ;
         rdfs:range <http://mismo.org/Containers/Party> ;
         rdfs:comment "A collection of objects that define specific parties to a deal. This includes the direct participating parties, such as borrower and seller and the indirect parties such as the credit report provider."^^xsd:string .


###  http://mismo.org/Subset/payment
:payment rdf:type owl:ObjectProperty ;
         rdfs:domain :Loan ;
         rdfs:range <http://mismo.org/Containers/Payment> ;
         rdfs:comment "Information regarding payments."^^xsd:string .


###  http://mismo.org/Subset/paymentIncreaseIndicator
:paymentIncreaseIndicator rdf:type owl:ObjectProperty ;
                          rdfs:domain :Loan ;
                          rdfs:range :MISMOIndicator ;
                          rdfs:comment "When true, indicates that the payments on the loan can increase after the closing."^^xsd:string ;
                          rdfs:label "Payment Increase Indicator"^^xsd:string .


###  http://mismo.org/Subset/piggybackLoanIndicator
:piggybackLoanIndicator rdf:type owl:ObjectProperty ;
                        rdfs:domain :Loan ;
                        rdfs:range :MISMOIndicator ;
                        rdfs:comment "Indicates a second lien being carried under the same loan number as a first mortgage. Generally one mortgage is covered by two notes and the borrower makes one combined payment."^^xsd:string ;
                        rdfs:label "Piggyback Loan Indicator"^^xsd:string .


###  http://mismo.org/Subset/plusFourZipCode
:plusFourZipCode rdf:type owl:ObjectProperty ;
                 rdfs:domain :Address ;
                 rdfs:range <http://mismo.org/DataTypes/MISMOCode> ;
                 rdfs:comment "This is the additional four digits in the code."^^xsd:string ;
                 rdfs:label "Plus Four Zip Code"^^xsd:string .


###  http://mismo.org/Subset/pool
:pool rdf:type owl:ObjectProperty ;
      rdfs:domain :DealSet ;
      rdfs:range :Pool ;
      rdfs:comment "Holds data on multiple loans transmitted as a pool."^^xsd:string .


###  http://mismo.org/Subset/poolAccrualRateStructureType
:poolAccrualRateStructureType rdf:type owl:ObjectProperty ;
                              rdfs:domain :Pool ;
                              rdfs:range <http://mismo.org/EnumeratedTypes/PoolAccrualRateStructureEnum> ;
                              rdfs:comment "Specifies the structure used to determine the accrual interest rate for the pool."^^xsd:string ;
                              rdfs:label "Pool Accrual Rate Structure Type"^^xsd:string .


###  http://mismo.org/Subset/poolAssumabilityIndicator
:poolAssumabilityIndicator rdf:type owl:ObjectProperty ;
                           rdfs:domain :Pool ;
                           rdfs:range :MISMOIndicator ;
                           rdfs:comment "Indicates whether the pool is backed by loans that are assumable by another borrower."^^xsd:string ;
                           rdfs:label "Pool Assumability Indicator"^^xsd:string .


###  http://mismo.org/Subset/poolBalloonIndicator
:poolBalloonIndicator rdf:type owl:ObjectProperty ;
                      rdfs:domain :Pool ;
                      rdfs:range :MISMOIndicator ;
                      rdfs:comment "Indicates whether or not the pool is backed by loans where a final balloon payment is required under the terms of the loan repayment schedule to fully pay off the loan."^^xsd:string ;
                      rdfs:label "Pool Balloon Indicator"^^xsd:string .


###  http://mismo.org/Subset/poolBidRequest
:poolBidRequest rdf:type owl:ObjectProperty ;
                rdfs:domain :DealSet ;
                rdfs:range <http://mismo.org/Containers/PoolBidRequest> ;
                rdfs:comment "Contains specific information pertaining to a Bid Wanted in Competition (BWIC) request for a pool of loans."^^xsd:string ;
                rdfs:label "pool bid request"^^xsd:string .


###  http://mismo.org/Subset/poolBidResponse
:poolBidResponse rdf:type owl:ObjectProperty ;
                 rdfs:domain :DealSet ;
                 rdfs:range <http://mismo.org/Containers/PoolBidResponse> ;
                 rdfs:comment "Contains specific information pertaining to a response received for a Bid Wanted in Competition (BWIC) request for a pool of loans."^^xsd:string ;
                 rdfs:label "pool bid response"^^xsd:string .


###  http://mismo.org/Subset/poolClassType
:poolClassType rdf:type owl:ObjectProperty ;
               rdfs:domain :Pool ;
               rdfs:range <http://mismo.org/EnumeratedTypes/PoolClassEnum> ;
               rdfs:comment "Indicates the type of pool and its guarantor (if any)."^^xsd:string ;
               rdfs:label "Pool Class Type"^^xsd:string .


###  http://mismo.org/Subset/poolClassTypeOtherDescription
:poolClassTypeOtherDescription rdf:type owl:ObjectProperty ;
                               rdfs:domain :Pool ;
                               rdfs:range :MISMOString ;
                               rdfs:comment "A free-form text field used to capture the Pool Class if Other is selected as the Pool Class Type."^^xsd:string ;
                               rdfs:label "Pool Class Type Other Description"^^xsd:string .


###  http://mismo.org/Subset/poolConcurrentTransferIndicator
:poolConcurrentTransferIndicator rdf:type owl:ObjectProperty ;
                                 rdfs:domain :Pool ;
                                 rdfs:range :MISMOIndicator ;
                                 rdfs:comment "When true, indicates that the pool will be immediately transferred upon pool issuance."^^xsd:string ;
                                 rdfs:label "Pool Concurrent Transfer Indicator"^^xsd:string .


###  http://mismo.org/Subset/poolCurrentLoanCount
:poolCurrentLoanCount rdf:type owl:ObjectProperty ;
                      rdfs:domain :Pool ;
                      rdfs:range <http://mismo.org/DataTypes/MISMOCount> ;
                      rdfs:comment "The current number of mortgages in the pool with principal balances as of the last cutoff."^^xsd:string ;
                      rdfs:label "Pool Current Loan Count"^^xsd:string .


###  http://mismo.org/Subset/poolCurrentPrincipalBalanceAmount
:poolCurrentPrincipalBalanceAmount rdf:type owl:ObjectProperty ;
                                   rdfs:domain :Pool ;
                                   rdfs:range :MISMOAmount ;
                                   rdfs:comment "Total dollar amount of the remaining unpaid principal balance for a pool of mortgages as of the last cutoff."^^xsd:string ;
                                   rdfs:label "Pool Current Principal Balance Amount"^^xsd:string .


###  http://mismo.org/Subset/poolFHA-LoanPercent
:poolFHA-LoanPercent rdf:type owl:ObjectProperty ;
                     rdfs:domain :Pool ;
                     rdfs:range <http://mismo.org/DataTypes/MISMOPercent> ;
                     rdfs:comment "A portion of 100 that represents the dollar amount of the pool that is insured by the Federal Housing Administration (FHA)."^^xsd:string ;
                     rdfs:label "Pool FHA Loan Percent"^^xsd:string .


###  http://mismo.org/Subset/poolFixedServicingFeePercent
:poolFixedServicingFeePercent rdf:type owl:ObjectProperty ;
                              rdfs:domain :Pool ;
                              rdfs:range <http://mismo.org/DataTypes/MISMOPercent> ;
                              rdfs:comment "The servicing fee to be used in determining the rate of interest that accrues on a mortgage backed security (MBS) pool that has a weighted-average structure based on a fixed servicing fee."^^xsd:string ;
                              rdfs:label "Pool Fixed Servicing Fee Percent"^^xsd:string .


###  http://mismo.org/Subset/poolGuarantyFeeRatePercent
:poolGuarantyFeeRatePercent rdf:type owl:ObjectProperty ;
                            rdfs:domain :Pool ;
                            rdfs:range <http://mismo.org/DataTypes/MISMOPercent> ;
                            rdfs:comment "The percentage of the guaranty fee rate that applies to loans in the pool that do not have a rate specified at the individual loan level."^^xsd:string ;
                            rdfs:label "Pool Guaranty Fee Rate Percent"^^xsd:string .


###  http://mismo.org/Subset/poolHighestPercentageStateCode
:poolHighestPercentageStateCode rdf:type owl:ObjectProperty ;
                                rdfs:domain :Pool ;
                                rdfs:range <http://mismo.org/DataTypes/MISMOCode> ;
                                rdfs:comment "A representation of the US state, US Territory, Canadian Province/Territory, or Military Address abbreviation (for example: AE, AP, AA) that represents the locations of the properties with the highest percentage of loans in the pool."^^xsd:string ;
                                rdfs:label "Pool Highest Percentage State Code"^^xsd:string .


###  http://mismo.org/Subset/poolHighestStateCodePercent
:poolHighestStateCodePercent rdf:type owl:ObjectProperty ;
                             rdfs:domain :Pool ;
                             rdfs:range <http://mismo.org/DataTypes/MISMOPercent> ;
                             rdfs:comment "A portion of 100 that represents the highest percentage of the loans in the pool in any single US state, US territory, Canadian Province/Territory, or Military Address in the pool."^^xsd:string ;
                             rdfs:label "Pool Highest State Code Percent"^^xsd:string .


###  http://mismo.org/Subset/poolIdentifier
:poolIdentifier rdf:type owl:ObjectProperty ;
                rdfs:domain [ rdf:type owl:Class ;
                              owl:unionOf ( :Loan
                                            :Pool
                                          )
                            ] ;
                rdfs:range :MISMOIdentifier ;
                rdfs:comment "The unique identifier for a group or pool of loans. May include relevant prefix and suffix when not parsed into applicable fields. See Pool Prefix Identifier or Pool Suffix Identifier."^^xsd:string ;
                rdfs:label "Pool Identifier"^^xsd:string .


###  http://mismo.org/Subset/poolInterestAdjustmentEffectiveDate
:poolInterestAdjustmentEffectiveDate rdf:type owl:ObjectProperty ;
                                     rdfs:domain :Pool ;
                                     rdfs:range :MISMODate ;
                                     rdfs:comment "The date the pool interest rate changes."^^xsd:string ;
                                     rdfs:label "Pool Interest Adjustment Effective Date"^^xsd:string .


###  http://mismo.org/Subset/poolInterestAdjustmentIndexLeadDaysCount
:poolInterestAdjustmentIndexLeadDaysCount rdf:type owl:ObjectProperty ;
                                          rdfs:domain :Pool ;
                                          rdfs:range <http://mismo.org/DataTypes/MISMOCount> ;
                                          rdfs:comment "The number of days prior to an interest rate effective date used to determine the date for the index value when calculating a new interest rate for a pool of loans."^^xsd:string ;
                                          rdfs:label "Pool Interest Adjustment Index Lead Days Count"^^xsd:string .


###  http://mismo.org/Subset/poolInterestAndPaymentAdjustmentIndexLeadDaysCount
:poolInterestAndPaymentAdjustmentIndexLeadDaysCount rdf:type owl:ObjectProperty ;
                                                    rdfs:domain :Pool ;
                                                    rdfs:range <http://mismo.org/DataTypes/MISMOCount> ;
                                                    rdfs:comment "The number of days prior to an interest rate effective date used to determine the date for the index value when calculating both a new interest rate and a principal and interest payment for a pool of loans."^^xsd:string ;
                                                    rdfs:label "Pool Interest And Payment Adjustment Index Lead Days Count"^^xsd:string .


###  http://mismo.org/Subset/poolInterestOnlyIndicator
:poolInterestOnlyIndicator rdf:type owl:ObjectProperty ;
                           rdfs:domain :Pool ;
                           rdfs:range :MISMOIndicator ;
                           rdfs:comment "Indicates whether a pool is backed by loans with interest only payments."^^xsd:string ;
                           rdfs:label "Pool Interest Only Indicator"^^xsd:string .


###  http://mismo.org/Subset/poolInterestRateRoundingPercent
:poolInterestRateRoundingPercent rdf:type owl:ObjectProperty ;
                                 rdfs:domain :Pool ;
                                 rdfs:range <http://mismo.org/DataTypes/MISMOPercent> ;
                                 rdfs:comment "The percentage to which the interest rate is rounded when a new interest rate is calculated for a pool. This field is used in conjunction with Pool Interest Rate Rounding Type which indicates how the rounding should occur."^^xsd:string ;
                                 rdfs:label "Pool Interest Rate Rounding Percent"^^xsd:string .


###  http://mismo.org/Subset/poolInterestRateRoundingType
:poolInterestRateRoundingType rdf:type owl:ObjectProperty ;
                              rdfs:domain :Pool ;
                              rdfs:range <http://mismo.org/EnumeratedTypes/PoolInterestRateRoundingEnum> ;
                              rdfs:comment "Indicates how the interest rate is rounded when a new interest rate is calculated for a pool of loans."^^xsd:string ;
                              rdfs:label "Pool Interest Rate Rounding Type"^^xsd:string .


###  http://mismo.org/Subset/poolInterestRateTruncatedDigitsCount
:poolInterestRateTruncatedDigitsCount rdf:type owl:ObjectProperty ;
                                      rdfs:domain :Pool ;
                                      rdfs:range <http://mismo.org/DataTypes/MISMOCount> ;
                                      rdfs:comment "Indicates the number of digits the interest rate should be truncated for a pool."^^xsd:string ;
                                      rdfs:label "Pool Interest Rate Truncated Digits Count"^^xsd:string .


###  http://mismo.org/Subset/poolInvestorAdditionalProductPlanIdentifier
:poolInvestorAdditionalProductPlanIdentifier rdf:type owl:ObjectProperty ;
                                             rdfs:domain :Pool ;
                                             rdfs:range :MISMOIdentifier ;
                                             rdfs:comment "A unique alphanumeric string identifying an optional additional product plan."^^xsd:string ;
                                             rdfs:label "Pool Investor Additional Product Plan Identifier"^^xsd:string .


###  http://mismo.org/Subset/poolInvestorProductPlanIdentifier
:poolInvestorProductPlanIdentifier rdf:type owl:ObjectProperty ;
                                   rdfs:domain :Pool ;
                                   rdfs:range :MISMOIdentifier ;
                                   rdfs:comment "Identifies the plan of the varying loan payment and/or rate change characteristics for a pool of loans issued by the servicer."^^xsd:string ;
                                   rdfs:label "Pool Investor Product Plan Identifier"^^xsd:string .


###  http://mismo.org/Subset/poolIssueDate
:poolIssueDate rdf:type owl:ObjectProperty ;
               rdfs:domain [ rdf:type owl:Class ;
                             owl:unionOf ( :Loan
                                           :Pool
                                         )
                           ] ;
               rdfs:range :MISMODate ;
               rdfs:comment "The date a mortgage backed security is issued to investors."^^xsd:string ;
               rdfs:label "Pool Issue Date"^^xsd:string .


###  http://mismo.org/Subset/poolIssuerIdentifier
:poolIssuerIdentifier rdf:type owl:ObjectProperty ;
                      rdfs:domain :Pool ;
                      rdfs:range :MISMOIdentifier ;
                      rdfs:comment "Identification number assigned by pool guarantor to the Issuer or current servicer of the pool."^^xsd:string ;
                      rdfs:label "Pool Issuer Identifier"^^xsd:string .


###  http://mismo.org/Subset/poolMarginRatePercent
:poolMarginRatePercent rdf:type owl:ObjectProperty ;
                       rdfs:domain :Pool ;
                       rdfs:range <http://mismo.org/DataTypes/MISMOPercent> ;
                       rdfs:comment "The factor that is added to the ARM index value to calculate the pool accrual rate."^^xsd:string ;
                       rdfs:label "Pool Margin Rate Percent"^^xsd:string .


###  http://mismo.org/Subset/poolMaturityDate
:poolMaturityDate rdf:type owl:ObjectProperty ;
                  rdfs:domain :Pool ;
                  rdfs:range :MISMODate ;
                  rdfs:comment "The date the final payment is due on the pool. The pool maturity date is typically 15 to 45 days after the maturity date of the latest maturing mortgage in the mortgage-backed security."^^xsd:string ;
                  rdfs:label "Pool Maturity Date"^^xsd:string .


###  http://mismo.org/Subset/poolMaximumAccrualRatePercent
:poolMaximumAccrualRatePercent rdf:type owl:ObjectProperty ;
                               rdfs:domain :Pool ;
                               rdfs:range <http://mismo.org/DataTypes/MISMOPercent> ;
                               rdfs:comment "The maximum rate, expressed as a percent, at which interest can accrue on a pool."^^xsd:string ;
                               rdfs:label "Pool Maximum Accrual Rate Percent"^^xsd:string .


###  http://mismo.org/Subset/poolMinimumAccrualRatePercent
:poolMinimumAccrualRatePercent rdf:type owl:ObjectProperty ;
                               rdfs:domain :Pool ;
                               rdfs:range <http://mismo.org/DataTypes/MISMOPercent> ;
                               rdfs:comment "The minimum rate, expressed as a percent, at which interest can accrue on a pool."^^xsd:string ;
                               rdfs:label "Pool Minimum Accrual Rate Percent"^^xsd:string .


###  http://mismo.org/Subset/poolModificationLoanPercent
:poolModificationLoanPercent rdf:type owl:ObjectProperty ;
                             rdfs:domain :Pool ;
                             rdfs:range <http://mismo.org/DataTypes/MISMOPercent> ;
                             rdfs:comment "A portion of 100 that represents the dollar amount of modified loans in the pool."^^xsd:string ;
                             rdfs:label "Pool Modification Loan Percent"^^xsd:string .


###  http://mismo.org/Subset/poolMortgageRatePercent
:poolMortgageRatePercent rdf:type owl:ObjectProperty ;
                         rdfs:domain :Pool ;
                         rdfs:range <http://mismo.org/DataTypes/MISMOPercent> ;
                         rdfs:comment "The annual interest rate, expressed as a percent, of the mortgages in a pool as of last cutoff date."^^xsd:string ;
                         rdfs:label "Pool Mortgage Rate Percent"^^xsd:string .


###  http://mismo.org/Subset/poolMortgageType
:poolMortgageType rdf:type owl:ObjectProperty ;
                  rdfs:domain :Pool ;
                  rdfs:range <http://mismo.org/EnumeratedTypes/PoolMortgageEnum> ;
                  rdfs:comment "Specifies mortgage type of the loans for the pool."^^xsd:string ;
                  rdfs:label "Pool Mortgage Type"^^xsd:string .


###  http://mismo.org/Subset/poolMortgageTypeOtherDescription
:poolMortgageTypeOtherDescription rdf:type owl:ObjectProperty ;
                                  rdfs:domain :Pool ;
                                  rdfs:range :MISMOString ;
                                  rdfs:comment "A free-form text field used to collect additional information or a description of the mortgage type when Other is selected for Pool Mortgage Type."^^xsd:string ;
                                  rdfs:label "Pool Mortgage Type Other Description"^^xsd:string .


###  http://mismo.org/Subset/poolNonTPO-LoanPercent
:poolNonTPO-LoanPercent rdf:type owl:ObjectProperty ;
                        rdfs:domain :Pool ;
                        rdfs:range <http://mismo.org/DataTypes/MISMOPercent> ;
                        rdfs:comment "A portion of 100 that represents the dollar amount of the pool that is originated by a third party."^^xsd:string ;
                        rdfs:label "Pool Non TPO Loan Percent"^^xsd:string .


###  http://mismo.org/Subset/poolOriginalLoanCount
:poolOriginalLoanCount rdf:type owl:ObjectProperty ;
                       rdfs:domain :Pool ;
                       rdfs:range <http://mismo.org/DataTypes/MISMOCount> ;
                       rdfs:comment "The total number of loans in the pool when the pool was set up."^^xsd:string ;
                       rdfs:label "Pool Original Loan Count"^^xsd:string .


###  http://mismo.org/Subset/poolOriginalPrincipalBalanceAmount
:poolOriginalPrincipalBalanceAmount rdf:type owl:ObjectProperty ;
                                    rdfs:domain :Pool ;
                                    rdfs:range :MISMOAmount ;
                                    rdfs:comment "The total of the original principal balance of all the loans in the pool. For participations the principal balance contributed for an individual loan is adjusted based upon the participation percent."^^xsd:string ;
                                    rdfs:label "Pool Original Principal Balance Amount"^^xsd:string .


###  http://mismo.org/Subset/poolOwnershipPercent
:poolOwnershipPercent rdf:type owl:ObjectProperty ;
                      rdfs:domain :Pool ;
                      rdfs:range <http://mismo.org/DataTypes/MISMOPercent> ;
                      rdfs:comment "Identifies the percentage amount of the pool owned by the investor."^^xsd:string ;
                      rdfs:label "Pool Ownership Percent"^^xsd:string .


###  http://mismo.org/Subset/poolPrefixIdentifier
:poolPrefixIdentifier rdf:type owl:ObjectProperty ;
                      rdfs:domain [ rdf:type owl:Class ;
                                    owl:unionOf ( :Loan
                                                  :Pool
                                                )
                                  ] ;
                      rdfs:range :MISMOIdentifier ;
                      rdfs:comment "The prefix associated with the pool identifier."^^xsd:string ;
                      rdfs:label "Pool Prefix Identifier"^^xsd:string .


###  http://mismo.org/Subset/poolPriorPeriodPrincipalBalanceAmount
:poolPriorPeriodPrincipalBalanceAmount rdf:type owl:ObjectProperty ;
                                       rdfs:domain :Pool ;
                                       rdfs:range :MISMOAmount ;
                                       rdfs:comment "The dollar amount of the outstanding principal balance, reported in the prior period, for the loans in the pool."^^xsd:string ;
                                       rdfs:label "Pool Prior Period Principal Balance Amount"^^xsd:string .


###  http://mismo.org/Subset/poolPurchaseLoanPercent
:poolPurchaseLoanPercent rdf:type owl:ObjectProperty ;
                         rdfs:domain :Pool ;
                         rdfs:range <http://mismo.org/DataTypes/MISMOPercent> ;
                         rdfs:comment "A portion of 100 that represents the dollar amount of the pool that represents purchase mortgages."^^xsd:string ;
                         rdfs:label "Pool Purchase Loan Percent"^^xsd:string .


###  http://mismo.org/Subset/poolScheduledPrincipalAndInterestPaymentAmount
:poolScheduledPrincipalAndInterestPaymentAmount rdf:type owl:ObjectProperty ;
                                                rdfs:domain :Pool ;
                                                rdfs:range :MISMOAmount ;
                                                rdfs:comment "Total scheduled dollar amount of the principal and interest payments of the underlying loans as of the last cutoff date."^^xsd:string ;
                                                rdfs:label "Pool Scheduled Principal And Interest Payment Amount"^^xsd:string .


###  http://mismo.org/Subset/poolScheduledPrincipalBalanceAmount
:poolScheduledPrincipalBalanceAmount rdf:type owl:ObjectProperty ;
                                     rdfs:domain :Pool ;
                                     rdfs:range :MISMOAmount ;
                                     rdfs:comment "The dollar amount of the scheduled principal balance of the loans in the pool amortized through the date when the activity report is made."^^xsd:string ;
                                     rdfs:label "Pool Scheduled Principal Balance Amount"^^xsd:string .


###  http://mismo.org/Subset/poolScheduledRemittancePaymentDay
:poolScheduledRemittancePaymentDay rdf:type owl:ObjectProperty ;
                                   rdfs:domain :Pool ;
                                   rdfs:range <http://mismo.org/DataTypes/MISMODay> ;
                                   rdfs:comment "Indicates the day of the month the servicer must remit the scheduled pass through payment to the certificate holders of a particular pool."^^xsd:string ;
                                   rdfs:label "Pool Scheduled Remittance Payment Day"^^xsd:string .


###  http://mismo.org/Subset/poolSecurityInterestRatePercent
:poolSecurityInterestRatePercent rdf:type owl:ObjectProperty ;
                                 rdfs:domain :Pool ;
                                 rdfs:range <http://mismo.org/DataTypes/MISMOPercent> ;
                                 rdfs:comment "The security interest rate, expressed as a percent, for the pool as of last cutoff date."^^xsd:string ;
                                 rdfs:label "Pool Security Interest Rate Percent"^^xsd:string .


###  http://mismo.org/Subset/poolSecurityIssueDateInterestRatePercent
:poolSecurityIssueDateInterestRatePercent rdf:type owl:ObjectProperty ;
                                          rdfs:domain :Pool ;
                                          rdfs:range <http://mismo.org/DataTypes/MISMOPercent> ;
                                          rdfs:comment "The security interest rate, expressed as a percent, for the pool as of the security issue date."^^xsd:string ;
                                          rdfs:label "Pool Security Issue Date Interest Rate Percent"^^xsd:string .


###  http://mismo.org/Subset/poolSecurityParValueAmount
:poolSecurityParValueAmount rdf:type owl:ObjectProperty ;
                            rdfs:domain :Pool ;
                            rdfs:range :MISMOAmount ;
                            rdfs:comment "The dollar amount of a securityâs par value or the actual selling price that an issuer contracts to repay."^^xsd:string ;
                            rdfs:label "Pool Security Par Value Amount"^^xsd:string .


###  http://mismo.org/Subset/poolSecuritySettlementDate
:poolSecuritySettlementDate rdf:type owl:ObjectProperty ;
                            rdfs:domain :Pool ;
                            rdfs:range :MISMODate ;
                            rdfs:comment "The date that parties enter into an agreement for the purchase or sale of mortgage-backed securities."^^xsd:string ;
                            rdfs:label "Pool Security Settlement Date"^^xsd:string .


###  http://mismo.org/Subset/poolServiceFeeRatePercent
:poolServiceFeeRatePercent rdf:type owl:ObjectProperty ;
                           rdfs:domain :Pool ;
                           rdfs:range <http://mismo.org/DataTypes/MISMOPercent> ;
                           rdfs:comment "The annualized rate, expressed as a percent, used to compute the fee paid to the servicer as of the last cutoff date."^^xsd:string ;
                           rdfs:label "Pool Service Fee Rate Percent"^^xsd:string .


###  http://mismo.org/Subset/poolStructureType
:poolStructureType rdf:type owl:ObjectProperty ;
                   rdfs:domain :Pool ;
                   rdfs:range <http://mismo.org/EnumeratedTypes/PoolStructureEnum> ;
                   rdfs:comment "Denotes the type of mortgage backed security structure."^^xsd:string ;
                   rdfs:label "Pool Structure Type"^^xsd:string .


###  http://mismo.org/Subset/poolStructureTypeOtherDescription
:poolStructureTypeOtherDescription rdf:type owl:ObjectProperty ;
                                   rdfs:domain :Pool ;
                                   rdfs:range :MISMOString ;
                                   rdfs:comment "A free-form text field used to collect additional information when Other is selected for Pool Structure Type."^^xsd:string ;
                                   rdfs:label "Pool Structure Type Other Description"^^xsd:string .


###  http://mismo.org/Subset/poolSuffixIdentifier
:poolSuffixIdentifier rdf:type owl:ObjectProperty ;
                      rdfs:domain :Pool ;
                      rdfs:range :MISMOIdentifier ;
                      rdfs:comment "Suffix associated with the pool identifier."^^xsd:string ;
                      rdfs:label "Pool Suffix Identifier"^^xsd:string .


###  http://mismo.org/Subset/poolUSDA-LoanPercent
:poolUSDA-LoanPercent rdf:type owl:ObjectProperty ;
                      rdfs:domain :Pool ;
                      rdfs:range <http://mismo.org/DataTypes/MISMOPercent> ;
                      rdfs:comment "A portion of 100 that represents the dollar amount of the pool that is guaranteed by the United States Department of Agriculture (USDA)."^^xsd:string ;
                      rdfs:label "Pool USDA Loan Percent"^^xsd:string .


###  http://mismo.org/Subset/poolUnscheduledPrincipalAmount
:poolUnscheduledPrincipalAmount rdf:type owl:ObjectProperty ;
                                rdfs:domain :Pool ;
                                rdfs:range :MISMOAmount ;
                                rdfs:comment "The dollar amount of the unscheduled principal paid, for the current reporting period, of the loans in the pool."^^xsd:string ;
                                rdfs:label "Pool Unscheduled Principal Amount"^^xsd:string .


###  http://mismo.org/Subset/poolUnscheduledPrincipalPaymentDay
:poolUnscheduledPrincipalPaymentDay rdf:type owl:ObjectProperty ;
                                    rdfs:domain :Pool ;
                                    rdfs:range <http://mismo.org/DataTypes/MISMODay> ;
                                    rdfs:comment "Indicates the day of the month the servicer must remit unscheduled principal payments to the certificate holders of a particular pool if they are to be remitted sooner than the scheduled remittance day."^^xsd:string ;
                                    rdfs:label "Pool Unscheduled Principal Payment Day"^^xsd:string .


###  http://mismo.org/Subset/poolVA-LoanPercent
:poolVA-LoanPercent rdf:type owl:ObjectProperty ;
                    rdfs:domain :Pool ;
                    rdfs:range <http://mismo.org/DataTypes/MISMOPercent> ;
                    rdfs:comment "A portion of 100 that represents the dollar amount of the pool that is guaranteed by the Veterans Administration (VA)."^^xsd:string ;
                    rdfs:label "Pool VA Loan Percent"^^xsd:string .


###  http://mismo.org/Subset/poolWeightedAverageCombinedLTV-RatioPercent
:poolWeightedAverageCombinedLTV-RatioPercent rdf:type owl:ObjectProperty ;
                                             rdfs:domain :Pool ;
                                             rdfs:range <http://mismo.org/DataTypes/MISMOPercent> ;
                                             rdfs:comment "A portion of 100 that represents the weighted average of the Combined Loan to Value ratio (CLTV) of the pool, with the UPB of each mortgage used as a weighting factor."^^xsd:string ;
                                             rdfs:label "Pool Weighted Average Combined LTV Ratio Percent"^^xsd:string .


###  http://mismo.org/Subset/poolWeightedAverageCouponRatePercent
:poolWeightedAverageCouponRatePercent rdf:type owl:ObjectProperty ;
                                      rdfs:domain :Pool ;
                                      rdfs:range <http://mismo.org/DataTypes/MISMOPercent> ;
                                      rdfs:comment "A portion of 100 that represents the weighted average of the gross interest rates of the mortgages in a pool, as of the issue date, with the UPB of each mortgage used as a weighting factor."^^xsd:string ;
                                      rdfs:label "Pool Weighted Average Coupon Rate Percent"^^xsd:string .


###  http://mismo.org/Subset/poolWeightedAverageCreditScoreValue
:poolWeightedAverageCreditScoreValue rdf:type owl:ObjectProperty ;
                                     rdfs:domain :Pool ;
                                     rdfs:range <http://mismo.org/DataTypes/MISMOValue> ;
                                     rdfs:comment "The specific value of the weighted average credit score of the pool, with the UPB of each mortgage used as a weighting factor."^^xsd:string ;
                                     rdfs:label "Pool Weighted Average Credit Score Value"^^xsd:string .


###  http://mismo.org/Subset/poolWeightedAverageLTV-RatioPercent
:poolWeightedAverageLTV-RatioPercent rdf:type owl:ObjectProperty ;
                                     rdfs:domain :Pool ;
                                     rdfs:range <http://mismo.org/DataTypes/MISMOPercent> ;
                                     rdfs:comment "A portion of 100 that represents the weighted average of the Loan to Value (LTV) ratio of the pool, with the UPB of each mortgage used as a weighting factor."^^xsd:string ;
                                     rdfs:label "Pool Weighted Average LTV Ratio Percent"^^xsd:string .


###  http://mismo.org/Subset/poolWeightedAverageOriginalUnpaidLoanBalanceAmount
:poolWeightedAverageOriginalUnpaidLoanBalanceAmount rdf:type owl:ObjectProperty ;
                                                    rdfs:domain :Pool ;
                                                    rdfs:range :MISMOAmount ;
                                                    rdfs:comment "The weighted average UPB amount of the mortgages in a pool, as of the issue date, with the UPB of each mortgage used as a weighting factor."^^xsd:string ;
                                                    rdfs:label "Pool Weighted Average Original Unpaid Loan Balance Amount"^^xsd:string .


###  http://mismo.org/Subset/poolingMethodType
:poolingMethodType rdf:type owl:ObjectProperty ;
                   rdfs:domain :Pool ;
                   rdfs:range <http://mismo.org/EnumeratedTypes/PoolingMethodEnum> ;
                   rdfs:comment "Indicates the timing of the remittance of the scheduled principal and interest payment from the servicer to the certificate holders of a particular pool."^^xsd:string ;
                   rdfs:label "Pooling Method Type"^^xsd:string .


###  http://mismo.org/Subset/poolingMethodTypeOtherDescription
:poolingMethodTypeOtherDescription rdf:type owl:ObjectProperty ;
                                   rdfs:domain :Pool ;
                                   rdfs:range :MISMOString ;
                                   rdfs:comment "A free-form text field used to capture the Pooling Method Type if Other is selected."^^xsd:string ;
                                   rdfs:label "Pooling Method Type Other Description"^^xsd:string .


###  http://mismo.org/Subset/positionOnePoolBidAmount
:positionOnePoolBidAmount rdf:type owl:ObjectProperty ;
                          rdfs:domain :Pool ;
                          rdfs:range :MISMOAmount ;
                          rdfs:comment "The dollar amount of the winning bid received by the Originator. This value is distributed after the BWIC process is over and the originator provides feedback to the dealer."^^xsd:string ;
                          rdfs:label "Position One Pool Bid Amount"^^xsd:string .


###  http://mismo.org/Subset/positionTwoPoolBidAmount
:positionTwoPoolBidAmount rdf:type owl:ObjectProperty ;
                          rdfs:domain :Pool ;
                          rdfs:range :MISMOAmount ;
                          rdfs:comment "The dollar amount of the second highest bid received by the Originator. This value is distributed after the BWIC process is over and the originator provides feedback to the dealer."^^xsd:string ;
                          rdfs:label "Position Two Pool Bid Amount"^^xsd:string .


###  http://mismo.org/Subset/postOfficeBoxIdentifier
:postOfficeBoxIdentifier rdf:type owl:ObjectProperty ;
                         rdfs:domain :Address ;
                         rdfs:range :MISMOIdentifier ;
                         rdfs:comment "The identifier of the locked box located in the post office lobby or other authorized place that customers may rent for delivery of mail."^^xsd:string ;
                         rdfs:label "Post Office Box Identifier"^^xsd:string .


###  http://mismo.org/Subset/postalCode
:postalCode rdf:type owl:ObjectProperty ;
            rdfs:domain :Address ;
            rdfs:range <http://mismo.org/DataTypes/MISMOCode> ;
            rdfs:comment "The postal code (ZIP Code in the US) for the address. ZIP Code may be either 5 or 9 digits."^^xsd:string ;
            rdfs:label "Postal Code"^^xsd:string .


###  http://mismo.org/Subset/prepaymentPenalty
:prepaymentPenalty rdf:type owl:ObjectProperty ;
                   rdfs:domain :Loan ;
                   rdfs:range <http://mismo.org/Containers/PrepaymentPenalty> ;
                   rdfs:comment "Information specific to calculation of penalties for partial or full principal re-payment prior to Loan Maturity."^^xsd:string ;
                   rdfs:label "prepayment penalty"^^xsd:string .


###  http://mismo.org/Subset/prepaymentPenaltyIndicator
:prepaymentPenaltyIndicator rdf:type owl:ObjectProperty ;
                            rdfs:domain :Loan ;
                            rdfs:range :MISMOIndicator ;
                            rdfs:comment "Indicates whether the loan includes a penalty charged to the borrower in the event of prepayment."^^xsd:string ;
                            rdfs:label "Prepayment Penalty Indicator"^^xsd:string .


###  http://mismo.org/Subset/prepaymentPenaltyWaivedIndicator
:prepaymentPenaltyWaivedIndicator rdf:type owl:ObjectProperty ;
                                  rdfs:domain :Loan ;
                                  rdfs:range :MISMOIndicator ;
                                  rdfs:comment "Indicates that the prepayment penalty has been waived."^^xsd:string ;
                                  rdfs:label "Prepayment Penalty Waived Indicator"^^xsd:string .


###  http://mismo.org/Subset/prepaymentRestrictionIndicator
:prepaymentRestrictionIndicator rdf:type owl:ObjectProperty ;
                                rdfs:domain :Loan ;
                                rdfs:range :MISMOIndicator ;
                                rdfs:comment "Indicates whether the loan has any restrictions on the prepayment of the loan (i.e. paying off the principal and or interest at a rate faster than prescribed by the payment schedule)."^^xsd:string ;
                                rdfs:label "Prepayment Restriction Indicator"^^xsd:string .


###  http://mismo.org/Subset/priorSaleInLastTwelveMonthsIndicator
:priorSaleInLastTwelveMonthsIndicator rdf:type owl:ObjectProperty ;
                                      rdfs:domain :Property ;
                                      rdfs:range :MISMOIndicator ;
                                      rdfs:comment "Indicates that property has been sold in the twelve months prior to origination of the delivery loan."^^xsd:string ;
                                      rdfs:label "Prior Sale In Last Twelve Months Indicator"^^xsd:string .


###  http://mismo.org/Subset/priorSalesOrTransfersIndicator
:priorSalesOrTransfersIndicator rdf:type owl:ObjectProperty ;
                                rdfs:domain :Property ;
                                rdfs:range :MISMOIndicator ;
                                rdfs:comment "When true, indicates that the property has a prior sale or transfer history included within the reporting period."^^xsd:string ;
                                rdfs:label "Prior Sales Or Transfers Indicator"^^xsd:string .


###  http://mismo.org/Subset/proRataSharePercent
:proRataSharePercent rdf:type owl:ObjectProperty ;
                     rdfs:domain :Property ;
                     rdfs:range <http://mismo.org/DataTypes/MISMOPercent> ;
                     rdfs:comment "A portion of 100 that represents the blanket mortgage payments that are attributable to the subject property, as determined by dividing the number of shares attributable to the subject property by the total number of project shares."^^xsd:string ;
                     rdfs:label "Pro Rata Share Percent"^^xsd:string .


###  http://mismo.org/Subset/project
:project rdf:type owl:ObjectProperty ;
         rdfs:domain :Property ;
         rdfs:range <http://mismo.org/Containers/Project> ;
         rdfs:comment "A residential development area that could be comprised of any combination of multifamily and single family structures and may include mixed land use such as commercial. A project refers to an organized development in which shared common areas, road ways and management structures exist. Project management and individual homeowner associations may also co-exist within the project."^^xsd:string .


###  http://mismo.org/Subset/propertiesFinancedByLenderCount
:propertiesFinancedByLenderCount rdf:type owl:ObjectProperty ;
                                 rdfs:domain :Loan ;
                                 rdfs:range <http://mismo.org/DataTypes/MISMOCount> ;
                                 rdfs:comment "Case or loan level count of properties already financed by this lender for the borrower(s) named on the loan application. Does not include subject property."^^xsd:string ;
                                 rdfs:label "Properties Financed By Lender Count"^^xsd:string .


###  http://mismo.org/Subset/property
:property rdf:type owl:ObjectProperty ;
          rdfs:domain :FloodResponse ;
          rdfs:range :Property ;
          rdfs:comment "Information specific to a real estate in terms of land structure, location and market."^^xsd:string .


###  http://mismo.org/Subset/propertyAcquiredDate
:propertyAcquiredDate rdf:type owl:ObjectProperty ;
                      rdfs:domain :Property ;
                      rdfs:range :MISMODate ;
                      rdfs:comment "The date the property was acquired."^^xsd:string ;
                      rdfs:label "Property Acquired Date"^^xsd:string .


###  http://mismo.org/Subset/propertyAcquiredYear
:propertyAcquiredYear rdf:type owl:ObjectProperty ;
                      rdfs:domain :Property ;
                      rdfs:range <http://mismo.org/DataTypes/MISMOYear> ;
                      rdfs:comment "The year in which the land and buildings of the property were acquired by the borrower."^^xsd:string ;
                      rdfs:label "Property Acquired Year"^^xsd:string .


###  http://mismo.org/Subset/propertyAcreageNumber
:propertyAcreageNumber rdf:type owl:ObjectProperty ;
                       rdfs:domain :Property ;
                       rdfs:range <http://mismo.org/DataTypes/MISMONumeric> ;
                       rdfs:comment "Number of acres of the subject property."^^xsd:string ;
                       rdfs:label "Property Acreage Number"^^xsd:string .


###  http://mismo.org/Subset/propertyAmenity
:propertyAmenity rdf:type owl:ObjectProperty ;
                 rdfs:domain :Property ;
                 rdfs:range <http://mismo.org/Containers/PropertyAmenity> ;
                 rdfs:comment "Contains information about one or more amenities located on the property."^^xsd:string ;
                 rdfs:label "property amenity"^^xsd:string .


###  http://mismo.org/Subset/propertyAmenityExistsIndicator
:propertyAmenityExistsIndicator rdf:type owl:ObjectProperty ;
                                rdfs:domain :Property ;
                                rdfs:range :MISMOIndicator ;
                                rdfs:comment "When true, indicates that the property has one or more amenities available."^^xsd:string ;
                                rdfs:label "Property Amenity Exists Indicator"^^xsd:string .


###  http://mismo.org/Subset/propertyConditionDescription
:propertyConditionDescription rdf:type owl:ObjectProperty ;
                              rdfs:domain :Property ;
                              rdfs:range :MISMOString ;
                              rdfs:comment "A free-form text field describing the condition of the property."^^xsd:string ;
                              rdfs:label "Property Condition Description"^^xsd:string .


###  http://mismo.org/Subset/propertyCooperativeSharesCount
:propertyCooperativeSharesCount rdf:type owl:ObjectProperty ;
                                rdfs:domain :Property ;
                                rdfs:range <http://mismo.org/DataTypes/MISMOCount> ;
                                rdfs:comment "The number of cooperative shares attributed to the property."^^xsd:string ;
                                rdfs:label "Property Cooperative Shares Count"^^xsd:string .


###  http://mismo.org/Subset/propertyCurrentOccupancyType
:propertyCurrentOccupancyType rdf:type owl:ObjectProperty ;
                              rdfs:domain :Property ;
                              rdfs:range <http://mismo.org/EnumeratedTypes/PropertyCurrentOccupancyEnum> ;
                              rdfs:comment "Specifies the property occupancy status of a subject property."^^xsd:string ;
                              rdfs:label "Property Current Occupancy Type"^^xsd:string .


###  http://mismo.org/Subset/propertyCurrentOccupantName
:propertyCurrentOccupantName rdf:type owl:ObjectProperty ;
                             rdfs:domain :Property ;
                             rdfs:range :MISMOString ;
                             rdfs:comment "The unparsed name of the current occupant of the property."^^xsd:string ;
                             rdfs:label "Property Current Occupant Name"^^xsd:string .


###  http://mismo.org/Subset/propertyDefect
:propertyDefect rdf:type owl:ObjectProperty ;
                rdfs:domain :Property ;
                rdfs:range <http://mismo.org/Containers/PropertyDefect> ;
                rdfs:comment "Contains information about one or more defect, damage and/or deficiency that has been observed on the property."^^xsd:string ;
                rdfs:label "property defect"^^xsd:string .


###  http://mismo.org/Subset/propertyDispositionStatusType
:propertyDispositionStatusType rdf:type owl:ObjectProperty ;
                               rdfs:domain :Property ;
                               rdfs:range <http://mismo.org/EnumeratedTypes/PropertyDispositionStatusEnum> ;
                               rdfs:comment "The intended disposition of the property."^^xsd:string ;
                               rdfs:label "Property Disposition Status Type"^^xsd:string .


###  http://mismo.org/Subset/propertyDispositionStatusTypeOtherDescription
:propertyDispositionStatusTypeOtherDescription rdf:type owl:ObjectProperty ;
                                               rdfs:domain :Property ;
                                               rdfs:range :MISMOString ;
                                               rdfs:comment "A free-form text field used to collect additional information when Other is selected for Property Disposition Status Type."^^xsd:string ;
                                               rdfs:label "Property Disposition Status Type Other Description"^^xsd:string .


###  http://mismo.org/Subset/propertyEarthquakeInsuranceIndicator
:propertyEarthquakeInsuranceIndicator rdf:type owl:ObjectProperty ;
                                      rdfs:domain :Property ;
                                      rdfs:range :MISMOIndicator ;
                                      rdfs:comment "An indicator denoting whether the property securing the mortgage has earthquake insurance."^^xsd:string ;
                                      rdfs:label "Property Earthquake Insurance Indicator"^^xsd:string .


###  http://mismo.org/Subset/propertyElevationLinearMeasure
:propertyElevationLinearMeasure rdf:type owl:ObjectProperty ;
                                rdfs:domain :FloodRiskFactor ;
                                rdfs:range <http://mismo.org/DataTypes/MISMOLinearMeasure> ;
                                rdfs:comment "A measurement that specifies the ground elevation in relation to sea level for a particular property.The applicable unit of measurement is specified by the Linear Unit Of Measure Type."^^xsd:string ;
                                rdfs:label "Property Elevation Linear Measure"^^xsd:string .


###  http://mismo.org/Subset/propertyEstateType
:propertyEstateType rdf:type owl:ObjectProperty ;
                    rdfs:domain :Property ;
                    rdfs:range <http://mismo.org/EnumeratedTypes/PropertyEstateEnum> ;
                    rdfs:comment "A value from a MISMO prescribed list that specifies the ownership interest in the property."^^xsd:string ;
                    rdfs:label "Property Estate Type"^^xsd:string .


###  http://mismo.org/Subset/propertyEstateTypeOtherDescription
:propertyEstateTypeOtherDescription rdf:type owl:ObjectProperty ;
                                    rdfs:domain :Property ;
                                    rdfs:range :MISMOString ;
                                    rdfs:comment "A free-form text field used to collect additional information when Other is selected for Property Estate Type."^^xsd:string ;
                                    rdfs:label "Property Estate Type Other Description"^^xsd:string .


###  http://mismo.org/Subset/propertyEstimatedValueAmount
:propertyEstimatedValueAmount rdf:type owl:ObjectProperty ;
                              rdfs:domain :Property ;
                              rdfs:range :MISMOAmount ;
                              rdfs:comment "A statement of the estimated present market value of the property that is from the borrower or loan originator."^^xsd:string ;
                              rdfs:label "Property Estimated Value Amount"^^xsd:string .


###  http://mismo.org/Subset/propertyExistingCleanEnergyLienIndicator
:propertyExistingCleanEnergyLienIndicator rdf:type owl:ObjectProperty ;
                                          rdfs:domain :Property ;
                                          rdfs:range :MISMOIndicator ;
                                          rdfs:comment "When true, indicates that the property is subject to a property clean energy lien that could take precedence over the first mortgage lien including PACE loan or other similar liens."^^xsd:string ;
                                          rdfs:label "Property Existing Clean Energy Lien Indicator"^^xsd:string .


###  http://mismo.org/Subset/propertyExistingLienAmount
:propertyExistingLienAmount rdf:type owl:ObjectProperty ;
                            rdfs:domain :Property ;
                            rdfs:range :MISMOAmount ;
                            rdfs:comment "The total amount of liens against the property at time of application for a loan. Used for Construction or Refinance loans."^^xsd:string ;
                            rdfs:label "Property Existing Lien Amount"^^xsd:string .


###  http://mismo.org/Subset/propertyFloodInsuranceIndicator
:propertyFloodInsuranceIndicator rdf:type owl:ObjectProperty ;
                                 rdfs:domain :Property ;
                                 rdfs:range :MISMOIndicator ;
                                 rdfs:comment "An indicator denoting whether the property securing the mortgage has flood insurance."^^xsd:string ;
                                 rdfs:label "Property Flood Insurance Indicator"^^xsd:string .


###  http://mismo.org/Subset/propertyForeclosureCount
:propertyForeclosureCount rdf:type owl:ObjectProperty ;
                          rdfs:domain :Property ;
                          rdfs:range <http://mismo.org/DataTypes/MISMOCount> ;
                          rdfs:comment "The total number of times previous lenders have foreclosed on the property."^^xsd:string ;
                          rdfs:label "Property Foreclosure Count"^^xsd:string .


###  http://mismo.org/Subset/propertyGroundRent
:propertyGroundRent rdf:type owl:ObjectProperty ;
                    rdfs:domain :Property ;
                    rdfs:range <http://mismo.org/Containers/PropertyGroundRent> ;
                    rdfs:comment "Information about ground rent associated with the property."^^xsd:string ;
                    rdfs:label "property ground rent"^^xsd:string .


###  http://mismo.org/Subset/propertyInProjectIndicator
:propertyInProjectIndicator rdf:type owl:ObjectProperty ;
                            rdfs:domain :Property ;
                            rdfs:range :MISMOIndicator ;
                            rdfs:comment "When true, indicates that the property is located in a project per trading partner guidelines."^^xsd:string ;
                            rdfs:label "Property In Project Indicator"^^xsd:string .


###  http://mismo.org/Subset/propertyInclusionaryZoningIndicator
:propertyInclusionaryZoningIndicator rdf:type owl:ObjectProperty ;
                                     rdfs:domain :Property ;
                                     rdfs:range :MISMOIndicator ;
                                     rdfs:comment "Indicates that the property is subject to Inclusionary zoning, a land-use concept in which builders include a certain amount of affordable housing units for eligible borrowers, in exchange for considerations, such as a \"density bonus\" along with other incentives from the jurisdiction."^^xsd:string ;
                                     rdfs:label "Property Inclusionary Zoning Indicator"^^xsd:string .


###  http://mismo.org/Subset/propertyInspectionWaiverIndicator
:propertyInspectionWaiverIndicator rdf:type owl:ObjectProperty ;
                                   rdfs:domain :Loan ;
                                   rdfs:range :MISMOIndicator ;
                                   rdfs:comment "Indicates whether a documented inspection of the property has been waived."^^xsd:string ;
                                   rdfs:label "Property Inspection Waiver Indicator"^^xsd:string .


###  http://mismo.org/Subset/propertyNotUsed
:propertyNotUsed rdf:type owl:ObjectProperty ;
                 rdfs:domain :Property ;
                 rdfs:range <http://mismo.org/Containers/PropertyNotUsed> ;
                 rdfs:comment "Contains information about data pertaining to properties analyzed but ultimately not used as part of the Sales Comparison Approach."^^xsd:string ;
                 rdfs:label "property not used"^^xsd:string .


###  http://mismo.org/Subset/propertyOriginalCostAmount
:propertyOriginalCostAmount rdf:type owl:ObjectProperty ;
                            rdfs:domain :Property ;
                            rdfs:range :MISMOAmount ;
                            rdfs:comment "The original cost of acquiring the entire property - land and structure. This is used for refinance loans."^^xsd:string ;
                            rdfs:label "Property Original Cost Amount"^^xsd:string .


###  http://mismo.org/Subset/propertyPreviouslyOccupiedIndicator
:propertyPreviouslyOccupiedIndicator rdf:type owl:ObjectProperty ;
                                     rdfs:domain :Property ;
                                     rdfs:range :MISMOIndicator ;
                                     rdfs:comment "Indicates that the property has been previously occupied."^^xsd:string ;
                                     rdfs:label "Property Previously Occupied Indicator"^^xsd:string .


###  http://mismo.org/Subset/propertyStructureHabitableYearRoundIndicator
:propertyStructureHabitableYearRoundIndicator rdf:type owl:ObjectProperty ;
                                              rdfs:domain :Property ;
                                              rdfs:range :MISMOIndicator ;
                                              rdfs:comment "Indicates that the structure or improvement is habitable year round."^^xsd:string ;
                                              rdfs:label "Property Structure Habitable Year Round Indicator"^^xsd:string .


###  http://mismo.org/Subset/propertyTaxes
:propertyTaxes rdf:type owl:ObjectProperty ;
               rdfs:domain :Property ;
               rdfs:range <http://mismo.org/Containers/PropertyTax> ;
               rdfs:comment "Information about one or more PROPERTY_TAX. Holds all occurrences of PROPERTY_TAX."^^xsd:string ;
               rdfs:label "property taxes"^^xsd:string .


###  http://mismo.org/Subset/propertyTitle
:propertyTitle rdf:type owl:ObjectProperty ;
               rdfs:domain :Property ;
               rdfs:range <http://mismo.org/Containers/PropertyTitle> ;
               rdfs:comment "Included Title related information necessary in Secondary Loan Delivery. This is not information captured or reported during the Title Request/Response interaction."^^xsd:string ;
               rdfs:label "property title"^^xsd:string .


###  http://mismo.org/Subset/propertyUsageType
:propertyUsageType rdf:type owl:ObjectProperty ;
                   rdfs:domain :Property ;
                   rdfs:range <http://mismo.org/EnumeratedTypes/PropertyUsageEnum> ;
                   rdfs:comment "A value from a MISMO prescribed list that specifies the intended usage of the property by the borrower."^^xsd:string ;
                   rdfs:label "Property Usage Type"^^xsd:string .


###  http://mismo.org/Subset/propertyUsageTypeOtherDescription
:propertyUsageTypeOtherDescription rdf:type owl:ObjectProperty ;
                                   rdfs:domain :Property ;
                                   rdfs:range :MISMOString ;
                                   rdfs:comment "A free-form text field used to collect additional information when Other is selected for Property Usage Type."^^xsd:string ;
                                   rdfs:label "Property Usage Type Other Description"^^xsd:string .


###  http://mismo.org/Subset/propertyUseSummary
:propertyUseSummary rdf:type owl:ObjectProperty ;
                    rdfs:domain :Property ;
                    rdfs:range <http://mismo.org/Containers/PropertyUseSummary> ;
                    rdfs:comment "Aggregate information about how a property is being used."^^xsd:string ;
                    rdfs:label "property use summary"^^xsd:string .


###  http://mismo.org/Subset/propertyUses
:propertyUses rdf:type owl:ObjectProperty ;
              rdfs:domain :Property ;
              rdfs:range <http://mismo.org/Containers/PropertyUse> ;
              rdfs:comment "Information about one or more PROPERTY_USE. Holds all occurrences of PROPERTY_USE."^^xsd:string ;
              rdfs:label "property uses"^^xsd:string .


###  http://mismo.org/Subset/propertyVacancyDate
:propertyVacancyDate rdf:type owl:ObjectProperty ;
                     rdfs:domain :Property ;
                     rdfs:range :MISMODate ;
                     rdfs:comment "The date the property was first determined to be vacant as determined by the date reported on an inspection report."^^xsd:string ;
                     rdfs:label "Property Vacancy Date"^^xsd:string .


###  http://mismo.org/Subset/propertyValuations
:propertyValuations rdf:type owl:ObjectProperty ;
                    rdfs:domain :Property ;
                    rdfs:range <http://mismo.org/Containers/PropertyValuation> ;
                    rdfs:comment "Information about one or more types of property valuation. Holds all occurrences of PROPERTY_VALUATION."^^xsd:string ;
                    rdfs:label "property valuations"^^xsd:string .


###  http://mismo.org/Subset/protectedAreaDesignationDate
:protectedAreaDesignationDate rdf:type owl:ObjectProperty ;
                              rdfs:domain :FloodDetermination ;
                              rdfs:range :MISMODate ;
                              rdfs:comment "The date of the Coastal Barrier Resources Area (CBRA) or Otherwise Protected Area (OPA)."^^xsd:string ;
                              rdfs:label "Protected Area Designation Date"^^xsd:string .


###  http://mismo.org/Subset/protectedAreaIndicator
:protectedAreaIndicator rdf:type owl:ObjectProperty ;
                        rdfs:domain :FloodDetermination ;
                        rdfs:range :MISMOIndicator ;
                        rdfs:comment "Indicates if the building/mobile home is within a Coastal Barrier Resources Area (CBRA) or Otherwise Protected Area (OPA)."^^xsd:string ;
                        rdfs:label "Protected Area Indicator"^^xsd:string .


###  http://mismo.org/Subset/pud-Indicator
:pud-Indicator rdf:type owl:ObjectProperty ;
               rdfs:domain :Property ;
               rdfs:range :MISMOIndicator ;
               rdfs:comment "When true, indicates that the property is located within a Planned Unit Development (PUD). A PUD is a project or subdivision that consists of common property and / or improvements that are owned and maintained by an ownersâ association for the benefit and use of the individual unit owners."^^xsd:string ;
               rdfs:label "PUD Indicator"^^xsd:string .


###  http://mismo.org/Subset/purchaseCreditSummary
:purchaseCreditSummary rdf:type owl:ObjectProperty ;
                       rdfs:domain :Loan ;
                       rdfs:range <http://mismo.org/Containers/PurchaseCreditSummary> ;
                       rdfs:comment "Information regarding the type and totals of a defined group of purchase credits."^^xsd:string ;
                       rdfs:label "purchase credit summary"^^xsd:string .


###  http://mismo.org/Subset/purchaseCredits
:purchaseCredits rdf:type owl:ObjectProperty ;
                 rdfs:domain :Loan ;
                 rdfs:range <http://mismo.org/Containers/PurchaseCredit> ;
                 rdfs:comment "Information about one or more PURCHASE_CREDIT. Holds all occurrences of PURCHASE_CREDIT."^^xsd:string ;
                 rdfs:label "purchase credits"^^xsd:string .


###  http://mismo.org/Subset/qualification
:qualification rdf:type owl:ObjectProperty ;
               rdfs:domain :Loan ;
               rdfs:range <http://mismo.org/Containers/Qualification> ;
               rdfs:comment "Information used to describe and determine a borrower's eligibility for a loan."^^xsd:string .


###  http://mismo.org/Subset/qualifiedMortgage
:qualifiedMortgage rdf:type owl:ObjectProperty ;
                   rdfs:domain :Loan ;
                   rdfs:range <http://mismo.org/Containers/QualifiedMortgage> ;
                   rdfs:comment "Information used to describe and determine Qualified Mortgage loan eligibility."^^xsd:string ;
                   rdfs:label "qualified mortgage"^^xsd:string .


###  http://mismo.org/Subset/qualifiedMortgageIndicator
:qualifiedMortgageIndicator rdf:type owl:ObjectProperty ;
                            rdfs:domain :Loan ;
                            rdfs:range :MISMOIndicator ;
                            rdfs:comment "When true, indicates the loan is determined to be a qualified mortgage under Regulation Z requirements."^^xsd:string ;
                            rdfs:label "Qualified Mortgage Indicator"^^xsd:string .


###  http://mismo.org/Subset/realPropertyInterests
:realPropertyInterests rdf:type owl:ObjectProperty ;
                       rdfs:domain :Property ;
                       rdfs:range <http://mismo.org/Containers/RealPropertyInterest> ;
                       rdfs:comment "Contains the details of the collateral valuation assignment sufficient for the provider to judge the amount of research and data necessary for the assignment."^^xsd:string ;
                       rdfs:label "real property interests"^^xsd:string .


###  http://mismo.org/Subset/recoverableCorporateAdvanceBalanceFromBorrowerAmount
:recoverableCorporateAdvanceBalanceFromBorrowerAmount rdf:type owl:ObjectProperty ;
                                                      rdfs:domain :Loan ;
                                                      rdfs:range :MISMOAmount ;
                                                      rdfs:comment "Monies advanced on the loan (i.e. delinquency expense, tax penalty, repairs, etc.) that are recoverable from the borrower."^^xsd:string ;
                                                      rdfs:label "Recoverable Corporate Advance Balance From Borrower Amount"^^xsd:string .


###  http://mismo.org/Subset/recoverableCorporateAdvanceBalanceFromThirdPartyAmount
:recoverableCorporateAdvanceBalanceFromThirdPartyAmount rdf:type owl:ObjectProperty ;
                                                        rdfs:domain :Loan ;
                                                        rdfs:range :MISMOAmount ;
                                                        rdfs:comment "Monies advanced on the loan (i.e. delinquency expense, tax penalty, repairs, etc.) that are recoverable from a third party."^^xsd:string ;
                                                        rdfs:label "Recoverable Corporate Advance Balance From Third Party Amount"^^xsd:string .


###  http://mismo.org/Subset/reference
:reference rdf:type owl:ObjectProperty ;
           rdfs:domain :DealChoice ;
           rdfs:range <http://mismo.org/Containers/Reference> ;
           rdfs:comment "REFERENCE is a pointer to an XML structure that satisfies the XML type required within this context. The referenced structure may exist internally or externally to the document. A REFERENCE is resolved by replacing its parent container with the referenced XML structure."^^xsd:string .


###  http://mismo.org/Subset/refinance
:refinance rdf:type owl:ObjectProperty ;
           rdfs:domain :Loan ;
           rdfs:range <http://mismo.org/Containers/Refinance> ;
           rdfs:comment "Information about the refinance of an existing lien."^^xsd:string .


###  http://mismo.org/Subset/refundOfOverpaidInterestCalendarYearAmount
:refundOfOverpaidInterestCalendarYearAmount rdf:type owl:ObjectProperty ;
                                            rdfs:domain :Loan ;
                                            rdfs:range :MISMOAmount ;
                                            rdfs:comment "The amount of overpaid interest refunded to the borrower for the calendar year."^^xsd:string ;
                                            rdfs:label "Refund Of Overpaid Interest Calendar Year Amount"^^xsd:string .


###  http://mismo.org/Subset/regulationZHighCostLoanIndicator
:regulationZHighCostLoanIndicator rdf:type owl:ObjectProperty ;
                                  rdfs:domain :Loan ;
                                  rdfs:range :MISMOIndicator ;
                                  rdfs:comment "When true, indicates the loan is determined to be high cost under Regulation Z."^^xsd:string ;
                                  rdfs:label "Regulation Z High Cost Loan Indicator"^^xsd:string .


###  http://mismo.org/Subset/rehabilitation
:rehabilitation rdf:type owl:ObjectProperty ;
                rdfs:domain :Loan ;
                rdfs:range <http://mismo.org/Containers/Rehabilitation> ;
                rdfs:comment "Information that described the financed cost and completion date of the repair and improvements to the property."^^xsd:string .


###  http://mismo.org/Subset/relationships
:relationships rdf:type owl:ObjectProperty ;
               rdfs:domain [ rdf:type owl:Class ;
                             owl:unionOf ( :DealSequence
                                           :DealSet
                                         )
                           ] ;
               rdfs:range <http://mismo.org/Containers/Relationship> ;
               rdfs:comment "Collection of xlink attributes that define relationships between two elements and optionally provide the type of relationship. Many:Many relationships are formed with multiple RELATIONSHIP children with the same xlink:title value."^^xsd:string .


###  http://mismo.org/Subset/relocationLoanIndicator
:relocationLoanIndicator rdf:type owl:ObjectProperty ;
                         rdfs:domain :Loan ;
                         rdfs:range :MISMOIndicator ;
                         rdfs:comment "Indicates if the loan is part of a corporate relocation program."^^xsd:string ;
                         rdfs:label "Relocation Loan Indicator"^^xsd:string .


###  http://mismo.org/Subset/remainingUnearnedInterestAmount
:remainingUnearnedInterestAmount rdf:type owl:ObjectProperty ;
                                 rdfs:domain :Loan ;
                                 rdfs:range :MISMOAmount ;
                                 rdfs:comment "The remaining amount of interest scheduled to be paid on a rule of 78s loan."^^xsd:string ;
                                 rdfs:label "Remaining Unearned Interest Amount"^^xsd:string .


###  http://mismo.org/Subset/remoteOnlineNotarizationIndicator
:remoteOnlineNotarizationIndicator rdf:type owl:ObjectProperty ;
                                   rdfs:domain :Loan ;
                                   rdfs:range :MISMOIndicator ;
                                   rdfs:comment "When true, indicates an online notarial act was performed between a notary public and a principal using audio-visual technology instead of being physically present."^^xsd:string ;
                                   rdfs:label "Remote Online Notarization Indicator"^^xsd:string .


###  http://mismo.org/Subset/renovationLoanIndicator
:renovationLoanIndicator rdf:type owl:ObjectProperty ;
                         rdfs:domain :Loan ;
                         rdfs:range :MISMOIndicator ;
                         rdfs:comment "When true, indicates that all or part of the subject loan proceeds will be used to finance the renovation of an existing property."^^xsd:string ;
                         rdfs:label "Renovation Loan Indicator"^^xsd:string .


###  http://mismo.org/Subset/rentalEstimatedGrossMonthlyRentAmount
:rentalEstimatedGrossMonthlyRentAmount rdf:type owl:ObjectProperty ;
                                       rdfs:domain :Property ;
                                       rdfs:range :MISMOAmount ;
                                       rdfs:comment "The amount of the estimated gross monthly rental income derived from a single rental unit or property."^^xsd:string ;
                                       rdfs:label "Rental Estimated Gross Monthly Rent Amount"^^xsd:string .


###  http://mismo.org/Subset/rentalEstimatedNetMonthlyRentAmount
:rentalEstimatedNetMonthlyRentAmount rdf:type owl:ObjectProperty ;
                                     rdfs:domain :Property ;
                                     rdfs:range :MISMOAmount ;
                                     rdfs:comment "The amount of the estimated net monthly rental income derived from a single rental unit or property."^^xsd:string ;
                                     rdfs:label "Rental Estimated Net Monthly Rent Amount"^^xsd:string .


###  http://mismo.org/Subset/rentalInformationSummary
:rentalInformationSummary rdf:type owl:ObjectProperty ;
                          rdfs:domain :Property ;
                          rdfs:range <http://mismo.org/Containers/RentalInformationSummary> ;
                          rdfs:comment "Contains aggregate information about the rental information for one or more property unit."^^xsd:string ;
                          rdfs:label "rental information summary"^^xsd:string .


###  http://mismo.org/Subset/repair
:repair rdf:type owl:ObjectProperty ;
        rdfs:domain :Property ;
        rdfs:range <http://mismo.org/Containers/Repair> ;
        rdfs:comment "Information about repairs to bring the property to good and habitable condition."^^xsd:string .


###  http://mismo.org/Subset/rescindableTransactionIndicator
:rescindableTransactionIndicator rdf:type owl:ObjectProperty ;
                                 rdfs:domain :Loan ;
                                 rdfs:range :MISMOIndicator ;
                                 rdfs:comment "When true, indicates that the loan closing transaction has a period of time in which the transaction can be cancelled."^^xsd:string ;
                                 rdfs:label "Rescindable Transaction Indicator"^^xsd:string .


###  http://mismo.org/Subset/respa-ConformingYearType
:respa-ConformingYearType rdf:type owl:ObjectProperty ;
                          rdfs:domain :Loan ;
                          rdfs:range <http://mismo.org/EnumeratedTypes/RESPAConformingYearEnum> ;
                          rdfs:comment "A value from a MISMO prescribed list that represents the version of RESPA regulation under which the loan was originated."^^xsd:string ;
                          rdfs:label "RESPA Conforming Year Type"^^xsd:string .


###  http://mismo.org/Subset/respa-ConformingYearTypeOtherDescription
:respa-ConformingYearTypeOtherDescription rdf:type owl:ObjectProperty ;
                                          rdfs:domain :Loan ;
                                          rdfs:range :MISMOString ;
                                          rdfs:comment "A free-form text field that specifies the enumeration when the value of Other is used for the RESPA Conforming Year Type."^^xsd:string ;
                                          rdfs:label "RESPA Conforming Year Type Other Description"^^xsd:string .


###  http://mismo.org/Subset/reverseMortgage
:reverseMortgage rdf:type owl:ObjectProperty ;
                 rdfs:domain :Loan ;
                 rdfs:range <http://mismo.org/Containers/ReverseMortgage> ;
                 rdfs:comment "Information specific to a reverse mortgage."^^xsd:string ;
                 rdfs:label "reverse mortgage"^^xsd:string .


###  http://mismo.org/Subset/reverseMortgageIndicator
:reverseMortgageIndicator rdf:type owl:ObjectProperty ;
                          rdfs:domain :Loan ;
                          rdfs:range :MISMOIndicator ;
                          rdfs:comment "When true, indicates the loan program uses present equity in the property to fund payments from the lender to the borrower-in lieu of the borrower receiving the proceeds of the loan in a lump sum. As a general rule no payments are made from the borrower to the lender and interest is accrued for payment at the end of the mortgage."^^xsd:string ;
                          rdfs:label "Reverse Mortgage Indicator"^^xsd:string .


###  http://mismo.org/Subset/rightOfRescissionWaitingPeriodWaivedIndicator
:rightOfRescissionWaitingPeriodWaivedIndicator rdf:type owl:ObjectProperty ;
                                               rdfs:domain :Loan ;
                                               rdfs:range :MISMOIndicator ;
                                               rdfs:comment "When true, indicates that due to a bona fide personal financial emergency, the consumer modified or waived the right to rescind waiting period requirement that must be met prior to consummation of the mortgage loan transaction."^^xsd:string ;
                                               rdfs:label "Right Of Rescission Waiting Period Waived Indicator"^^xsd:string .


###  http://mismo.org/Subset/ruralRouteBoxIdentifier
:ruralRouteBoxIdentifier rdf:type owl:ObjectProperty ;
                         rdfs:domain :Address ;
                         rdfs:range :MISMOIdentifier ;
                         rdfs:comment "A unique alphanumeric string identifying the box located on a rural route for the delivery of mail, as assigned by the USPS."^^xsd:string ;
                         rdfs:label "Rural Route Box Identifier"^^xsd:string .


###  http://mismo.org/Subset/ruralRouteIdentifier
:ruralRouteIdentifier rdf:type owl:ObjectProperty ;
                      rdfs:domain :Address ;
                      rdfs:range :MISMOIdentifier ;
                      rdfs:comment "A unique alphanumeric string identifying the rural route for the delivery of mail, as assigned by the USPS."^^xsd:string ;
                      rdfs:label "Rural Route Identifier"^^xsd:string .


###  http://mismo.org/Subset/ruralUnderservedCountyIndicator
:ruralUnderservedCountyIndicator rdf:type owl:ObjectProperty ;
                                 rdfs:domain :Property ;
                                 rdfs:range :MISMOIndicator ;
                                 rdfs:comment "When true, indicates the subject property county has been identified by the Bureau of Consumer Financial Protection as Rural or Underserved."^^xsd:string ;
                                 rdfs:label "Rural Underserved County Indicator"^^xsd:string .


###  http://mismo.org/Subset/salesContracts
:salesContracts rdf:type owl:ObjectProperty ;
                rdfs:domain :Property ;
                rdfs:range <http://mismo.org/Containers/SalesContract> ;
                rdfs:comment "Information about one or more SALES_CONTRACT. Holds all occurrences of SALES_CONTRACT."^^xsd:string ;
                rdfs:label "sales contracts"^^xsd:string .


###  http://mismo.org/Subset/salesHistories
:salesHistories rdf:type owl:ObjectProperty ;
                rdfs:domain :Property ;
                rdfs:range <http://mismo.org/Containers/SalesHistory> ;
                rdfs:comment "Information about one or more SALES_HISTORY. Holds all occurrences of SALES_HISTORY."^^xsd:string ;
                rdfs:label "sales histories"^^xsd:string .


###  http://mismo.org/Subset/scra-Indicator
:scra-Indicator rdf:type owl:ObjectProperty ;
                rdfs:domain :Loan ;
                rdfs:range :MISMOIndicator ;
                rdfs:comment "When true, indicates that the loan is subject to the Servicemembers Civil Relief Act (SCRA)."^^xsd:string ;
                rdfs:label "SCRA Indicator"^^xsd:string .


###  http://mismo.org/Subset/scra-ReliefForbearanceRequestedIndicator
:scra-ReliefForbearanceRequestedIndicator rdf:type owl:ObjectProperty ;
                                          rdfs:domain :Loan ;
                                          rdfs:range :MISMOIndicator ;
                                          rdfs:comment "When true indicates that relief under Servicemembers Civil Relief Act (SCRA) has been requested."^^xsd:string ;
                                          rdfs:label "SCRA Relief Forbearance Requested Indicator"^^xsd:string .


###  http://mismo.org/Subset/scra-ReliefStatusType
:scra-ReliefStatusType rdf:type owl:ObjectProperty ;
                       rdfs:domain :Loan ;
                       rdfs:range <http://mismo.org/EnumeratedTypes/SCRAReliefStatusEnum> ;
                       rdfs:comment "Specifies the status of relief under the Servicemembers Civil Relief Act (SCRA) for any borrower on the loan."^^xsd:string ;
                       rdfs:label "SCRA Relief Status Type"^^xsd:string .


###  http://mismo.org/Subset/scra-ReliefStatusTypeOtherDescription
:scra-ReliefStatusTypeOtherDescription rdf:type owl:ObjectProperty ;
                                       rdfs:domain :Loan ;
                                       rdfs:range :MISMOString ;
                                       rdfs:comment "A free-form text field used to collect additional information when Other is selected as the Servicemember Relief Status Type."^^xsd:string ;
                                       rdfs:label "SCRA Relief Status Type Other Description"^^xsd:string .


###  http://mismo.org/Subset/seasonalPaymentFeatureDescription
:seasonalPaymentFeatureDescription rdf:type owl:ObjectProperty ;
                                   rdfs:domain :Loan ;
                                   rdfs:range :MISMOString ;
                                   rdfs:comment "Specifies the details of the seasonal payment feature, including the period during which periodic payments are not scheduled."^^xsd:string ;
                                   rdfs:label "Seasonal Payment Feature Description"^^xsd:string .


###  http://mismo.org/Subset/seasonalPaymentFeatureIndicator
:seasonalPaymentFeatureIndicator rdf:type owl:ObjectProperty ;
                                 rdfs:domain :Loan ;
                                 rdfs:range :MISMOIndicator ;
                                 rdfs:comment "When true, indicates the loan contains a seasonal payment feature."^^xsd:string ;
                                 rdfs:label "Seasonal Payment Feature Indicator"^^xsd:string .


###  http://mismo.org/Subset/securityTradeBookEntryDate
:securityTradeBookEntryDate rdf:type owl:ObjectProperty ;
                            rdfs:domain :Pool ;
                            rdfs:range :MISMODate ;
                            rdfs:comment "The date that the security will be delivered to the designated book entry account."^^xsd:string ;
                            rdfs:label "Security Trade Book Entry Date"^^xsd:string .


###  http://mismo.org/Subset/securityTradeCustomerAccountIdentifier
:securityTradeCustomerAccountIdentifier rdf:type owl:ObjectProperty ;
                                        rdfs:domain :Pool ;
                                        rdfs:range :MISMOIdentifier ;
                                        rdfs:comment "The securities trading account identifier assigned to a customer by an investor."^^xsd:string ;
                                        rdfs:label "Security Trade Customer Account Identifier"^^xsd:string .


###  http://mismo.org/Subset/sequenceNumber
:sequenceNumber rdf:type owl:ObjectProperty ;
                rdfs:domain [ rdf:type owl:Class ;
                              owl:unionOf ( :Address
                                            :Deal
                                            :DealSet
                                            :HazardInsurance
                                            :Loan
                                            :Property
                                          )
                            ] ;
                rdfs:range <http://mismo.org/DataTypes/MISMOSequenceNumber_Base> ;
                rdfs:comment "An integer value used to provide an order to multi-instance sibling elements. The value must be unique for each sibling element."^^xsd:string ;
                rdfs:label "Sequence Number"^^xsd:string .


###  http://mismo.org/Subset/service
:service rdf:type owl:ObjectProperty ;
         rdfs:domain :DealSequence ;
         rdfs:range <http://mismo.org/Containers/Service> ;
         rdfs:comment "A collection of details related to a fulfillment service or product in terms of request, process and result."^^xsd:string .


###  http://mismo.org/Subset/servicerReporting
:servicerReporting rdf:type owl:ObjectProperty ;
                   rdfs:domain :DealSet ;
                   rdfs:range <http://mismo.org/Containers/ServicerReporting> ;
                   rdfs:comment "Information the servicer periodically reports to the investor."^^xsd:string ;
                   rdfs:label "servicer reporting"^^xsd:string .


###  http://mismo.org/Subset/servicing
:servicing rdf:type owl:ObjectProperty ;
           rdfs:domain :Loan ;
           rdfs:range <http://mismo.org/Containers/Servicing> ;
           rdfs:comment "Loan level information on the servicing of the loan."^^xsd:string .


###  http://mismo.org/Subset/servicingTransferProhibitedIndicator
:servicingTransferProhibitedIndicator rdf:type owl:ObjectProperty ;
                                      rdfs:domain :Loan ;
                                      rdfs:range :MISMOIndicator ;
                                      rdfs:comment "When true, indicates that the transfer of servicing is prohibited during life of the loan or for a designated period of time or until a certain event or condition is satisfied."^^xsd:string ;
                                      rdfs:label "Servicing Transfer Prohibited Indicator"^^xsd:string .


###  http://mismo.org/Subset/servicingTransferStatusType
:servicingTransferStatusType rdf:type owl:ObjectProperty ;
                             rdfs:domain :Loan ;
                             rdfs:range <http://mismo.org/EnumeratedTypes/ServicingTransferStatusEnum> ;
                             rdfs:comment "Defines whether the servicing on the loan will be retained or transferred to another party. Typically only on closed loans."^^xsd:string ;
                             rdfs:label "Servicing Transfer Status Type"^^xsd:string .


###  http://mismo.org/Subset/sharedAppreciationIndicator
:sharedAppreciationIndicator rdf:type owl:ObjectProperty ;
                             rdfs:domain :Loan ;
                             rdfs:range :MISMOIndicator ;
                             rdfs:comment "Indicates the loan is one in which the lender, in exchange for a loan with a favorable interest rate, participates in the profits (if any) the borrower receives when the property is eventually sold."^^xsd:string ;
                             rdfs:label "Shared Appreciation Indicator"^^xsd:string .


###  http://mismo.org/Subset/sharedEquityAmount
:sharedEquityAmount rdf:type owl:ObjectProperty ;
                    rdfs:domain :Loan ;
                    rdfs:range :MISMOAmount ;
                    rdfs:comment "The portion of the down payment paid by a third party as part of a shared equity agreement."^^xsd:string ;
                    rdfs:label "Shared Equity Amount"^^xsd:string .


###  http://mismo.org/Subset/sharedEquityIndicator
:sharedEquityIndicator rdf:type owl:ObjectProperty ;
                       rdfs:domain :Loan ;
                       rdfs:range :MISMOIndicator ;
                       rdfs:comment "Indicates the mortgage is for resale-restricted, owner-occupied housing in which the rights, responsibilities, and benefits of residential property ownership are shared between individual homeowners and another party."^^xsd:string ;
                       rdfs:label "Shared Equity Indicator"^^xsd:string .


###  http://mismo.org/Subset/signedAuthorizationToRequestTaxRecordsIndicator
:signedAuthorizationToRequestTaxRecordsIndicator rdf:type owl:ObjectProperty ;
                                                 rdfs:domain :Loan ;
                                                 rdfs:range :MISMOIndicator ;
                                                 rdfs:comment "Indicates that the IRS form (4506 or 4506T) that gives the lender the authority to request copies of tax records is present."^^xsd:string ;
                                                 rdfs:label "Signed Authorization To Request Tax Records Indicator"^^xsd:string .


###  http://mismo.org/Subset/site
:site rdf:type owl:ObjectProperty ;
      rdfs:domain :Property ;
      rdfs:range <http://mismo.org/Containers/Site> ;
      rdfs:comment "Information that describes features or aspects of the site."^^xsd:string .


###  http://mismo.org/Subset/sketchExistsIndicator
:sketchExistsIndicator rdf:type owl:ObjectProperty ;
                       rdfs:domain :Property ;
                       rdfs:range :MISMOIndicator ;
                       rdfs:comment "When true, indicates that a sketch and/or floor plan has been provided."^^xsd:string ;
                       rdfs:label "Sketch Exists Indicator"^^xsd:string .


###  http://mismo.org/Subset/specialFloodHazardAreaDistanceLinearMeasure
:specialFloodHazardAreaDistanceLinearMeasure rdf:type owl:ObjectProperty ;
                                             rdfs:domain :FloodRiskFactor ;
                                             rdfs:range <http://mismo.org/DataTypes/MISMOLinearMeasure> ;
                                             rdfs:comment "A measurement that specifies the distance in feet of the nearest Special Flood Hazard Area to a particular property.The applicable unit of measurement is specified by the Linear Unit Of Measure Type."^^xsd:string ;
                                             rdfs:label "Special Flood Hazard Area Distance Linear Measure"^^xsd:string .


###  http://mismo.org/Subset/specialFloodHazardAreaIndicator
:specialFloodHazardAreaIndicator rdf:type owl:ObjectProperty ;
                                 rdfs:domain :FloodDetermination ;
                                 rdfs:range :MISMOIndicator ;
                                 rdfs:comment "Flag that indicates if any portion of the building/mobile home is in an identified Special Flood Hazard Area (SFHA) and that flood insurance is required."^^xsd:string ;
                                 rdfs:label "Special Flood Hazard Area Indicator"^^xsd:string .


###  http://mismo.org/Subset/standardizedAdditionalAddressLineText
:standardizedAdditionalAddressLineText rdf:type owl:ObjectProperty ;
                                       rdfs:domain :Address ;
                                       rdfs:range :MISMOString ;
                                       rdfs:comment "A free-form alphanumeric string which contains an additional line of standardized Address information that must be on an additional line in order to be processed correctly by USPS."^^xsd:string ;
                                       rdfs:label "Standardized Additional Address Line Text"^^xsd:string .


###  http://mismo.org/Subset/standardizedAdditionalAddressLineTwoText
:standardizedAdditionalAddressLineTwoText rdf:type owl:ObjectProperty ;
                                          rdfs:domain :Address ;
                                          rdfs:range :MISMOString ;
                                          rdfs:comment "A free-form alphanumeric string which contains a second additional line of standardized Address information that must be on a second additional line in order to be processed correctly by USPS."^^xsd:string ;
                                          rdfs:label "Standardized Additional Address Line Two Text"^^xsd:string .


###  http://mismo.org/Subset/standardizedAddressLineText
:standardizedAddressLineText rdf:type owl:ObjectProperty ;
                             rdfs:domain :Address ;
                             rdfs:range :MISMOString ;
                             rdfs:comment "A free-form alphanumeric string which contains the USPS standardized address with the address number, pre-directional, street name, post-directional, address unit designators and address unit value."^^xsd:string ;
                             rdfs:label "Standardized Address Line Text"^^xsd:string .


###  http://mismo.org/Subset/standardizedAddressUnitDesignatorType
:standardizedAddressUnitDesignatorType rdf:type owl:ObjectProperty ;
                                       rdfs:domain :Address ;
                                       rdfs:range <http://mismo.org/EnumeratedTypes/StandardizedAddressUnitDesignatorEnum> ;
                                       rdfs:comment "A value from a MISMO prescribed list that specifies a further level of detail for a street address, for example, Suite or Unit, in a standardized abbreviated form approved by USPS. This list is based on the USPS Publication 28 on Postal Addressing Standards."^^xsd:string ;
                                       rdfs:label "Standardized Address Unit Designator Type"^^xsd:string .


###  http://mismo.org/Subset/standardizedAddressUnitDesignatorTypeOtherDescription
:standardizedAddressUnitDesignatorTypeOtherDescription rdf:type owl:ObjectProperty ;
                                                       rdfs:domain :Address ;
                                                       rdfs:range :MISMOString ;
                                                       rdfs:comment "A free-form text field that specifies the enumeration when the value of Other is used for Standardized Address Unit Designator Type. This should be used for new USPS values only."^^xsd:string ;
                                                       rdfs:label "Standardized Address Unit Designator Type Other Description"^^xsd:string .


###  http://mismo.org/Subset/standardizedPR-UrbanizationType
:standardizedPR-UrbanizationType rdf:type owl:ObjectProperty ;
                                 rdfs:domain :Address ;
                                 rdfs:range <http://mismo.org/EnumeratedTypes/StandardizedPRUrbanizationEnum> ;
                                 rdfs:comment "A value from a MISMO prescribed list that describes text used in a Spanish language Puerto Rican street address that contains an urbanization that is not preceded by the prefix URB, and is expressed as a standardized USPS abbreviation as outlined in USPS publication 28."^^xsd:string ;
                                 rdfs:label "Standardized PR Urbanization Type"^^xsd:string .


###  http://mismo.org/Subset/standardizedPR-UrbanizationTypeOtherDescription
:standardizedPR-UrbanizationTypeOtherDescription rdf:type owl:ObjectProperty ;
                                                 rdfs:domain :Address ;
                                                 rdfs:range :MISMOString ;
                                                 rdfs:comment "A free-form text field that specifies the enumeration when the value of Other is used for Standardized PR Urbanization Type. This should be used for new USPS values only."^^xsd:string ;
                                                 rdfs:label "Standardized PR Urbanization Type Other Description"^^xsd:string .


###  http://mismo.org/Subset/standardizedRuralHighwayContractRouteType
:standardizedRuralHighwayContractRouteType rdf:type owl:ObjectProperty ;
                                           rdfs:domain :Address ;
                                           rdfs:range <http://mismo.org/EnumeratedTypes/StandardizedRuralHighwayContractRouteEnum> ;
                                           rdfs:comment "A value from a MISMO prescribed list that describes the name of the Rural Route, Highway Contract Route, or other special route type, expressed as the standardized USPS abbreviation as outlined in USPS publication 28."^^xsd:string ;
                                           rdfs:label "Standardized Rural Highway Contract Route Type"^^xsd:string .


###  http://mismo.org/Subset/standardizedRuralHighwayContractRouteTypeOtherDescription
:standardizedRuralHighwayContractRouteTypeOtherDescription rdf:type owl:ObjectProperty ;
                                                           rdfs:domain :Address ;
                                                           rdfs:range :MISMOString ;
                                                           rdfs:comment "A free-form text field that specifies the enumeration when the value of Other is used for Standardized Rural Highway Contract Route Type. This should be used for new USPS values only."^^xsd:string ;
                                                           rdfs:label "Standardized Rural Highway Contract Route Type Other Description"^^xsd:string .


###  http://mismo.org/Subset/standardizedSpanishAddressDesignatorType
:standardizedSpanishAddressDesignatorType rdf:type owl:ObjectProperty ;
                                          rdfs:domain :Address ;
                                          rdfs:range <http://mismo.org/EnumeratedTypes/StandardizedSpanishAddressDesignatorEnum> ;
                                          rdfs:comment "A value from a MISMO prescribed list that describes text sometimes used in a Spanish language Puerto Rican address, instead of a specific street address, expressed as a standardized USPS abbreviation as outlined in USPS publication 28."^^xsd:string ;
                                          rdfs:label "Standardized Spanish Address Designator Type"^^xsd:string .


###  http://mismo.org/Subset/standardizedSpanishAddressDesignatorTypeOtherDescription
:standardizedSpanishAddressDesignatorTypeOtherDescription rdf:type owl:ObjectProperty ;
                                                          rdfs:domain :Address ;
                                                          rdfs:range :MISMOString ;
                                                          rdfs:comment "A free-form text field that specifies the enumeration when the value of Other is used for Standardized Spanish Address Designator Type. This should be used for new USPS values only."^^xsd:string ;
                                                          rdfs:label "Standardized Spanish Address Designator Type Other Description"^^xsd:string .


###  http://mismo.org/Subset/standardizedStreetSuffixType
:standardizedStreetSuffixType rdf:type owl:ObjectProperty ;
                              rdfs:domain :Address ;
                              rdfs:range <http://mismo.org/EnumeratedTypes/StandardizedStreetSuffixEnum> ;
                              rdfs:comment "A value from a MISMO prescribed list that describes the trailing designator in a street address expressed as the standardized USPS abbreviation as outlined in USPS publication 28."^^xsd:string ;
                              rdfs:label "Standardized Street Suffix Type"^^xsd:string .


###  http://mismo.org/Subset/standardizedStreetSuffixTypeOtherDescription
:standardizedStreetSuffixTypeOtherDescription rdf:type owl:ObjectProperty ;
                                              rdfs:domain :Address ;
                                              rdfs:range :MISMOString ;
                                              rdfs:comment "A free-form text field that specifies the enumeration when the value of Other is used for Standardized Street Suffix Type. This should be used for new USPS values only."^^xsd:string ;
                                              rdfs:label "Standardized Street Suffix Type Other Description"^^xsd:string .


###  http://mismo.org/Subset/stateCode
:stateCode rdf:type owl:ObjectProperty ;
           rdfs:domain :Address ;
           rdfs:range <http://mismo.org/DataTypes/MISMOCode> ;
           rdfs:comment "The two-character representation of the US state, US Territory, Canadian Province/Territory, or Military Address abbreviation (for example: AE, AP, AA)."^^xsd:string ;
           rdfs:label "State Code"^^xsd:string .


###  http://mismo.org/Subset/stateName
:stateName rdf:type owl:ObjectProperty ;
           rdfs:domain :Address ;
           rdfs:range :MISMOString ;
           rdfs:comment "The name of the US state, US Territory, Canadian Province/Territory, or Military Address."^^xsd:string ;
           rdfs:label "State Name"^^xsd:string .


###  http://mismo.org/Subset/stepPaymentsFeatureDescription
:stepPaymentsFeatureDescription rdf:type owl:ObjectProperty ;
                                rdfs:domain :Loan ;
                                rdfs:range :MISMOString ;
                                rdfs:comment "Specifies the details of the step payments feature, including the period during which periodic payments are scheduled to increase."^^xsd:string ;
                                rdfs:label "Step Payments Feature Description"^^xsd:string .


###  http://mismo.org/Subset/streetName
:streetName rdf:type owl:ObjectProperty ;
            rdfs:domain :Address ;
            rdfs:range :MISMOString ;
            rdfs:comment "The official name of a street assigned by a local governing authority."^^xsd:string ;
            rdfs:label "Street Name"^^xsd:string .


###  http://mismo.org/Subset/streetPostDirectionalText
:streetPostDirectionalText rdf:type owl:ObjectProperty ;
                           rdfs:domain :Address ;
                           rdfs:range :MISMOString ;
                           rdfs:comment "The directional symbol that represents the sector of a city where a street address is located. Example: E, W, N, S, NE, NW, SE, SW."^^xsd:string ;
                           rdfs:label "Street Post Directional Text"^^xsd:string .


###  http://mismo.org/Subset/streetPreDirectionalText
:streetPreDirectionalText rdf:type owl:ObjectProperty ;
                          rdfs:domain :Address ;
                          rdfs:range :MISMOString ;
                          rdfs:comment "The street vector or the direction the street has taken from some arbitrary starting point. Example: E, W, N, S, NE, NW, SE, SW."^^xsd:string ;
                          rdfs:label "Street Pre Directional Text"^^xsd:string .


###  http://mismo.org/Subset/streetPrimaryNumberText
:streetPrimaryNumberText rdf:type owl:ObjectProperty ;
                         rdfs:domain :Address ;
                         rdfs:range :MISMOString ;
                         rdfs:comment "The number assigned to a building or land parcel along the street to identify location and ensure accurate mail delivery."^^xsd:string ;
                         rdfs:label "Street Primary Number Text"^^xsd:string .


###  http://mismo.org/Subset/streetSuffixText
:streetSuffixText rdf:type owl:ObjectProperty ;
                  rdfs:domain :Address ;
                  rdfs:range :MISMOString ;
                  rdfs:comment "The trailing designator in a street address or the appropriate abbreviation. Example: Drive, Way, Court, Street, etc."^^xsd:string ;
                  rdfs:label "Street Suffix Text"^^xsd:string .


###  http://mismo.org/Subset/subjectPropertyAmenitiesDefectsExistIndicator
:subjectPropertyAmenitiesDefectsExistIndicator rdf:type owl:ObjectProperty ;
                                               rdfs:domain :Property ;
                                               rdfs:range :MISMOIndicator ;
                                               rdfs:comment "When true, indicates that at least one of the amenities associated with the property has defect(s), damage(s) or deficienc(ies)."^^xsd:string ;
                                               rdfs:label "Subject Property Amenities Defects Exist Indicator"^^xsd:string .


###  http://mismo.org/Subset/subordinateFinancingIsNewIndicator
:subordinateFinancingIsNewIndicator rdf:type owl:ObjectProperty ;
                                    rdfs:domain :Loan ;
                                    rdfs:range :MISMOIndicator ;
                                    rdfs:comment "When true indicates that subordinate financing is being created simultaneously with the subject loan."^^xsd:string ;
                                    rdfs:label "Subordinate Financing Is New Indicator"^^xsd:string .


###  http://mismo.org/Subset/supportingRecordSets
:supportingRecordSets rdf:type owl:ObjectProperty ;
                      rdfs:domain :DealSequence ;
                      rdfs:range <http://mismo.org/Containers/SupportingRecordSet> ;
                      rdfs:comment "Information about one or more supporting record sets. Holds all occurrences of SUPPORTING RECORD SET."^^xsd:string ;
                      rdfs:label "supporting record sets"^^xsd:string .


###  http://mismo.org/Subset/taxRecordsObtainedIndicator
:taxRecordsObtainedIndicator rdf:type owl:ObjectProperty ;
                             rdfs:domain :Loan ;
                             rdfs:range :MISMOIndicator ;
                             rdfs:comment "Indicates that the IRS form (4506 or 4506T) that gives the lender the authority to request copies of tax records has been executed by the lender."^^xsd:string ;
                             rdfs:label "Tax Records Obtained Indicator"^^xsd:string .


###  http://mismo.org/Subset/termsOfLoan
:termsOfLoan rdf:type owl:ObjectProperty ;
             rdfs:domain :Loan ;
             rdfs:range <http://mismo.org/Containers/TermsOfLoan> ;
             rdfs:comment "Describes characteristics of the loan, including the behavior defined in the financial instrument."^^xsd:string ;
             rdfs:label "terms of loan"^^xsd:string .


###  http://mismo.org/Subset/thirdPartyReviewIndicator
:thirdPartyReviewIndicator rdf:type owl:ObjectProperty ;
                           rdfs:domain :Loan ;
                           rdfs:range :MISMOIndicator ;
                           rdfs:comment "Indicates that a third party due diligence review firm has reviewed the loan data."^^xsd:string ;
                           rdfs:label "Third Party Review Indicator"^^xsd:string .


###  http://mismo.org/Subset/timelyPaymentRateReductionIndicator
:timelyPaymentRateReductionIndicator rdf:type owl:ObjectProperty ;
                                     rdfs:domain :Loan ;
                                     rdfs:range :MISMOIndicator ;
                                     rdfs:comment "Flag indicating if the loan is eligible for a rate reduction if payments are received in a timely manner."^^xsd:string ;
                                     rdfs:label "Timely Payment Rate Reduction Indicator"^^xsd:string .


###  http://mismo.org/Subset/totalFinancedEnergyImprovementsAmount
:totalFinancedEnergyImprovementsAmount rdf:type owl:ObjectProperty ;
                                       rdfs:domain :Loan ;
                                       rdfs:range :MISMOAmount ;
                                       rdfs:comment "The total financed amount of all new energy improvements to the subject property that are part of this loan."^^xsd:string ;
                                       rdfs:label "Total Financed Energy Improvements Amount"^^xsd:string .


###  http://mismo.org/Subset/totalFinishedAreaOfAllLivingUnitsIncludingADU-AreaMeasure
:totalFinishedAreaOfAllLivingUnitsIncludingADU-AreaMeasure rdf:type owl:ObjectProperty ;
                                                           rdfs:domain :Property ;
                                                           rdfs:range <http://mismo.org/DataTypes/MISMOAreaMeasure> ;
                                                           rdfs:comment "A measurement that specifies the total finished area from all accessory dwelling units, finished area of all living units, and finished area from any common area located within the dwelling(s). The applicable unit of measurement is specified by the Area Unit Of Measure Type."^^xsd:string ;
                                                           rdfs:label "Total Finished Area Of All Living Units Including ADU Area Measure"^^xsd:string .


###  http://mismo.org/Subset/totalMortgagedPropertiesCount
:totalMortgagedPropertiesCount rdf:type owl:ObjectProperty ;
                               rdfs:domain :Loan ;
                               rdfs:range <http://mismo.org/DataTypes/MISMOCount> ;
                               rdfs:comment "The number of 1-4 unit properties that are financed and owned and/or obligated on by the borrower(s). A jointly owned/obligated property by multiple borrowers would count only once."^^xsd:string ;
                               rdfs:label "Total Mortgaged Properties Count"^^xsd:string .


###  http://mismo.org/Subset/totalNonContinuousFinishedAreaOfAllDwellingsAreaMeasure
:totalNonContinuousFinishedAreaOfAllDwellingsAreaMeasure rdf:type owl:ObjectProperty ;
                                                         rdfs:domain :Property ;
                                                         rdfs:range <http://mismo.org/DataTypes/MISMOAreaMeasure> ;
                                                         rdfs:comment "The total measurement of the finished areas of all the dwellings with space attached to any that is separate and not accessible from any unit(s) (i.e. the sum total of all non-continuous space across all dwellings). The applicable unit of measurement is specified by the Area Unit Of Measure Type."^^xsd:string ;
                                                         rdfs:label "Total Non Continuous Finished Area Of All Dwellings Area Measure"^^xsd:string .


###  http://mismo.org/Subset/totalOfAllDwellingsVolumeMeasure
:totalOfAllDwellingsVolumeMeasure rdf:type owl:ObjectProperty ;
                                  rdfs:domain :Property ;
                                  rdfs:range <http://mismo.org/DataTypes/MISMOVolumeMeasure> ;
                                  rdfs:comment "A measurement that specifies the total volume, including finished and unfinished areas, of all dwellings on the property, including ADUs. The applicable unit of measurement is specified by the Volume Unit Of Measure Type."^^xsd:string ;
                                  rdfs:label "Total Of All Dwellings Volume Measure"^^xsd:string .


###  http://mismo.org/Subset/totalSalesConcessionAmount
:totalSalesConcessionAmount rdf:type owl:ObjectProperty ;
                            rdfs:domain :Loan ;
                            rdfs:range :MISMOAmount ;
                            rdfs:comment "The sum total dollar amount of the value of all sales concessions granted by an interested party including such items as furniture, carpeting, decorator allowances, automobiles, vacations, securities, giveaways or other sales incentives."^^xsd:string ;
                            rdfs:label "Total Sales Concession Amount"^^xsd:string .


###  http://mismo.org/Subset/totalSeniorFinancingAmount
:totalSeniorFinancingAmount rdf:type owl:ObjectProperty ;
                            rdfs:domain :Loan ;
                            rdfs:range :MISMOAmount ;
                            rdfs:comment "The total dollar amount of financing associated with all loans to which the subject loan is subordinated."^^xsd:string ;
                            rdfs:label "Total Senior Financing Amount"^^xsd:string .


###  http://mismo.org/Subset/totalSubordinateFinancingAmount
:totalSubordinateFinancingAmount rdf:type owl:ObjectProperty ;
                                 rdfs:domain :Loan ;
                                 rdfs:range :MISMOAmount ;
                                 rdfs:comment "The total amount of subordinate financing associated with the loan."^^xsd:string ;
                                 rdfs:label "Total Subordinate Financing Amount"^^xsd:string .


###  http://mismo.org/Subset/totalSubordinateFinancingProceedsAppliedAmount
:totalSubordinateFinancingProceedsAppliedAmount rdf:type owl:ObjectProperty ;
                                                rdfs:domain :Loan ;
                                                rdfs:range :MISMOAmount ;
                                                rdfs:comment "The total of all subordinate loan proceeds used for the mortgage transaction."^^xsd:string ;
                                                rdfs:label "Total Subordinate Financing Proceeds Applied Amount"^^xsd:string .


###  http://mismo.org/Subset/totalWindowSurfaceAreaOfAllDwellingsAreaMeasure
:totalWindowSurfaceAreaOfAllDwellingsAreaMeasure rdf:type owl:ObjectProperty ;
                                                 rdfs:domain :Property ;
                                                 rdfs:range <http://mismo.org/DataTypes/MISMOAreaMeasure> ;
                                                 rdfs:comment "A measurement that specifies the total window surface area for all windows of all dwellings on the property. The applicable unit of measurement is specified by the Area Unit Of Measure Type."^^xsd:string ;
                                                 rdfs:label "Total Window Surface Area Of All Dwellings Area Measure"^^xsd:string .


###  http://mismo.org/Subset/treasuryNpv
:treasuryNpv rdf:type owl:ObjectProperty ;
             rdfs:domain :Loan ;
             rdfs:range <http://mismo.org/Containers/TreasuryNPV> ;
             rdfs:comment "Information about the results and factors associated with the Treasury Net Present Value Test."^^xsd:string ;
             rdfs:label "treasury npv"^^xsd:string .


###  http://mismo.org/Subset/trid-RuleIndicator
:trid-RuleIndicator rdf:type owl:ObjectProperty ;
                    rdfs:domain :Loan ;
                    rdfs:range :MISMOIndicator ;
                    rdfs:comment "When true indicates the loan or application is subject to the TILA RESPA Integrated Disclosure (TRID) rule in Regulation Z."^^xsd:string ;
                    rdfs:label "TRID Rule Indicator"^^xsd:string .


###  http://mismo.org/Subset/undefinedPropertyType
:undefinedPropertyType rdf:type owl:ObjectProperty ;
                       rdfs:domain :Property ;
                       rdfs:range <http://mismo.org/EnumeratedTypes/UndefinedPropertyEnum> ;
                       rdfs:comment "A value from a MISMO prescribed list that represents a type of property that does not meet a uniform set of characteristics for defining the components used to classify a property type."^^xsd:string ;
                       rdfs:label "Undefined Property Type"^^xsd:string .


###  http://mismo.org/Subset/underwriting
:underwriting rdf:type owl:ObjectProperty ;
              rdfs:domain :Loan ;
              rdfs:range <http://mismo.org/Containers/Underwriting> ;
              rdfs:comment "Information about how the loan was underwritten, by whom the loan was underwritten, the underwriting decision, and key parameters influencing that decision."^^xsd:string .


###  http://mismo.org/Subset/uniqueDwellingType
:uniqueDwellingType rdf:type owl:ObjectProperty ;
                    rdfs:domain :Property ;
                    rdfs:range <http://mismo.org/EnumeratedTypes/UniqueDwellingEnum> ;
                    rdfs:comment "A dwelling that does not conform to a conventional building structure type or method."^^xsd:string ;
                    rdfs:label "Unique Dwelling Type"^^xsd:string .


###  http://mismo.org/Subset/uniqueDwellingTypeOtherDescription
:uniqueDwellingTypeOtherDescription rdf:type owl:ObjectProperty ;
                                    rdfs:domain :Property ;
                                    rdfs:range :MISMOString ;
                                    rdfs:comment "A text field used to describe the Unique Dwelling when \"Other\" is selected from the enumerated list."^^xsd:string ;
                                    rdfs:label "Unique Dwelling Type Other Description"^^xsd:string .


###  http://mismo.org/Subset/vehicleStorageDefectsExistIndicator
:vehicleStorageDefectsExistIndicator rdf:type owl:ObjectProperty ;
                                     rdfs:domain :Property ;
                                     rdfs:range :MISMOIndicator ;
                                     rdfs:comment "When true, indicates that at least one of the vehicle storages associated with the property has defect(s), damage(s) or deficienc(ies)."^^xsd:string ;
                                     rdfs:label "Vehicle Storage Defects Exist Indicator"^^xsd:string .


###  http://mismo.org/Subset/warehouseLenderIndicator
:warehouseLenderIndicator rdf:type owl:ObjectProperty ;
                          rdfs:domain :Loan ;
                          rdfs:range :MISMOIndicator ;
                          rdfs:comment "An indicator denoting whether a Warehouse Bank is involved in the mortgage loan transaction through a relationship with the lender."^^xsd:string ;
                          rdfs:label "Warehouse Lender Indicator"^^xsd:string .


###  http://mismo.org/Subset/workoutActiveIndicator
:workoutActiveIndicator rdf:type owl:ObjectProperty ;
                        rdfs:domain :Loan ;
                        rdfs:range :MISMOIndicator ;
                        rdfs:comment "When true, indicates that the loan is actively in the workout process."^^xsd:string ;
                        rdfs:label "Workout Active Indicator"^^xsd:string .


###  http://mismo.org/Subset/workoutSummary
:workoutSummary rdf:type owl:ObjectProperty ;
                rdfs:domain :Loan ;
                rdfs:range <http://mismo.org/Containers/WorkoutSummary> ;
                rdfs:comment "Summary information about workouts that have occurred or were attempted on the loan."^^xsd:string ;
                rdfs:label "workout summary"^^xsd:string .


###  http://mismo.org/Subset/workouts
:workouts rdf:type owl:ObjectProperty ;
          rdfs:domain :Loan ;
          rdfs:range <http://mismo.org/Containers/Workout> ;
          rdfs:comment "Information about one or more WORKOUT. Holds all occurrences of WORKOUT."^^xsd:string .


#################################################################
#    Data properties
#################################################################

###  http://mismo.org/Subset/DataNotSuppliedReasonType
:DataNotSuppliedReasonType rdf:type owl:DatatypeProperty ;
                           rdfs:domain [ rdf:type owl:Class ;
                                         owl:unionOf ( :MISMOAmount
                                                       :MISMODate
                                                       :MISMOIdentifier
                                                       :MISMOIndicator
                                                       :MISMORate
                                                       :MISMOString
                                                     )
                                       ] ;
                           rdfs:range <http://mismo.org/DataTypes/DataNotSuppliedReasonBase> ;
                           rdfs:comment "A value from a MISMO prescribed list that specifies the reason a specific data point is not included in the message."^^xsd:string .


###  http://mismo.org/Subset/loanRoleType
:loanRoleType rdf:type owl:DatatypeProperty ;
              rdfs:domain :Loan ;
              rdfs:range <http://mismo.org/EnumeratedTypes/LoanRoleBase> ;
              rdfs:comment "An attribute of LOAN used to identify the role the associated LOAN plays in the transaction."^^xsd:string ;
              rdfs:label "Loan Role Type"^^xsd:string .


###  http://mismo.org/Subset/selectionType
:selectionType rdf:type owl:DatatypeProperty ;
               rdfs:domain :Loan ;
               rdfs:range <http://mismo.org/EnumeratedTypes/SelectionBase> ;
               rdfs:comment "A classification of the collection of loan parameters to support borrower shopping for loan products or proposed loan products that would suit the current borrower needs."^^xsd:string ;
               rdfs:label "Selection Type"^^xsd:string .


###  http://mismo.org/Subset/valuationUseType
:valuationUseType rdf:type owl:DatatypeProperty ;
                  rdfs:domain :Property ;
                  rdfs:range <http://mismo.org/EnumeratedTypes/ValuationUseBase> ;
                  rdfs:comment "Used as an attribute on PROPERTY to specify whether the referenced property is the Subject property or a property valuation comparable."^^xsd:string ;
                  rdfs:label "Valuation Use Type"^^xsd:string .


#################################################################
#    Classes
#################################################################

###  http://mismo.org/Subset/Address
:Address rdf:type owl:Class ;
         rdfs:subClassOf [ rdf:type owl:Restriction ;
                           owl:onProperty :addressAdditionalLineText ;
                           owl:cardinality "1"^^xsd:nonNegativeInteger
                         ] ,
                         [ rdf:type owl:Restriction ;
                           owl:onProperty :addressAdditionalLineTwoText ;
                           owl:cardinality "1"^^xsd:nonNegativeInteger
                         ] ,
                         [ rdf:type owl:Restriction ;
                           owl:onProperty :addressCondominiumApartmentText ;
                           owl:cardinality "1"^^xsd:nonNegativeInteger
                         ] ,
                         [ rdf:type owl:Restriction ;
                           owl:onProperty :addressFormatType ;
                           owl:cardinality "1"^^xsd:nonNegativeInteger
                         ] ,
                         [ rdf:type owl:Restriction ;
                           owl:onProperty :addressFormatTypeOtherDescription ;
                           owl:cardinality "1"^^xsd:nonNegativeInteger
                         ] ,
                         [ rdf:type owl:Restriction ;
                           owl:onProperty :addressIsNotUSPS-CodableIndicator ;
                           owl:cardinality "1"^^xsd:nonNegativeInteger
                         ] ,
                         [ rdf:type owl:Restriction ;
                           owl:onProperty :addressLineText ;
                           owl:cardinality "1"^^xsd:nonNegativeInteger
                         ] ,
                         [ rdf:type owl:Restriction ;
                           owl:onProperty :addressPR-UrbanizationText ;
                           owl:cardinality "1"^^xsd:nonNegativeInteger
                         ] ,
                         [ rdf:type owl:Restriction ;
                           owl:onProperty :addressType ;
                           owl:cardinality "1"^^xsd:nonNegativeInteger
                         ] ,
                         [ rdf:type owl:Restriction ;
                           owl:onProperty :addressTypeOtherDescription ;
                           owl:cardinality "1"^^xsd:nonNegativeInteger
                         ] ,
                         [ rdf:type owl:Restriction ;
                           owl:onProperty :addressUnitDesignatorType ;
                           owl:cardinality "1"^^xsd:nonNegativeInteger
                         ] ,
                         [ rdf:type owl:Restriction ;
                           owl:onProperty :addressUnitDesignatorTypeOtherDescription ;
                           owl:cardinality "1"^^xsd:nonNegativeInteger
                         ] ,
                         [ rdf:type owl:Restriction ;
                           owl:onProperty :addressUnitIdentifier ;
                           owl:cardinality "1"^^xsd:nonNegativeInteger
                         ] ,
                         [ rdf:type owl:Restriction ;
                           owl:onProperty :attentionToName ;
                           owl:cardinality "1"^^xsd:nonNegativeInteger
                         ] ,
                         [ rdf:type owl:Restriction ;
                           owl:onProperty :carrierRouteCode ;
                           owl:cardinality "1"^^xsd:nonNegativeInteger
                         ] ,
                         [ rdf:type owl:Restriction ;
                           owl:onProperty :cityName ;
                           owl:cardinality "1"^^xsd:nonNegativeInteger
                         ] ,
                         [ rdf:type owl:Restriction ;
                           owl:onProperty :countryCode ;
                           owl:cardinality "1"^^xsd:nonNegativeInteger
                         ] ,
                         [ rdf:type owl:Restriction ;
                           owl:onProperty :countryName ;
                           owl:cardinality "1"^^xsd:nonNegativeInteger
                         ] ,
                         [ rdf:type owl:Restriction ;
                           owl:onProperty :countyCode ;
                           owl:cardinality "1"^^xsd:nonNegativeInteger
                         ] ,
                         [ rdf:type owl:Restriction ;
                           owl:onProperty :countyName ;
                           owl:cardinality "1"^^xsd:nonNegativeInteger
                         ] ,
                         [ rdf:type owl:Restriction ;
                           owl:onProperty :deliveryPointBarCodeCheckValue ;
                           owl:cardinality "1"^^xsd:nonNegativeInteger
                         ] ,
                         [ rdf:type owl:Restriction ;
                           owl:onProperty :deliveryPointBarCodeValue ;
                           owl:cardinality "1"^^xsd:nonNegativeInteger
                         ] ,
                         [ rdf:type owl:Restriction ;
                           owl:onProperty :highwayContractBoxIdentifier ;
                           owl:cardinality "1"^^xsd:nonNegativeInteger
                         ] ,
                         [ rdf:type owl:Restriction ;
                           owl:onProperty :highwayContractRouteIdentifier ;
                           owl:cardinality "1"^^xsd:nonNegativeInteger
                         ] ,
                         [ rdf:type owl:Restriction ;
                           owl:onProperty :mailStopCode ;
                           owl:cardinality "1"^^xsd:nonNegativeInteger
                         ] ,
                         [ rdf:type owl:Restriction ;
                           owl:onProperty :plusFourZipCode ;
                           owl:cardinality "1"^^xsd:nonNegativeInteger
                         ] ,
                         [ rdf:type owl:Restriction ;
                           owl:onProperty :postOfficeBoxIdentifier ;
                           owl:cardinality "1"^^xsd:nonNegativeInteger
                         ] ,
                         [ rdf:type owl:Restriction ;
                           owl:onProperty :postalCode ;
                           owl:cardinality "1"^^xsd:nonNegativeInteger
                         ] ,
                         [ rdf:type owl:Restriction ;
                           owl:onProperty :ruralRouteBoxIdentifier ;
                           owl:cardinality "1"^^xsd:nonNegativeInteger
                         ] ,
                         [ rdf:type owl:Restriction ;
                           owl:onProperty :ruralRouteIdentifier ;
                           owl:cardinality "1"^^xsd:nonNegativeInteger
                         ] ,
                         [ rdf:type owl:Restriction ;
                           owl:onProperty :sequenceNumber ;
                           owl:cardinality "1"^^xsd:nonNegativeInteger
                         ] ,
                         [ rdf:type owl:Restriction ;
                           owl:onProperty :standardizedAdditionalAddressLineText ;
                           owl:cardinality "1"^^xsd:nonNegativeInteger
                         ] ,
                         [ rdf:type owl:Restriction ;
                           owl:onProperty :standardizedAdditionalAddressLineTwoText ;
                           owl:cardinality "1"^^xsd:nonNegativeInteger
                         ] ,
                         [ rdf:type owl:Restriction ;
                           owl:onProperty :standardizedAddressLineText ;
                           owl:cardinality "1"^^xsd:nonNegativeInteger
                         ] ,
                         [ rdf:type owl:Restriction ;
                           owl:onProperty :standardizedAddressUnitDesignatorType ;
                           owl:cardinality "1"^^xsd:nonNegativeInteger
                         ] ,
                         [ rdf:type owl:Restriction ;
                           owl:onProperty :standardizedAddressUnitDesignatorTypeOtherDescription ;
                           owl:cardinality "1"^^xsd:nonNegativeInteger
                         ] ,
                         [ rdf:type owl:Restriction ;
                           owl:onProperty :standardizedPR-UrbanizationType ;
                           owl:cardinality "1"^^xsd:nonNegativeInteger
                         ] ,
                         [ rdf:type owl:Restriction ;
                           owl:onProperty :standardizedPR-UrbanizationTypeOtherDescription ;
                           owl:cardinality "1"^^xsd:nonNegativeInteger
                         ] ,
                         [ rdf:type owl:Restriction ;
                           owl:onProperty :standardizedRuralHighwayContractRouteType ;
                           owl:cardinality "1"^^xsd:nonNegativeInteger
                         ] ,
                         [ rdf:type owl:Restriction ;
                           owl:onProperty :standardizedRuralHighwayContractRouteTypeOtherDescription ;
                           owl:cardinality "1"^^xsd:nonNegativeInteger
                         ] ,
                         [ rdf:type owl:Restriction ;
                           owl:onProperty :standardizedSpanishAddressDesignatorType ;
                           owl:cardinality "1"^^xsd:nonNegativeInteger
                         ] ,
                         [ rdf:type owl:Restriction ;
                           owl:onProperty :standardizedSpanishAddressDesignatorTypeOtherDescription ;
                           owl:cardinality "1"^^xsd:nonNegativeInteger
                         ] ,
                         [ rdf:type owl:Restriction ;
                           owl:onProperty :standardizedStreetSuffixType ;
                           owl:cardinality "1"^^xsd:nonNegativeInteger
                         ] ,
                         [ rdf:type owl:Restriction ;
                           owl:onProperty :standardizedStreetSuffixTypeOtherDescription ;
                           owl:cardinality "1"^^xsd:nonNegativeInteger
                         ] ,
                         [ rdf:type owl:Restriction ;
                           owl:onProperty :stateCode ;
                           owl:cardinality "1"^^xsd:nonNegativeInteger
                         ] ,
                         [ rdf:type owl:Restriction ;
                           owl:onProperty :stateName ;
                           owl:cardinality "1"^^xsd:nonNegativeInteger
                         ] ,
                         [ rdf:type owl:Restriction ;
                           owl:onProperty :streetName ;
                           owl:cardinality "1"^^xsd:nonNegativeInteger
                         ] ,
                         [ rdf:type owl:Restriction ;
                           owl:onProperty :streetPostDirectionalText ;
                           owl:cardinality "1"^^xsd:nonNegativeInteger
                         ] ,
                         [ rdf:type owl:Restriction ;
                           owl:onProperty :streetPreDirectionalText ;
                           owl:cardinality "1"^^xsd:nonNegativeInteger
                         ] ,
                         [ rdf:type owl:Restriction ;
                           owl:onProperty :streetPrimaryNumberText ;
                           owl:cardinality "1"^^xsd:nonNegativeInteger
                         ] ,
                         [ rdf:type owl:Restriction ;
                           owl:onProperty :streetSuffixText ;
                           owl:cardinality "1"^^xsd:nonNegativeInteger
                         ] ,
                         [ rdf:type owl:Restriction ;
                           owl:onProperty :extension ;
                           owl:maxCardinality "1"^^xsd:nonNegativeInteger
                         ] ;
         rdfs:comment "Address is based upon USPS publication 28. Publication 28 has two sections, format of an address on a piece of mail and data points that MAY compose an address. The data point children of ADDRESS are the union components of an address on a piece of mail or a package."^^xsd:string .


###  http://mismo.org/Subset/Deal
:Deal rdf:type owl:Class ;
      rdfs:subClassOf [ rdf:type owl:Restriction ;
                        owl:onProperty :mismo-LogicalDataDictionaryIdentifier ;
                        owl:cardinality "1"^^xsd:nonNegativeInteger
                      ] ,
                      [ rdf:type owl:Restriction ;
                        owl:onProperty :mismo-ReferenceModelIdentifier ;
                        owl:cardinality "1"^^xsd:nonNegativeInteger
                      ] ,
                      [ rdf:type owl:Restriction ;
                        owl:onProperty :sequenceNumber ;
                        owl:cardinality "1"^^xsd:nonNegativeInteger
                      ] ,
                      [ rdf:type owl:Restriction ;
                        owl:onProperty :dealChoice1 ;
                        owl:maxCardinality "1"^^xsd:nonNegativeInteger
                      ] ;
      rdfs:comment "The root element for all transactions that apply to the use cases of a single deal. A Deal may contain multiple loans or loan applications."^^xsd:string .


###  http://mismo.org/Subset/DealChoice
:DealChoice rdf:type owl:Class ;
            rdfs:subClassOf [ rdf:type owl:Restriction ;
                              owl:onProperty :dealSequence1 ;
                              owl:maxCardinality "1"^^xsd:nonNegativeInteger
                            ] ,
                            [ rdf:type owl:Restriction ;
                              owl:onProperty :reference ;
                              owl:maxCardinality "1"^^xsd:nonNegativeInteger
                            ] ;
            rdfs:label "Deal Choice"^^xsd:string .


###  http://mismo.org/Subset/DealSequence
:DealSequence rdf:type owl:Class ;
              rdfs:subClassOf [ rdf:type owl:Restriction ;
                                owl:onProperty :assetSummary ;
                                owl:maxCardinality "1"^^xsd:nonNegativeInteger
                              ] ,
                              [ rdf:type owl:Restriction ;
                                owl:onProperty :extension ;
                                owl:maxCardinality "1"^^xsd:nonNegativeInteger
                              ] ,
                              [ rdf:type owl:Restriction ;
                                owl:onProperty :facilitateServicingREO-PurchaseIndicator ;
                                owl:maxCardinality "1"^^xsd:nonNegativeInteger
                              ] ,
                              [ rdf:type owl:Restriction ;
                                owl:onProperty :liabilitySummary ;
                                owl:maxCardinality "1"^^xsd:nonNegativeInteger
                              ] ,
                              [ rdf:type owl:Restriction ;
                                owl:onProperty :mortgageOriginatorFirstTimeHomeBuyerEligibilityIndicator ;
                                owl:maxCardinality "1"^^xsd:nonNegativeInteger
                              ] ;
              rdfs:label "Deal Sequence"^^xsd:string .


###  http://mismo.org/Subset/DealSet
:DealSet rdf:type owl:Class ;
         rdfs:subClassOf [ rdf:type owl:Restriction ;
                           owl:onProperty :sequenceNumber ;
                           owl:cardinality "1"^^xsd:nonNegativeInteger
                         ] ,
                         [ rdf:type owl:Restriction ;
                           owl:onProperty :ach ;
                           owl:maxCardinality "1"^^xsd:nonNegativeInteger
                         ] ,
                         [ rdf:type owl:Restriction ;
                           owl:onProperty :cashRemittanceSummaryNotification ;
                           owl:maxCardinality "1"^^xsd:nonNegativeInteger
                         ] ,
                         [ rdf:type owl:Restriction ;
                           owl:onProperty :extension ;
                           owl:maxCardinality "1"^^xsd:nonNegativeInteger
                         ] ,
                         [ rdf:type owl:Restriction ;
                           owl:onProperty :pool ;
                           owl:maxCardinality "1"^^xsd:nonNegativeInteger
                         ] ,
                         [ rdf:type owl:Restriction ;
                           owl:onProperty :poolBidRequest ;
                           owl:maxCardinality "1"^^xsd:nonNegativeInteger
                         ] ,
                         [ rdf:type owl:Restriction ;
                           owl:onProperty :poolBidResponse ;
                           owl:maxCardinality "1"^^xsd:nonNegativeInteger
                         ] ,
                         [ rdf:type owl:Restriction ;
                           owl:onProperty :servicerReporting ;
                           owl:maxCardinality "1"^^xsd:nonNegativeInteger
                         ] ;
         rdfs:comment "Container for a group of loan deals, sometimes referred to as a \"pool\". A DEAL SET may be used to transfer loans between servicers, or submission to an investor or other purposes."^^xsd:string ;
         rdfs:label "Deal Set"^^xsd:string .


###  http://mismo.org/Subset/FloodDetermination
:FloodDetermination rdf:type owl:Class ;
                    rdfs:subClassOf [ rdf:type owl:Restriction ;
                                      owl:onProperty :floodCertificationIdentifier ;
                                      owl:cardinality "1"^^xsd:nonNegativeInteger
                                    ] ,
                                    [ rdf:type owl:Restriction ;
                                      owl:onProperty :floodDeterminationLifeOfLoanIndicator ;
                                      owl:cardinality "1"^^xsd:nonNegativeInteger
                                    ] ,
                                    [ rdf:type owl:Restriction ;
                                      owl:onProperty :floodDiscrepancyGrandfatheredIndicator ;
                                      owl:cardinality "1"^^xsd:nonNegativeInteger
                                    ] ,
                                    [ rdf:type owl:Restriction ;
                                      owl:onProperty :floodDiscrepancyIndicator ;
                                      owl:cardinality "1"^^xsd:nonNegativeInteger
                                    ] ,
                                    [ rdf:type owl:Restriction ;
                                      owl:onProperty :floodDiscrepancyResolvedIndicator ;
                                      owl:cardinality "1"^^xsd:nonNegativeInteger
                                    ] ,
                                    [ rdf:type owl:Restriction ;
                                      owl:onProperty :floodPartialIndicator ;
                                      owl:cardinality "1"^^xsd:nonNegativeInteger
                                    ] ,
                                    [ rdf:type owl:Restriction ;
                                      owl:onProperty :floodProductCertifyDate ;
                                      owl:cardinality "1"^^xsd:nonNegativeInteger
                                    ] ,
                                    [ rdf:type owl:Restriction ;
                                      owl:onProperty :nfip-CommunityFIRM-Date ;
                                      owl:cardinality "1"^^xsd:nonNegativeInteger
                                    ] ,
                                    [ rdf:type owl:Restriction ;
                                      owl:onProperty :nfip-CommunityIdentifier ;
                                      owl:cardinality "1"^^xsd:nonNegativeInteger
                                    ] ,
                                    [ rdf:type owl:Restriction ;
                                      owl:onProperty :nfip-CommunityName ;
                                      owl:cardinality "1"^^xsd:nonNegativeInteger
                                    ] ,
                                    [ rdf:type owl:Restriction ;
                                      owl:onProperty :nfip-CommunityParticipationStartDate ;
                                      owl:cardinality "1"^^xsd:nonNegativeInteger
                                    ] ,
                                    [ rdf:type owl:Restriction ;
                                      owl:onProperty :nfip-CommunityParticipationStatusType ;
                                      owl:cardinality "1"^^xsd:nonNegativeInteger
                                    ] ,
                                    [ rdf:type owl:Restriction ;
                                      owl:onProperty :nfip-CommunityParticipationStatusTypeOtherDescription ;
                                      owl:cardinality "1"^^xsd:nonNegativeInteger
                                    ] ,
                                    [ rdf:type owl:Restriction ;
                                      owl:onProperty :nfip-CountyName ;
                                      owl:cardinality "1"^^xsd:nonNegativeInteger
                                    ] ,
                                    [ rdf:type owl:Restriction ;
                                      owl:onProperty :nfip-FloodDataRevisionType ;
                                      owl:cardinality "1"^^xsd:nonNegativeInteger
                                    ] ,
                                    [ rdf:type owl:Restriction ;
                                      owl:onProperty :nfip-FloodZoneIdentifier ;
                                      owl:cardinality "1"^^xsd:nonNegativeInteger
                                    ] ,
                                    [ rdf:type owl:Restriction ;
                                      owl:onProperty :nfip-LetterOfMapDate ;
                                      owl:cardinality "1"^^xsd:nonNegativeInteger
                                    ] ,
                                    [ rdf:type owl:Restriction ;
                                      owl:onProperty :nfip-MapIdentifier ;
                                      owl:cardinality "1"^^xsd:nonNegativeInteger
                                    ] ,
                                    [ rdf:type owl:Restriction ;
                                      owl:onProperty :nfip-MapIndicator ;
                                      owl:cardinality "1"^^xsd:nonNegativeInteger
                                    ] ,
                                    [ rdf:type owl:Restriction ;
                                      owl:onProperty :nfip-MapPanelDate ;
                                      owl:cardinality "1"^^xsd:nonNegativeInteger
                                    ] ,
                                    [ rdf:type owl:Restriction ;
                                      owl:onProperty :nfip-MapPanelIdentifier ;
                                      owl:cardinality "1"^^xsd:nonNegativeInteger
                                    ] ,
                                    [ rdf:type owl:Restriction ;
                                      owl:onProperty :nfip-MapPanelSuffixIdentifier ;
                                      owl:cardinality "1"^^xsd:nonNegativeInteger
                                    ] ,
                                    [ rdf:type owl:Restriction ;
                                      owl:onProperty :nfip-StateCode ;
                                      owl:cardinality "1"^^xsd:nonNegativeInteger
                                    ] ,
                                    [ rdf:type owl:Restriction ;
                                      owl:onProperty :protectedAreaDesignationDate ;
                                      owl:cardinality "1"^^xsd:nonNegativeInteger
                                    ] ,
                                    [ rdf:type owl:Restriction ;
                                      owl:onProperty :protectedAreaIndicator ;
                                      owl:cardinality "1"^^xsd:nonNegativeInteger
                                    ] ,
                                    [ rdf:type owl:Restriction ;
                                      owl:onProperty :specialFloodHazardAreaIndicator ;
                                      owl:cardinality "1"^^xsd:nonNegativeInteger
                                    ] ,
                                    [ rdf:type owl:Restriction ;
                                      owl:onProperty :extension ;
                                      owl:maxCardinality "1"^^xsd:nonNegativeInteger
                                    ] ,
                                    [ rdf:type owl:Restriction ;
                                      owl:onProperty :floodRiskFactor ;
                                      owl:maxCardinality "1"^^xsd:nonNegativeInteger
                                    ] ;
                    rdfs:comment "Information specific to the Flood Zone Determination pursuant to the National Flood Insurance Program."^^xsd:string ;
                    rdfs:label "Flood Determination"^^xsd:string .


###  http://mismo.org/Subset/FloodResponse
:FloodResponse rdf:type owl:Class ;
               rdfs:subClassOf [ rdf:type owl:Restriction ;
                                 owl:onProperty :disputeResolutionIndicator ;
                                 owl:cardinality "1"^^xsd:nonNegativeInteger
                               ] ,
                               [ rdf:type owl:Restriction ;
                                 owl:onProperty :fema-AdditionalLenderDescription ;
                                 owl:cardinality "1"^^xsd:nonNegativeInteger
                               ] ,
                               [ rdf:type owl:Restriction ;
                                 owl:onProperty :floodTransactionIdentifier ;
                                 owl:cardinality "1"^^xsd:nonNegativeInteger
                               ] ,
                               [ rdf:type owl:Restriction ;
                                 owl:onProperty :extension ;
                                 owl:maxCardinality "1"^^xsd:nonNegativeInteger
                               ] ,
                               [ rdf:type owl:Restriction ;
                                 owl:onProperty :floodDetermination ;
                                 owl:maxCardinality "1"^^xsd:nonNegativeInteger
                               ] ,
                               [ rdf:type owl:Restriction ;
                                 owl:onProperty :property ;
                                 owl:maxCardinality "1"^^xsd:nonNegativeInteger
                               ] ;
               rdfs:comment "Information about a response regarding a FLOOD certificate and/or insurance."^^xsd:string ;
               rdfs:label "Flood Response"^^xsd:string .


###  http://mismo.org/Subset/FloodRiskFactor
:FloodRiskFactor rdf:type owl:Class ;
                 rdfs:subClassOf [ rdf:type owl:Restriction ;
                                   owl:onProperty :baseFloodElevationLinearMeasure ;
                                   owl:cardinality "1"^^xsd:nonNegativeInteger
                                 ] ,
                                 [ rdf:type owl:Restriction ;
                                   owl:onProperty :floodDepthLinearMeasure ;
                                   owl:cardinality "1"^^xsd:nonNegativeInteger
                                 ] ,
                                 [ rdf:type owl:Restriction ;
                                   owl:onProperty :propertyElevationLinearMeasure ;
                                   owl:cardinality "1"^^xsd:nonNegativeInteger
                                 ] ,
                                 [ rdf:type owl:Restriction ;
                                   owl:onProperty :specialFloodHazardAreaDistanceLinearMeasure ;
                                   owl:cardinality "1"^^xsd:nonNegativeInteger
                                 ] ,
                                 [ rdf:type owl:Restriction ;
                                   owl:onProperty :extension ;
                                   owl:maxCardinality "1"^^xsd:nonNegativeInteger
                                 ] ;
                 rdfs:comment "Information about Risk Factors used in Flood Determination."^^xsd:string ;
                 rdfs:label "Flood Risk Factor"^^xsd:string .


###  http://mismo.org/Subset/HazardInsurance
:HazardInsurance rdf:type owl:Class ;
                 rdfs:subClassOf [ rdf:type owl:Restriction ;
                                   owl:onProperty :floodContractFeeAmount ;
                                   owl:cardinality "1"^^xsd:nonNegativeInteger
                                 ] ,
                                 [ rdf:type owl:Restriction ;
                                   owl:onProperty :hazardInsuranceCoverageAmount ;
                                   owl:cardinality "1"^^xsd:nonNegativeInteger
                                 ] ,
                                 [ rdf:type owl:Restriction ;
                                   owl:onProperty :hazardInsuranceCoverageType ;
                                   owl:cardinality "1"^^xsd:nonNegativeInteger
                                 ] ,
                                 [ rdf:type owl:Restriction ;
                                   owl:onProperty :hazardInsuranceCoverageTypeOtherDescription ;
                                   owl:cardinality "1"^^xsd:nonNegativeInteger
                                 ] ,
                                 [ rdf:type owl:Restriction ;
                                   owl:onProperty :hazardInsuranceEffectiveDate ;
                                   owl:cardinality "1"^^xsd:nonNegativeInteger
                                 ] ,
                                 [ rdf:type owl:Restriction ;
                                   owl:onProperty :hazardInsuranceEscrowedIndicator ;
                                   owl:cardinality "1"^^xsd:nonNegativeInteger
                                 ] ,
                                 [ rdf:type owl:Restriction ;
                                   owl:onProperty :hazardInsuranceExpirationDate ;
                                   owl:cardinality "1"^^xsd:nonNegativeInteger
                                 ] ,
                                 [ rdf:type owl:Restriction ;
                                   owl:onProperty :hazardInsuranceNextPremiumDueDate ;
                                   owl:cardinality "1"^^xsd:nonNegativeInteger
                                 ] ,
                                 [ rdf:type owl:Restriction ;
                                   owl:onProperty :hazardInsuranceNonStandardPolicyType ;
                                   owl:cardinality "1"^^xsd:nonNegativeInteger
                                 ] ,
                                 [ rdf:type owl:Restriction ;
                                   owl:onProperty :hazardInsuranceNonStandardPolicyTypeOtherDescription ;
                                   owl:cardinality "1"^^xsd:nonNegativeInteger
                                 ] ,
                                 [ rdf:type owl:Restriction ;
                                   owl:onProperty :hazardInsurancePolicyCancellationDate ;
                                   owl:cardinality "1"^^xsd:nonNegativeInteger
                                 ] ,
                                 [ rdf:type owl:Restriction ;
                                   owl:onProperty :hazardInsurancePolicyIdentifier ;
                                   owl:cardinality "1"^^xsd:nonNegativeInteger
                                 ] ,
                                 [ rdf:type owl:Restriction ;
                                   owl:onProperty :hazardInsurancePremiumAmount ;
                                   owl:cardinality "1"^^xsd:nonNegativeInteger
                                 ] ,
                                 [ rdf:type owl:Restriction ;
                                   owl:onProperty :hazardInsurancePremiumMonthsCount ;
                                   owl:cardinality "1"^^xsd:nonNegativeInteger
                                 ] ,
                                 [ rdf:type owl:Restriction ;
                                   owl:onProperty :hazardInsuranceReplacementValueIndicator ;
                                   owl:cardinality "1"^^xsd:nonNegativeInteger
                                 ] ,
                                 [ rdf:type owl:Restriction ;
                                   owl:onProperty :insuranceRequiredIndicator ;
                                   owl:cardinality "1"^^xsd:nonNegativeInteger
                                 ] ,
                                 [ rdf:type owl:Restriction ;
                                   owl:onProperty :sequenceNumber ;
                                   owl:cardinality "1"^^xsd:nonNegativeInteger
                                 ] ,
                                 [ rdf:type owl:Restriction ;
                                   owl:onProperty :extension ;
                                   owl:maxCardinality "1"^^xsd:nonNegativeInteger
                                 ] ;
                 rdfs:comment "Information specific to any hazard insurance policy on the property that secures the loan. There may be multiple policies, such as homeowners, fire and extended coverage, flood, wind, or earthquake insurance."^^xsd:string ;
                 rdfs:label "Hazard Insurance"^^xsd:string .


###  http://mismo.org/Subset/Loan
:Loan rdf:type owl:Class ;
      rdfs:subClassOf [ rdf:type owl:Restriction ;
                        owl:onProperty :acceleratedPaymentProgramIndicator ;
                        owl:cardinality "1"^^xsd:nonNegativeInteger
                      ] ,
                      [ rdf:type owl:Restriction ;
                        owl:onProperty :ach-Indicator ;
                        owl:cardinality "1"^^xsd:nonNegativeInteger
                      ] ,
                      [ rdf:type owl:Restriction ;
                        owl:onProperty :activeLitigationIndicator ;
                        owl:cardinality "1"^^xsd:nonNegativeInteger
                      ] ,
                      [ rdf:type owl:Restriction ;
                        owl:onProperty :affordableLoanTotalSubordinateFinancingAmount ;
                        owl:cardinality "1"^^xsd:nonNegativeInteger
                      ] ,
                      [ rdf:type owl:Restriction ;
                        owl:onProperty :applicationReceivedDate ;
                        owl:cardinality "1"^^xsd:nonNegativeInteger
                      ] ,
                      [ rdf:type owl:Restriction ;
                        owl:onProperty :armsLengthIndicator ;
                        owl:cardinality "1"^^xsd:nonNegativeInteger
                      ] ,
                      [ rdf:type owl:Restriction ;
                        owl:onProperty :assumabilityIndicator ;
                        owl:cardinality "1"^^xsd:nonNegativeInteger
                      ] ,
                      [ rdf:type owl:Restriction ;
                        owl:onProperty :assumedIndicator ;
                        owl:cardinality "1"^^xsd:nonNegativeInteger
                      ] ,
                      [ rdf:type owl:Restriction ;
                        owl:onProperty :balloonGuaranteedRefinancingIndicator ;
                        owl:cardinality "1"^^xsd:nonNegativeInteger
                      ] ,
                      [ rdf:type owl:Restriction ;
                        owl:onProperty :balloonIndicator ;
                        owl:cardinality "1"^^xsd:nonNegativeInteger
                      ] ,
                      [ rdf:type owl:Restriction ;
                        owl:onProperty :balloonPaymentAmount ;
                        owl:cardinality "1"^^xsd:nonNegativeInteger
                      ] ,
                      [ rdf:type owl:Restriction ;
                        owl:onProperty :balloonPaymentMaximumAmount ;
                        owl:cardinality "1"^^xsd:nonNegativeInteger
                      ] ,
                      [ rdf:type owl:Restriction ;
                        owl:onProperty :balloonPaymentMinimumAmount ;
                        owl:cardinality "1"^^xsd:nonNegativeInteger
                      ] ,
                      [ rdf:type owl:Restriction ;
                        owl:onProperty :balloonResetIndicator ;
                        owl:cardinality "1"^^xsd:nonNegativeInteger
                      ] ,
                      [ rdf:type owl:Restriction ;
                        owl:onProperty :balloonResetOptionIndicator ;
                        owl:cardinality "1"^^xsd:nonNegativeInteger
                      ] ,
                      [ rdf:type owl:Restriction ;
                        owl:onProperty :belowMarketSubordinateFinancingIndicator ;
                        owl:cardinality "1"^^xsd:nonNegativeInteger
                      ] ,
                      [ rdf:type owl:Restriction ;
                        owl:onProperty :biweeklyToMonthlyOnDefaultIndicator ;
                        owl:cardinality "1"^^xsd:nonNegativeInteger
                      ] ,
                      [ rdf:type owl:Restriction ;
                        owl:onProperty :borrowerCount ;
                        owl:cardinality "1"^^xsd:nonNegativeInteger
                      ] ,
                      [ rdf:type owl:Restriction ;
                        owl:onProperty :buydownTemporarySubsidyFundingIndicator ;
                        owl:cardinality "1"^^xsd:nonNegativeInteger
                      ] ,
                      [ rdf:type owl:Restriction ;
                        owl:onProperty :capitalizedFeesIndicator ;
                        owl:cardinality "1"^^xsd:nonNegativeInteger
                      ] ,
                      [ rdf:type owl:Restriction ;
                        owl:onProperty :capitalizedLoanIndicator ;
                        owl:cardinality "1"^^xsd:nonNegativeInteger
                      ] ,
                      [ rdf:type owl:Restriction ;
                        owl:onProperty :closingCostFinancedIndicator ;
                        owl:cardinality "1"^^xsd:nonNegativeInteger
                      ] ,
                      [ rdf:type owl:Restriction ;
                        owl:onProperty :closingDisclosureWaitingPeriodWaivedIndicator ;
                        owl:cardinality "1"^^xsd:nonNegativeInteger
                      ] ,
                      [ rdf:type owl:Restriction ;
                        owl:onProperty :collateralPledgedToName ;
                        owl:cardinality "1"^^xsd:nonNegativeInteger
                      ] ,
                      [ rdf:type owl:Restriction ;
                        owl:onProperty :concurrentOriginationIndicator ;
                        owl:cardinality "1"^^xsd:nonNegativeInteger
                      ] ,
                      [ rdf:type owl:Restriction ;
                        owl:onProperty :concurrentOriginationLenderIndicator ;
                        owl:cardinality "1"^^xsd:nonNegativeInteger
                      ] ,
                      [ rdf:type owl:Restriction ;
                        owl:onProperty :conformingIndicator ;
                        owl:cardinality "1"^^xsd:nonNegativeInteger
                      ] ,
                      [ rdf:type owl:Restriction ;
                        owl:onProperty :constructionLoanIndicator ;
                        owl:cardinality "1"^^xsd:nonNegativeInteger
                      ] ,
                      [ rdf:type owl:Restriction ;
                        owl:onProperty :conversionOfContractForDeedIndicator ;
                        owl:cardinality "1"^^xsd:nonNegativeInteger
                      ] ,
                      [ rdf:type owl:Restriction ;
                        owl:onProperty :convertibleIndicator ;
                        owl:cardinality "1"^^xsd:nonNegativeInteger
                      ] ,
                      [ rdf:type owl:Restriction ;
                        owl:onProperty :correspondentAcquisitionType ;
                        owl:cardinality "1"^^xsd:nonNegativeInteger
                      ] ,
                      [ rdf:type owl:Restriction ;
                        owl:onProperty :correspondentAcquisitionTypeOtherDescription ;
                        owl:cardinality "1"^^xsd:nonNegativeInteger
                      ] ,
                      [ rdf:type owl:Restriction ;
                        owl:onProperty :creditEnhancementIndicator ;
                        owl:cardinality "1"^^xsd:nonNegativeInteger
                      ] ,
                      [ rdf:type owl:Restriction ;
                        owl:onProperty :creditorServicingOfLoanStatementType ;
                        owl:cardinality "1"^^xsd:nonNegativeInteger
                      ] ,
                      [ rdf:type owl:Restriction ;
                        owl:onProperty :creditorServicingOfLoanStatementTypeOtherDescription ;
                        owl:cardinality "1"^^xsd:nonNegativeInteger
                      ] ,
                      [ rdf:type owl:Restriction ;
                        owl:onProperty :currentInterestRatePercent ;
                        owl:cardinality "1"^^xsd:nonNegativeInteger
                      ] ,
                      [ rdf:type owl:Restriction ;
                        owl:onProperty :deferredInterestBalanceAmount ;
                        owl:cardinality "1"^^xsd:nonNegativeInteger
                      ] ,
                      [ rdf:type owl:Restriction ;
                        owl:onProperty :delegatedUnderwritingIndicator ;
                        owl:cardinality "1"^^xsd:nonNegativeInteger
                      ] ,
                      [ rdf:type owl:Restriction ;
                        owl:onProperty :demandFeatureIndicator ;
                        owl:cardinality "1"^^xsd:nonNegativeInteger
                      ] ,
                      [ rdf:type owl:Restriction ;
                        owl:onProperty :eligibleForLenderPaidMI-Indicator ;
                        owl:cardinality "1"^^xsd:nonNegativeInteger
                      ] ,
                      [ rdf:type owl:Restriction ;
                        owl:onProperty :employeeLoanProgramIndicator ;
                        owl:cardinality "1"^^xsd:nonNegativeInteger
                      ] ,
                      [ rdf:type owl:Restriction ;
                        owl:onProperty :energyRelatedImprovementsIndicator ;
                        owl:cardinality "1"^^xsd:nonNegativeInteger
                      ] ,
                      [ rdf:type owl:Restriction ;
                        owl:onProperty :enoteCertifiedIndicator ;
                        owl:cardinality "1"^^xsd:nonNegativeInteger
                      ] ,
                      [ rdf:type owl:Restriction ;
                        owl:onProperty :enoteIndicator ;
                        owl:cardinality "1"^^xsd:nonNegativeInteger
                      ] ,
                      [ rdf:type owl:Restriction ;
                        owl:onProperty :escrowAbsenceReasonType ;
                        owl:cardinality "1"^^xsd:nonNegativeInteger
                      ] ,
                      [ rdf:type owl:Restriction ;
                        owl:onProperty :escrowAbsenceReasonTypeOtherDescription ;
                        owl:cardinality "1"^^xsd:nonNegativeInteger
                      ] ,
                      [ rdf:type owl:Restriction ;
                        owl:onProperty :escrowAccountLenderRequirementType ;
                        owl:cardinality "1"^^xsd:nonNegativeInteger
                      ] ,
                      [ rdf:type owl:Restriction ;
                        owl:onProperty :escrowAccountRequestedIndicator ;
                        owl:cardinality "1"^^xsd:nonNegativeInteger
                      ] ,
                      [ rdf:type owl:Restriction ;
                        owl:onProperty :escrowIndicator ;
                        owl:cardinality "1"^^xsd:nonNegativeInteger
                      ] ,
                      [ rdf:type owl:Restriction ;
                        owl:onProperty :escrowNotAllowedIndicator ;
                        owl:cardinality "1"^^xsd:nonNegativeInteger
                      ] ,
                      [ rdf:type owl:Restriction ;
                        owl:onProperty :escrowsElectedByBorrowerIndicator ;
                        owl:cardinality "1"^^xsd:nonNegativeInteger
                      ] ,
                      [ rdf:type owl:Restriction ;
                        owl:onProperty :heloc-Indicator ;
                        owl:cardinality "1"^^xsd:nonNegativeInteger
                      ] ,
                      [ rdf:type owl:Restriction ;
                        owl:onProperty :higherPricedMortgageLoanIndicator ;
                        owl:cardinality "1"^^xsd:nonNegativeInteger
                      ] ,
                      [ rdf:type owl:Restriction ;
                        owl:onProperty :homeBuyersHomeownershipEducationCertificateIndicator ;
                        owl:cardinality "1"^^xsd:nonNegativeInteger
                      ] ,
                      [ rdf:type owl:Restriction ;
                        owl:onProperty :ineligibleLoanProductIndicator ;
                        owl:cardinality "1"^^xsd:nonNegativeInteger
                      ] ,
                      [ rdf:type owl:Restriction ;
                        owl:onProperty :initialFixedPeriodEffectiveMonthsCount ;
                        owl:cardinality "1"^^xsd:nonNegativeInteger
                      ] ,
                      [ rdf:type owl:Restriction ;
                        owl:onProperty :interestCreditedToBorrowerIndicator ;
                        owl:cardinality "1"^^xsd:nonNegativeInteger
                      ] ,
                      [ rdf:type owl:Restriction ;
                        owl:onProperty :interestOnlyIndicator ;
                        owl:cardinality "1"^^xsd:nonNegativeInteger
                      ] ,
                      [ rdf:type owl:Restriction ;
                        owl:onProperty :interestRateIncreaseIndicator ;
                        owl:cardinality "1"^^xsd:nonNegativeInteger
                      ] ,
                      [ rdf:type owl:Restriction ;
                        owl:onProperty :jurisdictionHighCostLoanIndicator ;
                        owl:cardinality "1"^^xsd:nonNegativeInteger
                      ] ,
                      [ rdf:type owl:Restriction ;
                        owl:onProperty :lenderPlacedHazardInsuranceIndicator ;
                        owl:cardinality "1"^^xsd:nonNegativeInteger
                      ] ,
                      [ rdf:type owl:Restriction ;
                        owl:onProperty :lenderSelfInsuredIndicator ;
                        owl:cardinality "1"^^xsd:nonNegativeInteger
                      ] ,
                      [ rdf:type owl:Restriction ;
                        owl:onProperty :lendingLimitAmount ;
                        owl:cardinality "1"^^xsd:nonNegativeInteger
                      ] ,
                      [ rdf:type owl:Restriction ;
                        owl:onProperty :lendingLimitType ;
                        owl:cardinality "1"^^xsd:nonNegativeInteger
                      ] ,
                      [ rdf:type owl:Restriction ;
                        owl:onProperty :lendingLimitTypeOtherDescription ;
                        owl:cardinality "1"^^xsd:nonNegativeInteger
                      ] ,
                      [ rdf:type owl:Restriction ;
                        owl:onProperty :lienHolderSameAsSubjectLoanIndicator ;
                        owl:cardinality "1"^^xsd:nonNegativeInteger
                      ] ,
                      [ rdf:type owl:Restriction ;
                        owl:onProperty :loanAffordableIndicator ;
                        owl:cardinality "1"^^xsd:nonNegativeInteger
                      ] ,
                      [ rdf:type owl:Restriction ;
                        owl:onProperty :loanAgeMonthsCount ;
                        owl:cardinality "1"^^xsd:nonNegativeInteger
                      ] ,
                      [ rdf:type owl:Restriction ;
                        owl:onProperty :loanAmountIncreaseIndicator ;
                        owl:cardinality "1"^^xsd:nonNegativeInteger
                      ] ,
                      [ rdf:type owl:Restriction ;
                        owl:onProperty :loanApprovalDate ;
                        owl:cardinality "1"^^xsd:nonNegativeInteger
                      ] ,
                      [ rdf:type owl:Restriction ;
                        owl:onProperty :loanApprovalExpirationDate ;
                        owl:cardinality "1"^^xsd:nonNegativeInteger
                      ] ,
                      [ rdf:type owl:Restriction ;
                        owl:onProperty :loanApprovalPeriodDaysCount ;
                        owl:cardinality "1"^^xsd:nonNegativeInteger
                      ] ,
                      [ rdf:type owl:Restriction ;
                        owl:onProperty :loanAssetAddedIndicator ;
                        owl:cardinality "1"^^xsd:nonNegativeInteger
                      ] ,
                      [ rdf:type owl:Restriction ;
                        owl:onProperty :loanClosingStatusType ;
                        owl:cardinality "1"^^xsd:nonNegativeInteger
                      ] ,
                      [ rdf:type owl:Restriction ;
                        owl:onProperty :loanCommitmentDate ;
                        owl:cardinality "1"^^xsd:nonNegativeInteger
                      ] ,
                      [ rdf:type owl:Restriction ;
                        owl:onProperty :loanCommitmentExpirationDate ;
                        owl:cardinality "1"^^xsd:nonNegativeInteger
                      ] ,
                      [ rdf:type owl:Restriction ;
                        owl:onProperty :loanCommitmentPeriodDaysCount ;
                        owl:cardinality "1"^^xsd:nonNegativeInteger
                      ] ,
                      [ rdf:type owl:Restriction ;
                        owl:onProperty :loanEstimateWaitingPeriodWaivedIndicator ;
                        owl:cardinality "1"^^xsd:nonNegativeInteger
                      ] ,
                      [ rdf:type owl:Restriction ;
                        owl:onProperty :loanFundingDate ;
                        owl:cardinality "1"^^xsd:nonNegativeInteger
                      ] ,
                      [ rdf:type owl:Restriction ;
                        owl:onProperty :loanLevelCreditScoreIndicator ;
                        owl:cardinality "1"^^xsd:nonNegativeInteger
                      ] ,
                      [ rdf:type owl:Restriction ;
                        owl:onProperty :loanRepaymentType ;
                        owl:cardinality "1"^^xsd:nonNegativeInteger
                      ] ,
                      [ rdf:type owl:Restriction ;
                        owl:onProperty :loanRepaymentTypeOtherDescription ;
                        owl:cardinality "1"^^xsd:nonNegativeInteger
                      ] ,
                      [ rdf:type owl:Restriction ;
                        owl:onProperty :loanSaleFundingDate ;
                        owl:cardinality "1"^^xsd:nonNegativeInteger
                      ] ,
                      [ rdf:type owl:Restriction ;
                        owl:onProperty :loanSecuredByType ;
                        owl:cardinality "1"^^xsd:nonNegativeInteger
                      ] ,
                      [ rdf:type owl:Restriction ;
                        owl:onProperty :loanSecuredByTypeOtherDescription ;
                        owl:cardinality "1"^^xsd:nonNegativeInteger
                      ] ,
                      [ rdf:type owl:Restriction ;
                        owl:onProperty :loanSecuredIndicator ;
                        owl:cardinality "1"^^xsd:nonNegativeInteger
                      ] ,
                      [ rdf:type owl:Restriction ;
                        owl:onProperty :loanSellerProvidedInvestmentRatingDescription ;
                        owl:cardinality "1"^^xsd:nonNegativeInteger
                      ] ,
                      [ rdf:type owl:Restriction ;
                        owl:onProperty :lostNoteAffidavitIndicator ;
                        owl:cardinality "1"^^xsd:nonNegativeInteger
                      ] ,
                      [ rdf:type owl:Restriction ;
                        owl:onProperty :mi-CoverageExistsIndicator ;
                        owl:cardinality "1"^^xsd:nonNegativeInteger
                      ] ,
                      [ rdf:type owl:Restriction ;
                        owl:onProperty :mi-RequiredIndicator ;
                        owl:cardinality "1"^^xsd:nonNegativeInteger
                      ] ,
                      [ rdf:type owl:Restriction ;
                        owl:onProperty :mortgageModificationIndicator ;
                        owl:cardinality "1"^^xsd:nonNegativeInteger
                      ] ,
                      [ rdf:type owl:Restriction ;
                        owl:onProperty :negativeAmortizationIndicator ;
                        owl:cardinality "1"^^xsd:nonNegativeInteger
                      ] ,
                      [ rdf:type owl:Restriction ;
                        owl:onProperty :openEndCreditIndicator ;
                        owl:cardinality "1"^^xsd:nonNegativeInteger
                      ] ,
                      [ rdf:type owl:Restriction ;
                        owl:onProperty :originalLoanStandardEscrowProvisionsIndicator ;
                        owl:cardinality "1"^^xsd:nonNegativeInteger
                      ] ,
                      [ rdf:type owl:Restriction ;
                        owl:onProperty :overdueInterestAmount ;
                        owl:cardinality "1"^^xsd:nonNegativeInteger
                      ] ,
                      [ rdf:type owl:Restriction ;
                        owl:onProperty :pace-LoanPayoffAmount ;
                        owl:cardinality "1"^^xsd:nonNegativeInteger
                      ] ,
                      [ rdf:type owl:Restriction ;
                        owl:onProperty :paymentIncreaseIndicator ;
                        owl:cardinality "1"^^xsd:nonNegativeInteger
                      ] ,
                      [ rdf:type owl:Restriction ;
                        owl:onProperty :piggybackLoanIndicator ;
                        owl:cardinality "1"^^xsd:nonNegativeInteger
                      ] ,
                      [ rdf:type owl:Restriction ;
                        owl:onProperty :poolIdentifier ;
                        owl:cardinality "1"^^xsd:nonNegativeInteger
                      ] ,
                      [ rdf:type owl:Restriction ;
                        owl:onProperty :poolIssueDate ;
                        owl:cardinality "1"^^xsd:nonNegativeInteger
                      ] ,
                      [ rdf:type owl:Restriction ;
                        owl:onProperty :poolPrefixIdentifier ;
                        owl:cardinality "1"^^xsd:nonNegativeInteger
                      ] ,
                      [ rdf:type owl:Restriction ;
                        owl:onProperty :prepaymentPenaltyIndicator ;
                        owl:cardinality "1"^^xsd:nonNegativeInteger
                      ] ,
                      [ rdf:type owl:Restriction ;
                        owl:onProperty :prepaymentPenaltyWaivedIndicator ;
                        owl:cardinality "1"^^xsd:nonNegativeInteger
                      ] ,
                      [ rdf:type owl:Restriction ;
                        owl:onProperty :prepaymentRestrictionIndicator ;
                        owl:cardinality "1"^^xsd:nonNegativeInteger
                      ] ,
                      [ rdf:type owl:Restriction ;
                        owl:onProperty :propertiesFinancedByLenderCount ;
                        owl:cardinality "1"^^xsd:nonNegativeInteger
                      ] ,
                      [ rdf:type owl:Restriction ;
                        owl:onProperty :propertyInspectionWaiverIndicator ;
                        owl:cardinality "1"^^xsd:nonNegativeInteger
                      ] ,
                      [ rdf:type owl:Restriction ;
                        owl:onProperty :qualifiedMortgageIndicator ;
                        owl:cardinality "1"^^xsd:nonNegativeInteger
                      ] ,
                      [ rdf:type owl:Restriction ;
                        owl:onProperty :recoverableCorporateAdvanceBalanceFromBorrowerAmount ;
                        owl:cardinality "1"^^xsd:nonNegativeInteger
                      ] ,
                      [ rdf:type owl:Restriction ;
                        owl:onProperty :recoverableCorporateAdvanceBalanceFromThirdPartyAmount ;
                        owl:cardinality "1"^^xsd:nonNegativeInteger
                      ] ,
                      [ rdf:type owl:Restriction ;
                        owl:onProperty :refundOfOverpaidInterestCalendarYearAmount ;
                        owl:cardinality "1"^^xsd:nonNegativeInteger
                      ] ,
                      [ rdf:type owl:Restriction ;
                        owl:onProperty :regulationZHighCostLoanIndicator ;
                        owl:cardinality "1"^^xsd:nonNegativeInteger
                      ] ,
                      [ rdf:type owl:Restriction ;
                        owl:onProperty :relocationLoanIndicator ;
                        owl:cardinality "1"^^xsd:nonNegativeInteger
                      ] ,
                      [ rdf:type owl:Restriction ;
                        owl:onProperty :remainingUnearnedInterestAmount ;
                        owl:cardinality "1"^^xsd:nonNegativeInteger
                      ] ,
                      [ rdf:type owl:Restriction ;
                        owl:onProperty :remoteOnlineNotarizationIndicator ;
                        owl:cardinality "1"^^xsd:nonNegativeInteger
                      ] ,
                      [ rdf:type owl:Restriction ;
                        owl:onProperty :renovationLoanIndicator ;
                        owl:cardinality "1"^^xsd:nonNegativeInteger
                      ] ,
                      [ rdf:type owl:Restriction ;
                        owl:onProperty :rescindableTransactionIndicator ;
                        owl:cardinality "1"^^xsd:nonNegativeInteger
                      ] ,
                      [ rdf:type owl:Restriction ;
                        owl:onProperty :respa-ConformingYearType ;
                        owl:cardinality "1"^^xsd:nonNegativeInteger
                      ] ,
                      [ rdf:type owl:Restriction ;
                        owl:onProperty :respa-ConformingYearTypeOtherDescription ;
                        owl:cardinality "1"^^xsd:nonNegativeInteger
                      ] ,
                      [ rdf:type owl:Restriction ;
                        owl:onProperty :reverseMortgageIndicator ;
                        owl:cardinality "1"^^xsd:nonNegativeInteger
                      ] ,
                      [ rdf:type owl:Restriction ;
                        owl:onProperty :rightOfRescissionWaitingPeriodWaivedIndicator ;
                        owl:cardinality "1"^^xsd:nonNegativeInteger
                      ] ,
                      [ rdf:type owl:Restriction ;
                        owl:onProperty :scra-Indicator ;
                        owl:cardinality "1"^^xsd:nonNegativeInteger
                      ] ,
                      [ rdf:type owl:Restriction ;
                        owl:onProperty :scra-ReliefForbearanceRequestedIndicator ;
                        owl:cardinality "1"^^xsd:nonNegativeInteger
                      ] ,
                      [ rdf:type owl:Restriction ;
                        owl:onProperty :scra-ReliefStatusType ;
                        owl:cardinality "1"^^xsd:nonNegativeInteger
                      ] ,
                      [ rdf:type owl:Restriction ;
                        owl:onProperty :scra-ReliefStatusTypeOtherDescription ;
                        owl:cardinality "1"^^xsd:nonNegativeInteger
                      ] ,
                      [ rdf:type owl:Restriction ;
                        owl:onProperty :seasonalPaymentFeatureDescription ;
                        owl:cardinality "1"^^xsd:nonNegativeInteger
                      ] ,
                      [ rdf:type owl:Restriction ;
                        owl:onProperty :seasonalPaymentFeatureIndicator ;
                        owl:cardinality "1"^^xsd:nonNegativeInteger
                      ] ,
                      [ rdf:type owl:Restriction ;
                        owl:onProperty :sequenceNumber ;
                        owl:cardinality "1"^^xsd:nonNegativeInteger
                      ] ,
                      [ rdf:type owl:Restriction ;
                        owl:onProperty :servicingTransferProhibitedIndicator ;
                        owl:cardinality "1"^^xsd:nonNegativeInteger
                      ] ,
                      [ rdf:type owl:Restriction ;
                        owl:onProperty :servicingTransferStatusType ;
                        owl:cardinality "1"^^xsd:nonNegativeInteger
                      ] ,
                      [ rdf:type owl:Restriction ;
                        owl:onProperty :sharedAppreciationIndicator ;
                        owl:cardinality "1"^^xsd:nonNegativeInteger
                      ] ,
                      [ rdf:type owl:Restriction ;
                        owl:onProperty :sharedEquityAmount ;
                        owl:cardinality "1"^^xsd:nonNegativeInteger
                      ] ,
                      [ rdf:type owl:Restriction ;
                        owl:onProperty :sharedEquityIndicator ;
                        owl:cardinality "1"^^xsd:nonNegativeInteger
                      ] ,
                      [ rdf:type owl:Restriction ;
                        owl:onProperty :signedAuthorizationToRequestTaxRecordsIndicator ;
                        owl:cardinality "1"^^xsd:nonNegativeInteger
                      ] ,
                      [ rdf:type owl:Restriction ;
                        owl:onProperty :stepPaymentsFeatureDescription ;
                        owl:cardinality "1"^^xsd:nonNegativeInteger
                      ] ,
                      [ rdf:type owl:Restriction ;
                        owl:onProperty :subordinateFinancingIsNewIndicator ;
                        owl:cardinality "1"^^xsd:nonNegativeInteger
                      ] ,
                      [ rdf:type owl:Restriction ;
                        owl:onProperty :taxRecordsObtainedIndicator ;
                        owl:cardinality "1"^^xsd:nonNegativeInteger
                      ] ,
                      [ rdf:type owl:Restriction ;
                        owl:onProperty :thirdPartyReviewIndicator ;
                        owl:cardinality "1"^^xsd:nonNegativeInteger
                      ] ,
                      [ rdf:type owl:Restriction ;
                        owl:onProperty :timelyPaymentRateReductionIndicator ;
                        owl:cardinality "1"^^xsd:nonNegativeInteger
                      ] ,
                      [ rdf:type owl:Restriction ;
                        owl:onProperty :totalFinancedEnergyImprovementsAmount ;
                        owl:cardinality "1"^^xsd:nonNegativeInteger
                      ] ,
                      [ rdf:type owl:Restriction ;
                        owl:onProperty :totalMortgagedPropertiesCount ;
                        owl:cardinality "1"^^xsd:nonNegativeInteger
                      ] ,
                      [ rdf:type owl:Restriction ;
                        owl:onProperty :totalSalesConcessionAmount ;
                        owl:cardinality "1"^^xsd:nonNegativeInteger
                      ] ,
                      [ rdf:type owl:Restriction ;
                        owl:onProperty :totalSeniorFinancingAmount ;
                        owl:cardinality "1"^^xsd:nonNegativeInteger
                      ] ,
                      [ rdf:type owl:Restriction ;
                        owl:onProperty :totalSubordinateFinancingAmount ;
                        owl:cardinality "1"^^xsd:nonNegativeInteger
                      ] ,
                      [ rdf:type owl:Restriction ;
                        owl:onProperty :totalSubordinateFinancingProceedsAppliedAmount ;
                        owl:cardinality "1"^^xsd:nonNegativeInteger
                      ] ,
                      [ rdf:type owl:Restriction ;
                        owl:onProperty :trid-RuleIndicator ;
                        owl:cardinality "1"^^xsd:nonNegativeInteger
                      ] ,
                      [ rdf:type owl:Restriction ;
                        owl:onProperty :warehouseLenderIndicator ;
                        owl:cardinality "1"^^xsd:nonNegativeInteger
                      ] ,
                      [ rdf:type owl:Restriction ;
                        owl:onProperty :workoutActiveIndicator ;
                        owl:cardinality "1"^^xsd:nonNegativeInteger
                      ] ,
                      [ rdf:type owl:Restriction ;
                        owl:onProperty :ach ;
                        owl:maxCardinality "1"^^xsd:nonNegativeInteger
                      ] ,
                      [ rdf:type owl:Restriction ;
                        owl:onProperty :adjustment ;
                        owl:maxCardinality "1"^^xsd:nonNegativeInteger
                      ] ,
                      [ rdf:type owl:Restriction ;
                        owl:onProperty :affordableLending ;
                        owl:maxCardinality "1"^^xsd:nonNegativeInteger
                      ] ,
                      [ rdf:type owl:Restriction ;
                        owl:onProperty :amortization ;
                        owl:maxCardinality "1"^^xsd:nonNegativeInteger
                      ] ,
                      [ rdf:type owl:Restriction ;
                        owl:onProperty :assumability ;
                        owl:maxCardinality "1"^^xsd:nonNegativeInteger
                      ] ,
                      [ rdf:type owl:Restriction ;
                        owl:onProperty :billingAddress ;
                        owl:maxCardinality "1"^^xsd:nonNegativeInteger
                      ] ,
                      [ rdf:type owl:Restriction ;
                        owl:onProperty :buydown ;
                        owl:maxCardinality "1"^^xsd:nonNegativeInteger
                      ] ,
                      [ rdf:type owl:Restriction ;
                        owl:onProperty :capitalizationSummary ;
                        owl:maxCardinality "1"^^xsd:nonNegativeInteger
                      ] ,
                      [ rdf:type owl:Restriction ;
                        owl:onProperty :chargeOff ;
                        owl:maxCardinality "1"^^xsd:nonNegativeInteger
                      ] ,
                      [ rdf:type owl:Restriction ;
                        owl:onProperty :closingInformation ;
                        owl:maxCardinality "1"^^xsd:nonNegativeInteger
                      ] ,
                      [ rdf:type owl:Restriction ;
                        owl:onProperty :construction ;
                        owl:maxCardinality "1"^^xsd:nonNegativeInteger
                      ] ,
                      [ rdf:type owl:Restriction ;
                        owl:onProperty :draw ;
                        owl:maxCardinality "1"^^xsd:nonNegativeInteger
                      ] ,
                      [ rdf:type owl:Restriction ;
                        owl:onProperty :escrow ;
                        owl:maxCardinality "1"^^xsd:nonNegativeInteger
                      ] ,
                      [ rdf:type owl:Restriction ;
                        owl:onProperty :extension ;
                        owl:maxCardinality "1"^^xsd:nonNegativeInteger
                      ] ,
                      [ rdf:type owl:Restriction ;
                        owl:onProperty :feeInformation ;
                        owl:maxCardinality "1"^^xsd:nonNegativeInteger
                      ] ,
                      [ rdf:type owl:Restriction ;
                        owl:onProperty :governmentLoan ;
                        owl:maxCardinality "1"^^xsd:nonNegativeInteger
                      ] ,
                      [ rdf:type owl:Restriction ;
                        owl:onProperty :heloc ;
                        owl:maxCardinality "1"^^xsd:nonNegativeInteger
                      ] ,
                      [ rdf:type owl:Restriction ;
                        owl:onProperty :hmdaLoan ;
                        owl:maxCardinality "1"^^xsd:nonNegativeInteger
                      ] ,
                      [ rdf:type owl:Restriction ;
                        owl:onProperty :housingExpenseSummary ;
                        owl:maxCardinality "1"^^xsd:nonNegativeInteger
                      ] ,
                      [ rdf:type owl:Restriction ;
                        owl:onProperty :interestCalculation ;
                        owl:maxCardinality "1"^^xsd:nonNegativeInteger
                      ] ,
                      [ rdf:type owl:Restriction ;
                        owl:onProperty :interestOnly ;
                        owl:maxCardinality "1"^^xsd:nonNegativeInteger
                      ] ,
                      [ rdf:type owl:Restriction ;
                        owl:onProperty :investorLoanInformation ;
                        owl:maxCardinality "1"^^xsd:nonNegativeInteger
                      ] ,
                      [ rdf:type owl:Restriction ;
                        owl:onProperty :lateCharge ;
                        owl:maxCardinality "1"^^xsd:nonNegativeInteger
                      ] ,
                      [ rdf:type owl:Restriction ;
                        owl:onProperty :loanLevelCredit ;
                        owl:maxCardinality "1"^^xsd:nonNegativeInteger
                      ] ,
                      [ rdf:type owl:Restriction ;
                        owl:onProperty :loanProduct ;
                        owl:maxCardinality "1"^^xsd:nonNegativeInteger
                      ] ,
                      [ rdf:type owl:Restriction ;
                        owl:onProperty :loanState ;
                        owl:maxCardinality "1"^^xsd:nonNegativeInteger
                      ] ,
                      [ rdf:type owl:Restriction ;
                        owl:onProperty :ltv ;
                        owl:maxCardinality "1"^^xsd:nonNegativeInteger
                      ] ,
                      [ rdf:type owl:Restriction ;
                        owl:onProperty :maturity ;
                        owl:maxCardinality "1"^^xsd:nonNegativeInteger
                      ] ,
                      [ rdf:type owl:Restriction ;
                        owl:onProperty :miData ;
                        owl:maxCardinality "1"^^xsd:nonNegativeInteger
                      ] ,
                      [ rdf:type owl:Restriction ;
                        owl:onProperty :modificationSummary ;
                        owl:maxCardinality "1"^^xsd:nonNegativeInteger
                      ] ,
                      [ rdf:type owl:Restriction ;
                        owl:onProperty :negativeAmortization ;
                        owl:maxCardinality "1"^^xsd:nonNegativeInteger
                      ] ,
                      [ rdf:type owl:Restriction ;
                        owl:onProperty :optionalProductSummary ;
                        owl:maxCardinality "1"^^xsd:nonNegativeInteger
                      ] ,
                      [ rdf:type owl:Restriction ;
                        owl:onProperty :payment ;
                        owl:maxCardinality "1"^^xsd:nonNegativeInteger
                      ] ,
                      [ rdf:type owl:Restriction ;
                        owl:onProperty :prepaymentPenalty ;
                        owl:maxCardinality "1"^^xsd:nonNegativeInteger
                      ] ,
                      [ rdf:type owl:Restriction ;
                        owl:onProperty :purchaseCreditSummary ;
                        owl:maxCardinality "1"^^xsd:nonNegativeInteger
                      ] ,
                      [ rdf:type owl:Restriction ;
                        owl:onProperty :qualification ;
                        owl:maxCardinality "1"^^xsd:nonNegativeInteger
                      ] ,
                      [ rdf:type owl:Restriction ;
                        owl:onProperty :qualifiedMortgage ;
                        owl:maxCardinality "1"^^xsd:nonNegativeInteger
                      ] ,
                      [ rdf:type owl:Restriction ;
                        owl:onProperty :refinance ;
                        owl:maxCardinality "1"^^xsd:nonNegativeInteger
                      ] ,
                      [ rdf:type owl:Restriction ;
                        owl:onProperty :rehabilitation ;
                        owl:maxCardinality "1"^^xsd:nonNegativeInteger
                      ] ,
                      [ rdf:type owl:Restriction ;
                        owl:onProperty :reverseMortgage ;
                        owl:maxCardinality "1"^^xsd:nonNegativeInteger
                      ] ,
                      [ rdf:type owl:Restriction ;
                        owl:onProperty :servicing ;
                        owl:maxCardinality "1"^^xsd:nonNegativeInteger
                      ] ,
                      [ rdf:type owl:Restriction ;
                        owl:onProperty :termsOfLoan ;
                        owl:maxCardinality "1"^^xsd:nonNegativeInteger
                      ] ,
                      [ rdf:type owl:Restriction ;
                        owl:onProperty :treasuryNpv ;
                        owl:maxCardinality "1"^^xsd:nonNegativeInteger
                      ] ,
                      [ rdf:type owl:Restriction ;
                        owl:onProperty :underwriting ;
                        owl:maxCardinality "1"^^xsd:nonNegativeInteger
                      ] ,
                      [ rdf:type owl:Restriction ;
                        owl:onProperty :workoutSummary ;
                        owl:maxCardinality "1"^^xsd:nonNegativeInteger
                      ] ,
                      [ rdf:type owl:Restriction ;
                        owl:onProperty :loanRoleType ;
                        owl:qualifiedCardinality "1"^^xsd:nonNegativeInteger ;
                        owl:onDataRange <http://mismo.org/EnumeratedTypes/LoanRoleBase>
                      ] ,
                      [ rdf:type owl:Restriction ;
                        owl:onProperty :selectionType ;
                        owl:qualifiedCardinality "1"^^xsd:nonNegativeInteger ;
                        owl:onDataRange <http://mismo.org/EnumeratedTypes/SelectionBase>
                      ] ;
      rdfs:comment "Information specific to a mortgage loan agreement between one or more borrowers and a mortgage lender."^^xsd:string .


###  http://mismo.org/Subset/MISMOAmount
:MISMOAmount rdf:type owl:Class ;
             rdfs:subClassOf <http://mismo.org/DataTypes/MISMOAmount_Base> ,
                             [ rdf:type owl:Restriction ;
                               owl:onProperty :CurrencyURI ;
                               owl:cardinality "1"^^xsd:nonNegativeInteger
                             ] ,
                             [ rdf:type owl:Restriction ;
                               owl:onProperty :DataNotSuppliedReasonTypeAdditionalDescription ;
                               owl:cardinality "1"^^xsd:nonNegativeInteger
                             ] ,
                             [ rdf:type owl:Restriction ;
                               owl:onProperty :DataNotSuppliedReasonTypeOtherDescription ;
                               owl:cardinality "1"^^xsd:nonNegativeInteger
                             ] ,
                             [ rdf:type owl:Restriction ;
                               owl:onProperty :SensitiveIndicator ;
                               owl:cardinality "1"^^xsd:nonNegativeInteger
                             ] ,
                             [ rdf:type owl:Restriction ;
                               owl:onProperty :DataNotSuppliedReasonType ;
                               owl:qualifiedCardinality "1"^^xsd:nonNegativeInteger ;
                               owl:onDataRange <http://mismo.org/DataTypes/DataNotSuppliedReasonBase>
                             ] ;
             rdfs:comment """A data type of Amount SHOULD identify a number value that is an amount of money and MAY have a CurrencyURI attribute. It SHALL NOT contain any punctuation other than the decimal point or sign values. The decimal point is ALWAYS the US nationalization character (.) in the designated character encoding (UTF-8 assumed when not stated )
It SHOULD be able to contain at least 18 digits.
EXAMPLE: An Unpaid Principle Balance Amount of $100,000.12 would be expressed as \"100000.12\"."""^^xsd:string .


###  http://mismo.org/Subset/MISMODate
:MISMODate rdf:type owl:Class ;
           rdfs:subClassOf <http://mismo.org/DataTypes/MISMODate_Base> ,
                           [ rdf:type owl:Restriction ;
                             owl:onProperty :DataNotSuppliedReasonTypeAdditionalDescription ;
                             owl:cardinality "1"^^xsd:nonNegativeInteger
                           ] ,
                           [ rdf:type owl:Restriction ;
                             owl:onProperty :DataNotSuppliedReasonTypeOtherDescription ;
                             owl:cardinality "1"^^xsd:nonNegativeInteger
                           ] ,
                           [ rdf:type owl:Restriction ;
                             owl:onProperty :SensitiveIndicator ;
                             owl:cardinality "1"^^xsd:nonNegativeInteger
                           ] ,
                           [ rdf:type owl:Restriction ;
                             owl:onProperty :DataNotSuppliedReasonType ;
                             owl:qualifiedCardinality "1"^^xsd:nonNegativeInteger ;
                             owl:onDataRange <http://mismo.org/DataTypes/DataNotSuppliedReasonBase>
                           ] ;
           rdfs:comment """A data type of Date SHOULD identify a data point that represents numerically a specific year, month and year, or day month and year of the Gregorian Calendar.
Full dates MUST be represented in the extended format CCYY-MM-DD
CCYY is a four-digit year, \"0001\" through \"9999\"
MM is a two-digit month of that year, \"01\" through \"12\"
DD is a two-digit day of that month, \"01\" through \"31\"
Padded zeros must be used.
- is the required separator between CCYY-MM-DD
if the day or month and day are dropped, the preceding separator is also dropped
an optional trailing time zone indicator is permitted using either Z (for Coordinated Universal Time UTC) or an offset from UTC using +hh:mm or -hh:mm as in Datetime
Note that negative or extended (more than 4 digit) years are not permitted.
EXAMPLE: A Next Escrow Review Date that discloses the year and month would be expressed as \"2010-06\"."""^^xsd:string .


###  http://mismo.org/Subset/MISMOIdentifier
:MISMOIdentifier rdf:type owl:Class ;
                 rdfs:subClassOf <http://mismo.org/DataTypes/MISMOIdentifier_Base> ,
                                 [ rdf:type owl:Restriction ;
                                   owl:onProperty :DataNotSuppliedReasonTypeAdditionalDescription ;
                                   owl:cardinality "1"^^xsd:nonNegativeInteger
                                 ] ,
                                 [ rdf:type owl:Restriction ;
                                   owl:onProperty :DataNotSuppliedReasonTypeOtherDescription ;
                                   owl:cardinality "1"^^xsd:nonNegativeInteger
                                 ] ,
                                 [ rdf:type owl:Restriction ;
                                   owl:onProperty :IdentifierEffectiveDate ;
                                   owl:cardinality "1"^^xsd:nonNegativeInteger
                                 ] ,
                                 [ rdf:type owl:Restriction ;
                                   owl:onProperty :IdentifierOwnerURI ;
                                   owl:cardinality "1"^^xsd:nonNegativeInteger
                                 ] ,
                                 [ rdf:type owl:Restriction ;
                                   owl:onProperty :SensitiveIndicator ;
                                   owl:cardinality "1"^^xsd:nonNegativeInteger
                                 ] ,
                                 [ rdf:type owl:Restriction ;
                                   owl:onProperty :DataNotSuppliedReasonType ;
                                   owl:qualifiedCardinality "1"^^xsd:nonNegativeInteger ;
                                   owl:onDataRange <http://mismo.org/DataTypes/DataNotSuppliedReasonBase>
                                 ] ;
                 rdfs:comment """A data type of Identifier SHOULD identify a data point that provides a unique value for reference purposes and MAY have IdentifierOwnerURI and IdentifierEffectiveDate attributes.
EXAMPLE: A Loan Identifier could be expressed as \"0034567891-A\"."""^^xsd:string .


###  http://mismo.org/Subset/MISMOIndicator
:MISMOIndicator rdf:type owl:Class ;
                rdfs:subClassOf <http://mismo.org/DataTypes/MISMOIndicator_Base> ,
                                [ rdf:type owl:Restriction ;
                                  owl:onProperty :DataNotSuppliedReasonTypeAdditionalDescription ;
                                  owl:cardinality "1"^^xsd:nonNegativeInteger
                                ] ,
                                [ rdf:type owl:Restriction ;
                                  owl:onProperty :DataNotSuppliedReasonTypeOtherDescription ;
                                  owl:cardinality "1"^^xsd:nonNegativeInteger
                                ] ,
                                [ rdf:type owl:Restriction ;
                                  owl:onProperty :SensitiveIndicator ;
                                  owl:cardinality "1"^^xsd:nonNegativeInteger
                                ] ,
                                [ rdf:type owl:Restriction ;
                                  owl:onProperty :DataNotSuppliedReasonType ;
                                  owl:qualifiedCardinality "1"^^xsd:nonNegativeInteger ;
                                  owl:onDataRange <http://mismo.org/DataTypes/DataNotSuppliedReasonBase>
                                ] ;
                rdfs:comment """A data type of Indicator SHOULD identify a data point that represents a boolean value.
The value choices SHOULD be \"true\" or \"false\" but MAY be \"1\" or \"0\".
EXAMPLE: A Basement Finished Indicator for a basement that qualifies would be expressed as \"true\"."""^^xsd:string .


###  http://mismo.org/Subset/MISMORate
:MISMORate rdf:type owl:Class ;
           rdfs:subClassOf <http://mismo.org/DataTypes/MISMORate_Base> ,
                           [ rdf:type owl:Restriction ;
                             owl:onProperty :DataNotSuppliedReasonTypeAdditionalDescription ;
                             owl:cardinality "1"^^xsd:nonNegativeInteger
                           ] ,
                           [ rdf:type owl:Restriction ;
                             owl:onProperty :DataNotSuppliedReasonTypeOtherDescription ;
                             owl:cardinality "1"^^xsd:nonNegativeInteger
                           ] ,
                           [ rdf:type owl:Restriction ;
                             owl:onProperty :SensitiveIndicator ;
                             owl:cardinality "1"^^xsd:nonNegativeInteger
                           ] ,
                           [ rdf:type owl:Restriction ;
                             owl:onProperty :DataNotSuppliedReasonType ;
                             owl:qualifiedCardinality "1"^^xsd:nonNegativeInteger ;
                             owl:onDataRange <http://mismo.org/DataTypes/DataNotSuppliedReasonBase>
                           ] ;
           rdfs:comment """A data type of Rate SHOULD identify a number value that is in the subset of real numbers expressible by decimal numerals and represents a value that is a ratio. It MAY contain a single decimal point as punctuation. The decimal point is ALWAYS the US nationalization character (.) in the designated character encoding (UTF-8 assumed when not stated.)
It SHOULD be able to contain at least 18 digits.
EXAMPLE: A Tax Rate of 5 percent for computing annual taxes based on a property's value would be expressed as \".05\"."""^^xsd:string .


###  http://mismo.org/Subset/MISMOString
:MISMOString rdf:type owl:Class ;
             rdfs:subClassOf <http://mismo.org/DataTypes/MISMOString_Base> ,
                             [ rdf:type owl:Restriction ;
                               owl:onProperty :DataNotSuppliedReasonTypeAdditionalDescription ;
                               owl:cardinality "1"^^xsd:nonNegativeInteger
                             ] ,
                             [ rdf:type owl:Restriction ;
                               owl:onProperty :DataNotSuppliedReasonTypeOtherDescription ;
                               owl:cardinality "1"^^xsd:nonNegativeInteger
                             ] ,
                             [ rdf:type owl:Restriction ;
                               owl:onProperty :SensitiveIndicator ;
                               owl:cardinality "1"^^xsd:nonNegativeInteger
                             ] ,
                             [ rdf:type owl:Restriction ;
                               owl:onProperty :lang ;
                               owl:cardinality "1"^^xsd:nonNegativeInteger
                             ] ,
                             [ rdf:type owl:Restriction ;
                               owl:onProperty :DataNotSuppliedReasonType ;
                               owl:qualifiedCardinality "1"^^xsd:nonNegativeInteger ;
                               owl:onDataRange <http://mismo.org/DataTypes/DataNotSuppliedReasonBase>
                             ] ;
             rdfs:comment """A data type of String SHOULD identify a data point that is either a text value consisting of a word, phrase, sentence, paragraph, or formatted (TAB, CR, LF) character content depending on its purpose or a numeric value with a maximum of 16383 characters and MAY have the lang attribute. There is no list of valid values provided.
EXAMPLE: A Disqualificaton Reason Text for excluding a product from those offered to a borrower could be expressed as \"Does not meet income to indebtedness guidelines for down payment support.\"."""^^xsd:string .


###  http://mismo.org/Subset/Pool
:Pool rdf:type owl:Class ;
      rdfs:subClassOf [ rdf:type owl:Restriction ;
                        owl:onProperty :amortizationType ;
                        owl:cardinality "1"^^xsd:nonNegativeInteger
                      ] ,
                      [ rdf:type owl:Restriction ;
                        owl:onProperty :amortizationTypeOtherDescription ;
                        owl:cardinality "1"^^xsd:nonNegativeInteger
                      ] ,
                      [ rdf:type owl:Restriction ;
                        owl:onProperty :cusip-Identifier ;
                        owl:cardinality "1"^^xsd:nonNegativeInteger
                      ] ,
                      [ rdf:type owl:Restriction ;
                        owl:onProperty :governmentBondFinanceIndicator ;
                        owl:cardinality "1"^^xsd:nonNegativeInteger
                      ] ,
                      [ rdf:type owl:Restriction ;
                        owl:onProperty :governmentBondFinancingProgramType ;
                        owl:cardinality "1"^^xsd:nonNegativeInteger
                      ] ,
                      [ rdf:type owl:Restriction ;
                        owl:onProperty :governmentBondFinancingProgramTypeOtherDescription ;
                        owl:cardinality "1"^^xsd:nonNegativeInteger
                      ] ,
                      [ rdf:type owl:Restriction ;
                        owl:onProperty :poolAccrualRateStructureType ;
                        owl:cardinality "1"^^xsd:nonNegativeInteger
                      ] ,
                      [ rdf:type owl:Restriction ;
                        owl:onProperty :poolAssumabilityIndicator ;
                        owl:cardinality "1"^^xsd:nonNegativeInteger
                      ] ,
                      [ rdf:type owl:Restriction ;
                        owl:onProperty :poolBalloonIndicator ;
                        owl:cardinality "1"^^xsd:nonNegativeInteger
                      ] ,
                      [ rdf:type owl:Restriction ;
                        owl:onProperty :poolClassType ;
                        owl:cardinality "1"^^xsd:nonNegativeInteger
                      ] ,
                      [ rdf:type owl:Restriction ;
                        owl:onProperty :poolClassTypeOtherDescription ;
                        owl:cardinality "1"^^xsd:nonNegativeInteger
                      ] ,
                      [ rdf:type owl:Restriction ;
                        owl:onProperty :poolConcurrentTransferIndicator ;
                        owl:cardinality "1"^^xsd:nonNegativeInteger
                      ] ,
                      [ rdf:type owl:Restriction ;
                        owl:onProperty :poolCurrentLoanCount ;
                        owl:cardinality "1"^^xsd:nonNegativeInteger
                      ] ,
                      [ rdf:type owl:Restriction ;
                        owl:onProperty :poolCurrentPrincipalBalanceAmount ;
                        owl:cardinality "1"^^xsd:nonNegativeInteger
                      ] ,
                      [ rdf:type owl:Restriction ;
                        owl:onProperty :poolFHA-LoanPercent ;
                        owl:cardinality "1"^^xsd:nonNegativeInteger
                      ] ,
                      [ rdf:type owl:Restriction ;
                        owl:onProperty :poolFixedServicingFeePercent ;
                        owl:cardinality "1"^^xsd:nonNegativeInteger
                      ] ,
                      [ rdf:type owl:Restriction ;
                        owl:onProperty :poolGuarantyFeeRatePercent ;
                        owl:cardinality "1"^^xsd:nonNegativeInteger
                      ] ,
                      [ rdf:type owl:Restriction ;
                        owl:onProperty :poolHighestPercentageStateCode ;
                        owl:cardinality "1"^^xsd:nonNegativeInteger
                      ] ,
                      [ rdf:type owl:Restriction ;
                        owl:onProperty :poolHighestStateCodePercent ;
                        owl:cardinality "1"^^xsd:nonNegativeInteger
                      ] ,
                      [ rdf:type owl:Restriction ;
                        owl:onProperty :poolIdentifier ;
                        owl:cardinality "1"^^xsd:nonNegativeInteger
                      ] ,
                      [ rdf:type owl:Restriction ;
                        owl:onProperty :poolInterestAdjustmentEffectiveDate ;
                        owl:cardinality "1"^^xsd:nonNegativeInteger
                      ] ,
                      [ rdf:type owl:Restriction ;
                        owl:onProperty :poolInterestAdjustmentIndexLeadDaysCount ;
                        owl:cardinality "1"^^xsd:nonNegativeInteger
                      ] ,
                      [ rdf:type owl:Restriction ;
                        owl:onProperty :poolInterestAndPaymentAdjustmentIndexLeadDaysCount ;
                        owl:cardinality "1"^^xsd:nonNegativeInteger
                      ] ,
                      [ rdf:type owl:Restriction ;
                        owl:onProperty :poolInterestOnlyIndicator ;
                        owl:cardinality "1"^^xsd:nonNegativeInteger
                      ] ,
                      [ rdf:type owl:Restriction ;
                        owl:onProperty :poolInterestRateRoundingPercent ;
                        owl:cardinality "1"^^xsd:nonNegativeInteger
                      ] ,
                      [ rdf:type owl:Restriction ;
                        owl:onProperty :poolInterestRateRoundingType ;
                        owl:cardinality "1"^^xsd:nonNegativeInteger
                      ] ,
                      [ rdf:type owl:Restriction ;
                        owl:onProperty :poolInterestRateTruncatedDigitsCount ;
                        owl:cardinality "1"^^xsd:nonNegativeInteger
                      ] ,
                      [ rdf:type owl:Restriction ;
                        owl:onProperty :poolInvestorAdditionalProductPlanIdentifier ;
                        owl:cardinality "1"^^xsd:nonNegativeInteger
                      ] ,
                      [ rdf:type owl:Restriction ;
                        owl:onProperty :poolInvestorProductPlanIdentifier ;
                        owl:cardinality "1"^^xsd:nonNegativeInteger
                      ] ,
                      [ rdf:type owl:Restriction ;
                        owl:onProperty :poolIssueDate ;
                        owl:cardinality "1"^^xsd:nonNegativeInteger
                      ] ,
                      [ rdf:type owl:Restriction ;
                        owl:onProperty :poolIssuerIdentifier ;
                        owl:cardinality "1"^^xsd:nonNegativeInteger
                      ] ,
                      [ rdf:type owl:Restriction ;
                        owl:onProperty :poolMarginRatePercent ;
                        owl:cardinality "1"^^xsd:nonNegativeInteger
                      ] ,
                      [ rdf:type owl:Restriction ;
                        owl:onProperty :poolMaturityDate ;
                        owl:cardinality "1"^^xsd:nonNegativeInteger
                      ] ,
                      [ rdf:type owl:Restriction ;
                        owl:onProperty :poolMaximumAccrualRatePercent ;
                        owl:cardinality "1"^^xsd:nonNegativeInteger
                      ] ,
                      [ rdf:type owl:Restriction ;
                        owl:onProperty :poolMinimumAccrualRatePercent ;
                        owl:cardinality "1"^^xsd:nonNegativeInteger
                      ] ,
                      [ rdf:type owl:Restriction ;
                        owl:onProperty :poolModificationLoanPercent ;
                        owl:cardinality "1"^^xsd:nonNegativeInteger
                      ] ,
                      [ rdf:type owl:Restriction ;
                        owl:onProperty :poolMortgageRatePercent ;
                        owl:cardinality "1"^^xsd:nonNegativeInteger
                      ] ,
                      [ rdf:type owl:Restriction ;
                        owl:onProperty :poolMortgageType ;
                        owl:cardinality "1"^^xsd:nonNegativeInteger
                      ] ,
                      [ rdf:type owl:Restriction ;
                        owl:onProperty :poolMortgageTypeOtherDescription ;
                        owl:cardinality "1"^^xsd:nonNegativeInteger
                      ] ,
                      [ rdf:type owl:Restriction ;
                        owl:onProperty :poolNonTPO-LoanPercent ;
                        owl:cardinality "1"^^xsd:nonNegativeInteger
                      ] ,
                      [ rdf:type owl:Restriction ;
                        owl:onProperty :poolOriginalLoanCount ;
                        owl:cardinality "1"^^xsd:nonNegativeInteger
                      ] ,
                      [ rdf:type owl:Restriction ;
                        owl:onProperty :poolOriginalPrincipalBalanceAmount ;
                        owl:cardinality "1"^^xsd:nonNegativeInteger
                      ] ,
                      [ rdf:type owl:Restriction ;
                        owl:onProperty :poolOwnershipPercent ;
                        owl:cardinality "1"^^xsd:nonNegativeInteger
                      ] ,
                      [ rdf:type owl:Restriction ;
                        owl:onProperty :poolPrefixIdentifier ;
                        owl:cardinality "1"^^xsd:nonNegativeInteger
                      ] ,
                      [ rdf:type owl:Restriction ;
                        owl:onProperty :poolPriorPeriodPrincipalBalanceAmount ;
                        owl:cardinality "1"^^xsd:nonNegativeInteger
                      ] ,
                      [ rdf:type owl:Restriction ;
                        owl:onProperty :poolPurchaseLoanPercent ;
                        owl:cardinality "1"^^xsd:nonNegativeInteger
                      ] ,
                      [ rdf:type owl:Restriction ;
                        owl:onProperty :poolScheduledPrincipalAndInterestPaymentAmount ;
                        owl:cardinality "1"^^xsd:nonNegativeInteger
                      ] ,
                      [ rdf:type owl:Restriction ;
                        owl:onProperty :poolScheduledPrincipalBalanceAmount ;
                        owl:cardinality "1"^^xsd:nonNegativeInteger
                      ] ,
                      [ rdf:type owl:Restriction ;
                        owl:onProperty :poolScheduledRemittancePaymentDay ;
                        owl:cardinality "1"^^xsd:nonNegativeInteger
                      ] ,
                      [ rdf:type owl:Restriction ;
                        owl:onProperty :poolSecurityInterestRatePercent ;
                        owl:cardinality "1"^^xsd:nonNegativeInteger
                      ] ,
                      [ rdf:type owl:Restriction ;
                        owl:onProperty :poolSecurityIssueDateInterestRatePercent ;
                        owl:cardinality "1"^^xsd:nonNegativeInteger
                      ] ,
                      [ rdf:type owl:Restriction ;
                        owl:onProperty :poolSecurityParValueAmount ;
                        owl:cardinality "1"^^xsd:nonNegativeInteger
                      ] ,
                      [ rdf:type owl:Restriction ;
                        owl:onProperty :poolSecuritySettlementDate ;
                        owl:cardinality "1"^^xsd:nonNegativeInteger
                      ] ,
                      [ rdf:type owl:Restriction ;
                        owl:onProperty :poolServiceFeeRatePercent ;
                        owl:cardinality "1"^^xsd:nonNegativeInteger
                      ] ,
                      [ rdf:type owl:Restriction ;
                        owl:onProperty :poolStructureType ;
                        owl:cardinality "1"^^xsd:nonNegativeInteger
                      ] ,
                      [ rdf:type owl:Restriction ;
                        owl:onProperty :poolStructureTypeOtherDescription ;
                        owl:cardinality "1"^^xsd:nonNegativeInteger
                      ] ,
                      [ rdf:type owl:Restriction ;
                        owl:onProperty :poolSuffixIdentifier ;
                        owl:cardinality "1"^^xsd:nonNegativeInteger
                      ] ,
                      [ rdf:type owl:Restriction ;
                        owl:onProperty :poolUSDA-LoanPercent ;
                        owl:cardinality "1"^^xsd:nonNegativeInteger
                      ] ,
                      [ rdf:type owl:Restriction ;
                        owl:onProperty :poolUnscheduledPrincipalAmount ;
                        owl:cardinality "1"^^xsd:nonNegativeInteger
                      ] ,
                      [ rdf:type owl:Restriction ;
                        owl:onProperty :poolUnscheduledPrincipalPaymentDay ;
                        owl:cardinality "1"^^xsd:nonNegativeInteger
                      ] ,
                      [ rdf:type owl:Restriction ;
                        owl:onProperty :poolVA-LoanPercent ;
                        owl:cardinality "1"^^xsd:nonNegativeInteger
                      ] ,
                      [ rdf:type owl:Restriction ;
                        owl:onProperty :poolWeightedAverageCombinedLTV-RatioPercent ;
                        owl:cardinality "1"^^xsd:nonNegativeInteger
                      ] ,
                      [ rdf:type owl:Restriction ;
                        owl:onProperty :poolWeightedAverageCouponRatePercent ;
                        owl:cardinality "1"^^xsd:nonNegativeInteger
                      ] ,
                      [ rdf:type owl:Restriction ;
                        owl:onProperty :poolWeightedAverageCreditScoreValue ;
                        owl:cardinality "1"^^xsd:nonNegativeInteger
                      ] ,
                      [ rdf:type owl:Restriction ;
                        owl:onProperty :poolWeightedAverageLTV-RatioPercent ;
                        owl:cardinality "1"^^xsd:nonNegativeInteger
                      ] ,
                      [ rdf:type owl:Restriction ;
                        owl:onProperty :poolWeightedAverageOriginalUnpaidLoanBalanceAmount ;
                        owl:cardinality "1"^^xsd:nonNegativeInteger
                      ] ,
                      [ rdf:type owl:Restriction ;
                        owl:onProperty :poolingMethodType ;
                        owl:cardinality "1"^^xsd:nonNegativeInteger
                      ] ,
                      [ rdf:type owl:Restriction ;
                        owl:onProperty :poolingMethodTypeOtherDescription ;
                        owl:cardinality "1"^^xsd:nonNegativeInteger
                      ] ,
                      [ rdf:type owl:Restriction ;
                        owl:onProperty :positionOnePoolBidAmount ;
                        owl:cardinality "1"^^xsd:nonNegativeInteger
                      ] ,
                      [ rdf:type owl:Restriction ;
                        owl:onProperty :positionTwoPoolBidAmount ;
                        owl:cardinality "1"^^xsd:nonNegativeInteger
                      ] ,
                      [ rdf:type owl:Restriction ;
                        owl:onProperty :securityTradeBookEntryDate ;
                        owl:cardinality "1"^^xsd:nonNegativeInteger
                      ] ,
                      [ rdf:type owl:Restriction ;
                        owl:onProperty :securityTradeCustomerAccountIdentifier ;
                        owl:cardinality "1"^^xsd:nonNegativeInteger
                      ] ,
                      [ rdf:type owl:Restriction ;
                        owl:onProperty :extension ;
                        owl:maxCardinality "1"^^xsd:nonNegativeInteger
                      ] ;
      rdfs:comment "Holds data on multiple loans transmitted as a pool."^^xsd:string .


###  http://mismo.org/Subset/Property
:Property rdf:type owl:Class ;
          rdfs:subClassOf [ rdf:type owl:Restriction ;
                            owl:onProperty :accessoryDwellingUnitTotalCount ;
                            owl:cardinality "1"^^xsd:nonNegativeInteger
                          ] ,
                          [ rdf:type owl:Restriction ;
                            owl:onProperty :affordableUnitsCount ;
                            owl:cardinality "1"^^xsd:nonNegativeInteger
                          ] ,
                          [ rdf:type owl:Restriction ;
                            owl:onProperty :assignmentOfRentsIndicator ;
                            owl:cardinality "1"^^xsd:nonNegativeInteger
                          ] ,
                          [ rdf:type owl:Restriction ;
                            owl:onProperty :attachmentType ;
                            owl:cardinality "1"^^xsd:nonNegativeInteger
                          ] ,
                          [ rdf:type owl:Restriction ;
                            owl:onProperty :borrowerContinuesToOwnPropertyIndicator ;
                            owl:cardinality "1"^^xsd:nonNegativeInteger
                          ] ,
                          [ rdf:type owl:Restriction ;
                            owl:onProperty :buildingCount ;
                            owl:cardinality "1"^^xsd:nonNegativeInteger
                          ] ,
                          [ rdf:type owl:Restriction ;
                            owl:onProperty :communityLandTrustIndicator ;
                            owl:cardinality "1"^^xsd:nonNegativeInteger
                          ] ,
                          [ rdf:type owl:Restriction ;
                            owl:onProperty :communityPropertyStateIndicator ;
                            owl:cardinality "1"^^xsd:nonNegativeInteger
                          ] ,
                          [ rdf:type owl:Restriction ;
                            owl:onProperty :communityReinvestmentActDelineatedCommunityIndicator ;
                            owl:cardinality "1"^^xsd:nonNegativeInteger
                          ] ,
                          [ rdf:type owl:Restriction ;
                            owl:onProperty :constructionStatusType ;
                            owl:cardinality "1"^^xsd:nonNegativeInteger
                          ] ,
                          [ rdf:type owl:Restriction ;
                            owl:onProperty :constructionStatusTypeOtherDescription ;
                            owl:cardinality "1"^^xsd:nonNegativeInteger
                          ] ,
                          [ rdf:type owl:Restriction ;
                            owl:onProperty :cooperativeProprietaryLeaseExpirationDate ;
                            owl:cardinality "1"^^xsd:nonNegativeInteger
                          ] ,
                          [ rdf:type owl:Restriction ;
                            owl:onProperty :deedRestrictionIndicator ;
                            owl:cardinality "1"^^xsd:nonNegativeInteger
                          ] ,
                          [ rdf:type owl:Restriction ;
                            owl:onProperty :disasterIndicator ;
                            owl:cardinality "1"^^xsd:nonNegativeInteger
                          ] ,
                          [ rdf:type owl:Restriction ;
                            owl:onProperty :dwellingCount ;
                            owl:cardinality "1"^^xsd:nonNegativeInteger
                          ] ,
                          [ rdf:type owl:Restriction ;
                            owl:onProperty :fha-SecondaryResidenceIndicator ;
                            owl:cardinality "1"^^xsd:nonNegativeInteger
                          ] ,
                          [ rdf:type owl:Restriction ;
                            owl:onProperty :financedUnitCount ;
                            owl:cardinality "1"^^xsd:nonNegativeInteger
                          ] ,
                          [ rdf:type owl:Restriction ;
                            owl:onProperty :functionalIssueDescription ;
                            owl:cardinality "1"^^xsd:nonNegativeInteger
                          ] ,
                          [ rdf:type owl:Restriction ;
                            owl:onProperty :grossLivingAreaTotalAreaMeasure ;
                            owl:cardinality "1"^^xsd:nonNegativeInteger
                          ] ,
                          [ rdf:type owl:Restriction ;
                            owl:onProperty :groundRentIndicator ;
                            owl:cardinality "1"^^xsd:nonNegativeInteger
                          ] ,
                          [ rdf:type owl:Restriction ;
                            owl:onProperty :groupHomeIndicator ;
                            owl:cardinality "1"^^xsd:nonNegativeInteger
                          ] ,
                          [ rdf:type owl:Restriction ;
                            owl:onProperty :homeownerResponsibleForExteriorMaintenanceIndicator ;
                            owl:cardinality "1"^^xsd:nonNegativeInteger
                          ] ,
                          [ rdf:type owl:Restriction ;
                            owl:onProperty :homeownersAssociationIndicator ;
                            owl:cardinality "1"^^xsd:nonNegativeInteger
                          ] ,
                          [ rdf:type owl:Restriction ;
                            owl:onProperty :investmentRentalIncomePresentIndicator ;
                            owl:cardinality "1"^^xsd:nonNegativeInteger
                          ] ,
                          [ rdf:type owl:Restriction ;
                            owl:onProperty :investorREO-PropertyIdentifier ;
                            owl:cardinality "1"^^xsd:nonNegativeInteger
                          ] ,
                          [ rdf:type owl:Restriction ;
                            owl:onProperty :landTrustType ;
                            owl:cardinality "1"^^xsd:nonNegativeInteger
                          ] ,
                          [ rdf:type owl:Restriction ;
                            owl:onProperty :landTrustTypeOtherDescription ;
                            owl:cardinality "1"^^xsd:nonNegativeInteger
                          ] ,
                          [ rdf:type owl:Restriction ;
                            owl:onProperty :landUseDescription ;
                            owl:cardinality "1"^^xsd:nonNegativeInteger
                          ] ,
                          [ rdf:type owl:Restriction ;
                            owl:onProperty :landUseType ;
                            owl:cardinality "1"^^xsd:nonNegativeInteger
                          ] ,
                          [ rdf:type owl:Restriction ;
                            owl:onProperty :landUseTypeOtherDescription ;
                            owl:cardinality "1"^^xsd:nonNegativeInteger
                          ] ,
                          [ rdf:type owl:Restriction ;
                            owl:onProperty :lenderDesignatedDecliningMarketIdentifier ;
                            owl:cardinality "1"^^xsd:nonNegativeInteger
                          ] ,
                          [ rdf:type owl:Restriction ;
                            owl:onProperty :livingUnitExcludingADU-Count ;
                            owl:cardinality "1"^^xsd:nonNegativeInteger
                          ] ,
                          [ rdf:type owl:Restriction ;
                            owl:onProperty :metropolitanDivisionIndicator ;
                            owl:cardinality "1"^^xsd:nonNegativeInteger
                          ] ,
                          [ rdf:type owl:Restriction ;
                            owl:onProperty :mineralRightsLeasedIndicator ;
                            owl:cardinality "1"^^xsd:nonNegativeInteger
                          ] ,
                          [ rdf:type owl:Restriction ;
                            owl:onProperty :msa-Indicator ;
                            owl:cardinality "1"^^xsd:nonNegativeInteger
                          ] ,
                          [ rdf:type owl:Restriction ;
                            owl:onProperty :nativeAmericanLandsIndicator ;
                            owl:cardinality "1"^^xsd:nonNegativeInteger
                          ] ,
                          [ rdf:type owl:Restriction ;
                            owl:onProperty :nativeAmericanLandsType ;
                            owl:cardinality "1"^^xsd:nonNegativeInteger
                          ] ,
                          [ rdf:type owl:Restriction ;
                            owl:onProperty :nativeAmericanLandsTypeOtherDescription ;
                            owl:cardinality "1"^^xsd:nonNegativeInteger
                          ] ,
                          [ rdf:type owl:Restriction ;
                            owl:onProperty :newConstructionIndicator ;
                            owl:cardinality "1"^^xsd:nonNegativeInteger
                          ] ,
                          [ rdf:type owl:Restriction ;
                            owl:onProperty :outbuildingCount ;
                            owl:cardinality "1"^^xsd:nonNegativeInteger
                          ] ,
                          [ rdf:type owl:Restriction ;
                            owl:onProperty :overallConditionRatingCode ;
                            owl:cardinality "1"^^xsd:nonNegativeInteger
                          ] ,
                          [ rdf:type owl:Restriction ;
                            owl:onProperty :overallQualityRatingCode ;
                            owl:cardinality "1"^^xsd:nonNegativeInteger
                          ] ,
                          [ rdf:type owl:Restriction ;
                            owl:onProperty :priorSaleInLastTwelveMonthsIndicator ;
                            owl:cardinality "1"^^xsd:nonNegativeInteger
                          ] ,
                          [ rdf:type owl:Restriction ;
                            owl:onProperty :priorSalesOrTransfersIndicator ;
                            owl:cardinality "1"^^xsd:nonNegativeInteger
                          ] ,
                          [ rdf:type owl:Restriction ;
                            owl:onProperty :proRataSharePercent ;
                            owl:cardinality "1"^^xsd:nonNegativeInteger
                          ] ,
                          [ rdf:type owl:Restriction ;
                            owl:onProperty :propertyAcquiredDate ;
                            owl:cardinality "1"^^xsd:nonNegativeInteger
                          ] ,
                          [ rdf:type owl:Restriction ;
                            owl:onProperty :propertyAcquiredYear ;
                            owl:cardinality "1"^^xsd:nonNegativeInteger
                          ] ,
                          [ rdf:type owl:Restriction ;
                            owl:onProperty :propertyAcreageNumber ;
                            owl:cardinality "1"^^xsd:nonNegativeInteger
                          ] ,
                          [ rdf:type owl:Restriction ;
                            owl:onProperty :propertyAmenityExistsIndicator ;
                            owl:cardinality "1"^^xsd:nonNegativeInteger
                          ] ,
                          [ rdf:type owl:Restriction ;
                            owl:onProperty :propertyConditionDescription ;
                            owl:cardinality "1"^^xsd:nonNegativeInteger
                          ] ,
                          [ rdf:type owl:Restriction ;
                            owl:onProperty :propertyCooperativeSharesCount ;
                            owl:cardinality "1"^^xsd:nonNegativeInteger
                          ] ,
                          [ rdf:type owl:Restriction ;
                            owl:onProperty :propertyCurrentOccupancyType ;
                            owl:cardinality "1"^^xsd:nonNegativeInteger
                          ] ,
                          [ rdf:type owl:Restriction ;
                            owl:onProperty :propertyCurrentOccupantName ;
                            owl:cardinality "1"^^xsd:nonNegativeInteger
                          ] ,
                          [ rdf:type owl:Restriction ;
                            owl:onProperty :propertyDispositionStatusType ;
                            owl:cardinality "1"^^xsd:nonNegativeInteger
                          ] ,
                          [ rdf:type owl:Restriction ;
                            owl:onProperty :propertyDispositionStatusTypeOtherDescription ;
                            owl:cardinality "1"^^xsd:nonNegativeInteger
                          ] ,
                          [ rdf:type owl:Restriction ;
                            owl:onProperty :propertyEarthquakeInsuranceIndicator ;
                            owl:cardinality "1"^^xsd:nonNegativeInteger
                          ] ,
                          [ rdf:type owl:Restriction ;
                            owl:onProperty :propertyEstateType ;
                            owl:cardinality "1"^^xsd:nonNegativeInteger
                          ] ,
                          [ rdf:type owl:Restriction ;
                            owl:onProperty :propertyEstateTypeOtherDescription ;
                            owl:cardinality "1"^^xsd:nonNegativeInteger
                          ] ,
                          [ rdf:type owl:Restriction ;
                            owl:onProperty :propertyEstimatedValueAmount ;
                            owl:cardinality "1"^^xsd:nonNegativeInteger
                          ] ,
                          [ rdf:type owl:Restriction ;
                            owl:onProperty :propertyExistingCleanEnergyLienIndicator ;
                            owl:cardinality "1"^^xsd:nonNegativeInteger
                          ] ,
                          [ rdf:type owl:Restriction ;
                            owl:onProperty :propertyExistingLienAmount ;
                            owl:cardinality "1"^^xsd:nonNegativeInteger
                          ] ,
                          [ rdf:type owl:Restriction ;
                            owl:onProperty :propertyFloodInsuranceIndicator ;
                            owl:cardinality "1"^^xsd:nonNegativeInteger
                          ] ,
                          [ rdf:type owl:Restriction ;
                            owl:onProperty :propertyForeclosureCount ;
                            owl:cardinality "1"^^xsd:nonNegativeInteger
                          ] ,
                          [ rdf:type owl:Restriction ;
                            owl:onProperty :propertyInProjectIndicator ;
                            owl:cardinality "1"^^xsd:nonNegativeInteger
                          ] ,
                          [ rdf:type owl:Restriction ;
                            owl:onProperty :propertyInclusionaryZoningIndicator ;
                            owl:cardinality "1"^^xsd:nonNegativeInteger
                          ] ,
                          [ rdf:type owl:Restriction ;
                            owl:onProperty :propertyOriginalCostAmount ;
                            owl:cardinality "1"^^xsd:nonNegativeInteger
                          ] ,
                          [ rdf:type owl:Restriction ;
                            owl:onProperty :propertyPreviouslyOccupiedIndicator ;
                            owl:cardinality "1"^^xsd:nonNegativeInteger
                          ] ,
                          [ rdf:type owl:Restriction ;
                            owl:onProperty :propertyStructureHabitableYearRoundIndicator ;
                            owl:cardinality "1"^^xsd:nonNegativeInteger
                          ] ,
                          [ rdf:type owl:Restriction ;
                            owl:onProperty :propertyUsageType ;
                            owl:cardinality "1"^^xsd:nonNegativeInteger
                          ] ,
                          [ rdf:type owl:Restriction ;
                            owl:onProperty :propertyUsageTypeOtherDescription ;
                            owl:cardinality "1"^^xsd:nonNegativeInteger
                          ] ,
                          [ rdf:type owl:Restriction ;
                            owl:onProperty :propertyVacancyDate ;
                            owl:cardinality "1"^^xsd:nonNegativeInteger
                          ] ,
                          [ rdf:type owl:Restriction ;
                            owl:onProperty :pud-Indicator ;
                            owl:cardinality "1"^^xsd:nonNegativeInteger
                          ] ,
                          [ rdf:type owl:Restriction ;
                            owl:onProperty :rentalEstimatedGrossMonthlyRentAmount ;
                            owl:cardinality "1"^^xsd:nonNegativeInteger
                          ] ,
                          [ rdf:type owl:Restriction ;
                            owl:onProperty :rentalEstimatedNetMonthlyRentAmount ;
                            owl:cardinality "1"^^xsd:nonNegativeInteger
                          ] ,
                          [ rdf:type owl:Restriction ;
                            owl:onProperty :ruralUnderservedCountyIndicator ;
                            owl:cardinality "1"^^xsd:nonNegativeInteger
                          ] ,
                          [ rdf:type owl:Restriction ;
                            owl:onProperty :sequenceNumber ;
                            owl:cardinality "1"^^xsd:nonNegativeInteger
                          ] ,
                          [ rdf:type owl:Restriction ;
                            owl:onProperty :sketchExistsIndicator ;
                            owl:cardinality "1"^^xsd:nonNegativeInteger
                          ] ,
                          [ rdf:type owl:Restriction ;
                            owl:onProperty :subjectPropertyAmenitiesDefectsExistIndicator ;
                            owl:cardinality "1"^^xsd:nonNegativeInteger
                          ] ,
                          [ rdf:type owl:Restriction ;
                            owl:onProperty :totalFinishedAreaOfAllLivingUnitsIncludingADU-AreaMeasure ;
                            owl:cardinality "1"^^xsd:nonNegativeInteger
                          ] ,
                          [ rdf:type owl:Restriction ;
                            owl:onProperty :totalNonContinuousFinishedAreaOfAllDwellingsAreaMeasure ;
                            owl:cardinality "1"^^xsd:nonNegativeInteger
                          ] ,
                          [ rdf:type owl:Restriction ;
                            owl:onProperty :totalOfAllDwellingsVolumeMeasure ;
                            owl:cardinality "1"^^xsd:nonNegativeInteger
                          ] ,
                          [ rdf:type owl:Restriction ;
                            owl:onProperty :totalWindowSurfaceAreaOfAllDwellingsAreaMeasure ;
                            owl:cardinality "1"^^xsd:nonNegativeInteger
                          ] ,
                          [ rdf:type owl:Restriction ;
                            owl:onProperty :undefinedPropertyType ;
                            owl:cardinality "1"^^xsd:nonNegativeInteger
                          ] ,
                          [ rdf:type owl:Restriction ;
                            owl:onProperty :uniqueDwellingType ;
                            owl:cardinality "1"^^xsd:nonNegativeInteger
                          ] ,
                          [ rdf:type owl:Restriction ;
                            owl:onProperty :uniqueDwellingTypeOtherDescription ;
                            owl:cardinality "1"^^xsd:nonNegativeInteger
                          ] ,
                          [ rdf:type owl:Restriction ;
                            owl:onProperty :vehicleStorageDefectsExistIndicator ;
                            owl:cardinality "1"^^xsd:nonNegativeInteger
                          ] ,
                          [ rdf:type owl:Restriction ;
                            owl:onProperty :address ;
                            owl:maxCardinality "1"^^xsd:nonNegativeInteger
                          ] ,
                          [ rdf:type owl:Restriction ;
                            owl:onProperty :comparable ;
                            owl:maxCardinality "1"^^xsd:nonNegativeInteger
                          ] ,
                          [ rdf:type owl:Restriction ;
                            owl:onProperty :energyEfficiencyAndGreen ;
                            owl:maxCardinality "1"^^xsd:nonNegativeInteger
                          ] ,
                          [ rdf:type owl:Restriction ;
                            owl:onProperty :extension ;
                            owl:maxCardinality "1"^^xsd:nonNegativeInteger
                          ] ,
                          [ rdf:type owl:Restriction ;
                            owl:onProperty :floodDetermination ;
                            owl:maxCardinality "1"^^xsd:nonNegativeInteger
                          ] ,
                          [ rdf:type owl:Restriction ;
                            owl:onProperty :listingInformationSummary ;
                            owl:maxCardinality "1"^^xsd:nonNegativeInteger
                          ] ,
                          [ rdf:type owl:Restriction ;
                            owl:onProperty :locationIdentifier ;
                            owl:maxCardinality "1"^^xsd:nonNegativeInteger
                          ] ,
                          [ rdf:type owl:Restriction ;
                            owl:onProperty :market ;
                            owl:maxCardinality "1"^^xsd:nonNegativeInteger
                          ] ,
                          [ rdf:type owl:Restriction ;
                            owl:onProperty :neighborhood ;
                            owl:maxCardinality "1"^^xsd:nonNegativeInteger
                          ] ,
                          [ rdf:type owl:Restriction ;
                            owl:onProperty :parcelSummary ;
                            owl:maxCardinality "1"^^xsd:nonNegativeInteger
                          ] ,
                          [ rdf:type owl:Restriction ;
                            owl:onProperty :project ;
                            owl:maxCardinality "1"^^xsd:nonNegativeInteger
                          ] ,
                          [ rdf:type owl:Restriction ;
                            owl:onProperty :propertyAmenity ;
                            owl:maxCardinality "1"^^xsd:nonNegativeInteger
                          ] ,
                          [ rdf:type owl:Restriction ;
                            owl:onProperty :propertyDefect ;
                            owl:maxCardinality "1"^^xsd:nonNegativeInteger
                          ] ,
                          [ rdf:type owl:Restriction ;
                            owl:onProperty :propertyGroundRent ;
                            owl:maxCardinality "1"^^xsd:nonNegativeInteger
                          ] ,
                          [ rdf:type owl:Restriction ;
                            owl:onProperty :propertyNotUsed ;
                            owl:maxCardinality "1"^^xsd:nonNegativeInteger
                          ] ,
                          [ rdf:type owl:Restriction ;
                            owl:onProperty :propertyTitle ;
                            owl:maxCardinality "1"^^xsd:nonNegativeInteger
                          ] ,
                          [ rdf:type owl:Restriction ;
                            owl:onProperty :propertyUseSummary ;
                            owl:maxCardinality "1"^^xsd:nonNegativeInteger
                          ] ,
                          [ rdf:type owl:Restriction ;
                            owl:onProperty :rentalInformationSummary ;
                            owl:maxCardinality "1"^^xsd:nonNegativeInteger
                          ] ,
                          [ rdf:type owl:Restriction ;
                            owl:onProperty :repair ;
                            owl:maxCardinality "1"^^xsd:nonNegativeInteger
                          ] ,
                          [ rdf:type owl:Restriction ;
                            owl:onProperty :site ;
                            owl:maxCardinality "1"^^xsd:nonNegativeInteger
                          ] ,
                          [ rdf:type owl:Restriction ;
                            owl:onProperty :valuationUseType ;
                            owl:qualifiedCardinality "1"^^xsd:nonNegativeInteger ;
                            owl:onDataRange <http://mismo.org/EnumeratedTypes/ValuationUseBase>
                          ] ;
          rdfs:comment "Information specific to a real estate in terms of land structure, location and market."^^xsd:string .


###  Generated by the OWL API (version 5.0.2.20160507-1747) https://github.com/owlcs/owlapi/
###  Warning: type declarations were not added automatically.


## Generated using the No Magic Cameo Concept Modeler (19.0 SP3, build 20190909_1921-137b5364) on 2024-05-02 at 20:42:54 GMT